abs1_comb_thm/abs1_comb_hold_ref_rel_tau_combScript.sml
@@ -14,103 +14,19 @@ FULL_SIMP_TAC (arith_ss++WORD_ss) []);
 val n_tau_tr_dr_init_setting_1 = store_thm("n_tau_tr_dr_init_setting_1",
 ``!dr spi. 
 dr.state = dr_init_setting /\ spi.state = init_setregs /\
-~ dr.dr_init.issue_wr_ch0conf_mode /\ ~ dr.dr_init.issue_wr_ch0conf_speed /\
-dr.dr_init.issue_wr_ch0conf_wl /\ dr.dr_init.issue_wr_modulctrl /\
-dr.dr_init.issue_wr_sysconfig /\  spi.init.sysconfig_mode_done /\
-spi.init.modulctrl_bus_done /\ spi.init.ch0conf_wordlen_done /\
-~spi.init.ch0conf_mode_done /\ ~spi.init.ch0conf_speed_done ==>
-n_tau_tr (SUC 0) local_tr (dr,spi) tau 
-(dr with <| state := dr_ready; 
-dr_init := dr.dr_init with
-<| issue_wr_ch0conf_mode := T; issue_wr_ch0conf_speed := T|> |>, 
-spi with <|state := spi_ready;
-regs := spi.regs with CH0CONF := spi.regs.CH0CONF with
-<|PHA := 0w; POL := 0w; CLKD := 6w; EPOL := 1w; TRM := 0w;
-DPE0 := 1w; DPE1 := 0w; IS := 0w|>;
-init := spi.init with <|ch0conf_mode_done := T; ch0conf_speed_done := T|> |>)``,
-rw [n_tau_tr_def, local_tr_cases, driver_tr_cases, spi_tr_cases, 
-DR_TAU_ENABLE_def, SPI_TAU_ENABLE_def, DR_WR_ENABLE_def, DR_RD_ENABLE_def] >>
-`(dr_write_state dr = dr with <| state := dr_init_setting;
-dr_init := dr.dr_init with issue_wr_ch0conf_mode := T |>) /\
-(dr_write_address dr = SOME SPI0_CH0CONF) /\
-(dr_write_value dr = SOME (0x00010040w:word32))` 
-by rw [dr_write_state_def, dr_write_address_def, dr_write_value_def,
-dr_write_def, dr_write_ch0conf_mode_def] >>
-rw [dr_write_state_def, dr_write_address_def, dr_write_value_def, dr_write_def,
-dr_write_ch0conf_speed_def] >>
-rw [write_SPI_regs_def, SPI0_CH0CONF_def, SPI0_PA_RANGE_def, 
-SPI0_START_def, SPI0_END_def, SPI0_SYSCONFIG_def, 
-SPI0_MODULCTRL_def, SPI0_TX0_def, write_CH0CONF_comb_def, 
-write_CH0CONF_def, write_CH0CONF_speed_def]);
-
-(* dr.state = dr_init_setting and spi.state = init_setregs, 2 steps before the final one *)
-val n_tau_tr_dr_init_setting_2 = store_thm("n_tau_tr_dr_init_setting_2",
-``!dr spi. 
-dr.state = dr_init_setting /\ spi.state = init_setregs /\
-~ dr.dr_init.issue_wr_ch0conf_mode /\ ~ dr.dr_init.issue_wr_ch0conf_speed /\
-~ dr.dr_init.issue_wr_ch0conf_wl /\ dr.dr_init.issue_wr_modulctrl /\
-dr.dr_init.issue_wr_sysconfig /\ spi.init.sysconfig_mode_done /\
-spi.init.modulctrl_bus_done /\ ~spi.init.ch0conf_wordlen_done /\
-~spi.init.ch0conf_mode_done /\ ~spi.init.ch0conf_speed_done ==>
-n_tau_tr 2 local_tr (dr,spi) tau 
-(dr with <| state := dr_ready; 
-dr_init := dr.dr_init with
-<| issue_wr_ch0conf_wl := T; issue_wr_ch0conf_mode := T; 
-issue_wr_ch0conf_speed := T |> |>, 
-spi with <|state := spi_ready;
-regs := spi.regs with CH0CONF := spi.regs.CH0CONF with
-<|PHA := 0w; POL := 0w; CLKD := 6w; EPOL := 1w; WL := 7w; 
-TRM := 0w; DPE0 := 1w; DPE1 := 0w; IS := 0w|>;
-init := spi.init with <|ch0conf_wordlen_done :=  T; 
-ch0conf_mode_done := T; ch0conf_speed_done := T|> |>)``,
-rw [n_tau_tr_def, n_tau_tr_SUC, local_tr_cases, driver_tr_cases, spi_tr_cases, 
-DR_TAU_ENABLE_def, SPI_TAU_ENABLE_def, DR_WR_ENABLE_def, DR_RD_ENABLE_def] >>
-`(dr_write_state dr = dr with <| state := dr_init_setting;
-dr_init := dr.dr_init with issue_wr_ch0conf_wl := T |>) /\
-(dr_write_address dr = SOME SPI0_CH0CONF) /\
-(dr_write_value dr = SOME (0x00000380w:word32))` 
-by rw [dr_write_state_def, dr_write_address_def, dr_write_value_def,
-dr_write_def, dr_write_ch0conf_wl_def] >>
-rw [] >>
-`7w:word5 >+ 2w:word5` by EVAL_TAC >>
-`write_SPI_regs SPI0_CH0CONF 896w spi = 
-(spi with <|state := init_setregs; 
-regs := spi.regs with CH0CONF := spi.regs.CH0CONF with WL := 7w; 
-init := spi.init with ch0conf_wordlen_done := T|>)`
-by fs [write_SPI_regs_def, SPI0_CH0CONF_def, SPI0_PA_RANGE_def, 
-SPI0_START_def, SPI0_END_def, SPI0_SYSCONFIG_def, SPI0_MODULCTRL_def, 
-SPI0_TX0_def, write_CH0CONF_comb_def, write_CH0CONF_WL_def] >>
-rw [] >>
-rw [dr_write_state_def, dr_write_address_def, dr_write_value_def,
-dr_write_def, dr_write_ch0conf_speed_def, dr_write_ch0conf_mode_def] >>
-fs [write_SPI_regs_def, SPI0_CH0CONF_def, SPI0_PA_RANGE_def, 
-SPI0_START_def, SPI0_END_def, SPI0_SYSCONFIG_def, 
-SPI0_MODULCTRL_def, SPI0_TX0_def, write_CH0CONF_comb_def, 
-write_CH0CONF_def, write_CH0CONF_speed_def]);
-
-(* dr.state = dr_init_setting and spi.state = init_setregs, 3 steps before the final one *)
-val n_tau_tr_dr_init_setting_3 = store_thm("n_tau_tr_dr_init_setting_3",
-``!dr spi. 
-dr.state = dr_init_setting /\ spi.state = init_setregs /\
 dr.dr_init.issue_wr_sysconfig /\ ~ dr.dr_init.issue_wr_modulctrl /\ 
-~ dr.dr_init.issue_wr_ch0conf_wl /\ ~ dr.dr_init.issue_wr_ch0conf_speed /\ 
-~ dr.dr_init.issue_wr_ch0conf_mode /\ spi.init.sysconfig_mode_done /\
-~ spi.init.ch0conf_wordlen_done /\ ~ spi.init.ch0conf_mode_done /\ 
-~ spi.init.ch0conf_speed_done /\ ~ spi.init.modulctrl_bus_done ==>
-n_tau_tr 3 local_tr (dr,spi) tau 
+spi.init.sysconfig_mode_done /\ ~ spi.init.modulctrl_bus_done /\ 
+spi.regs.CH0CONF.WL = 0w /\ spi.regs.CH0CONF.IS = 1w /\ spi.regs.CH0CONF.FORCE = 0w ==>
+n_tau_tr 1 local_tr (dr,spi) tau 
 (dr with <| state := dr_ready; 
-dr_init := dr.dr_init with
-<| issue_wr_modulctrl := T; issue_wr_ch0conf_wl := T; 
-issue_wr_ch0conf_mode := T; issue_wr_ch0conf_speed := T |> |>, 
+dr_init := dr.dr_init with issue_wr_modulctrl := T |>, 
 spi with <|state := spi_ready;
 regs := spi.regs with 
 <| MODULCTRL := <|SYSTEM_TEST := 0w; MS := 0w; SINGLE := 1w|>;
 CH0CONF := spi.regs.CH0CONF with
 <|PHA := 0w; POL := 0w; CLKD := 6w; EPOL := 1w; WL := 7w; 
 TRM := 0w; DPE0 := 1w; DPE1 := 0w; IS := 0w|> |>;
-init := spi.init with 
-<|modulctrl_bus_done := T; ch0conf_wordlen_done :=  T; 
-ch0conf_mode_done := T; ch0conf_speed_done := T|> |>)``, 
+init := spi.init with modulctrl_bus_done := T |>)``, 
 rw [n_tau_tr_def, n_tau_tr_SUC, local_tr_cases, driver_tr_cases, spi_tr_cases, 
 DR_TAU_ENABLE_def, SPI_TAU_ENABLE_def, DR_WR_ENABLE_def, DR_RD_ENABLE_def] >>
 `(dr_write_state dr = dr with <| state := dr_init_setting;
@@ -118,65 +34,48 @@ dr_init := dr.dr_init with issue_wr_modulctrl := T |>) /\
 (dr_write_address dr = SOME SPI0_MODULCTRL) /\
 (dr_write_value dr = SOME (0x00000001w:word32))` 
 by rw [dr_write_state_def, dr_write_address_def, dr_write_value_def,
-dr_write_def, dr_write_modulctrl_def] >>
-rw [] >>
+dr_write_def, dr_write_modulctrl_def] >> rw [] >>
+`~(0w:word5 >+ 2w:word5)` by EVAL_TAC >>
 `write_SPI_regs SPI0_MODULCTRL 1w spi = 
 (spi with <|state := init_setregs; 
 regs := spi.regs with 
 MODULCTRL := <|SYSTEM_TEST := 0w; MS := 0w; SINGLE := 1w|>; 
 init := spi.init with modulctrl_bus_done := T |>)`
-by rw [write_SPI_regs_def, SPI0_PA_RANGE_def, SPI0_START_def, SPI0_END_def, 
-SPI0_SYSCONFIG_def, SPI0_MODULCTRL_def, write_MODULCTRL_def] >>
-rw [] >>
+by fs [write_SPI_regs_def, SPI0_PA_RANGE_def, SPI0_START_def, SPI0_END_def, 
+SPI0_SYSCONFIG_def, SPI0_MODULCTRL_def, write_MODULCTRL_def] >> fs [] >>
 `(dr_write_state (dr with <|state := dr_init_setting;
 dr_init := dr.dr_init with issue_wr_modulctrl := T |>) = 
-dr with <|state := dr_init_setting;
-dr_init := dr.dr_init with 
-<|issue_wr_modulctrl := T; issue_wr_ch0conf_wl := T |> |>) /\
+dr with <|state := dr_ready;
+dr_init := dr.dr_init with issue_wr_modulctrl := T |>) /\
 (dr_write_address (dr with <| state := dr_init_setting;
 dr_init := dr.dr_init with issue_wr_modulctrl := T |>) = SOME SPI0_CH0CONF) /\
 (dr_write_value (dr with <| state := dr_init_setting;
-dr_init := dr.dr_init with issue_wr_modulctrl := T |>) = SOME (0x00000380w:word32))` 
+dr_init := dr.dr_init with issue_wr_modulctrl := T |>) = SOME (66520w:word32))` 
 by fs [dr_write_state_def, dr_write_address_def, dr_write_value_def,
-dr_write_def, dr_write_ch0conf_wl_def] >>
-rw [] >>
+dr_write_def, dr_write_ch0conf_init_def] >> fs [] >>
+`(19 >< 19) (66520w:word32):word1 <> spi.regs.CH0CONF.IS` 
+by FULL_SIMP_TAC (std_ss++WORD_ss) [] >>
+`ch0conf_changed (66520w:word32) 
+(spi with <|state := init_setregs;
+regs:= spi.regs with MODULCTRL := <|SYSTEM_TEST := 0w; MS := 0w; SINGLE := 1w|>;
+init := spi.init with modulctrl_bus_done := T |>)` by fs [ch0conf_changed_def] >>
+rw [write_SPI_regs_def, SPI0_CH0CONF_def, SPI0_PA_RANGE_def, SPI0_START_def, 
+SPI0_END_def, SPI0_SYSCONFIG_def, SPI0_MODULCTRL_def, SPI0_TX0_def, 
+write_CH0CONF_comb_def, write_CH0CONF_init_def] >>
 `7w:word5 >+ 2w:word5` by EVAL_TAC >>
-`write_SPI_regs SPI0_CH0CONF 896w 
-(spi with <|state := init_setregs; 
-regs := spi.regs with MODULCTRL := <|SYSTEM_TEST := 0w; MS := 0w; SINGLE := 1w|>;
-init := spi.init with modulctrl_bus_done := T |>) = 
-(spi with <|state := init_setregs; 
-regs := spi.regs with <|
-MODULCTRL := <|SYSTEM_TEST := 0w; MS := 0w; SINGLE := 1w|>;
-CH0CONF := spi.regs.CH0CONF with WL := 7w |>;
-init := spi.init with 
-<|ch0conf_wordlen_done := T; modulctrl_bus_done := T |> |>)`
-by fs [write_SPI_regs_def, SPI0_CH0CONF_def, SPI0_PA_RANGE_def, 
-SPI0_START_def, SPI0_END_def, SPI0_SYSCONFIG_def, SPI0_MODULCTRL_def, 
-SPI0_TX0_def, write_CH0CONF_comb_def, write_CH0CONF_WL_def] >>
-rw [] >>
-rw [dr_write_state_def, dr_write_address_def, dr_write_value_def,
-dr_write_def, dr_write_ch0conf_speed_def, dr_write_ch0conf_mode_def] >>
-fs [write_SPI_regs_def, SPI0_CH0CONF_def, SPI0_PA_RANGE_def, 
-SPI0_START_def, SPI0_END_def, SPI0_SYSCONFIG_def, 
-SPI0_MODULCTRL_def, SPI0_TX0_def, write_CH0CONF_comb_def, 
-write_CH0CONF_def, write_CH0CONF_speed_def]);
+fs [ref_rel_def, IS_STATE_REL_def]);
 
-(* dr.state = dr_init_setting and spi.state = init_setregs, 4 steps before the final one *)
-val n_tau_tr_dr_init_setting_4 = store_thm("n_tau_tr_dr_init_setting_4",
+(* dr.state = dr_init_setting and spi.state = init_setregs, 2 steps before the final one *)
+val n_tau_tr_dr_init_setting_2 = store_thm("n_tau_tr_dr_init_setting_2",
 ``!dr spi. 
 dr.state = dr_init_setting /\ spi.state = init_setregs /\
 ~ dr.dr_init.issue_wr_sysconfig /\ ~ dr.dr_init.issue_wr_modulctrl /\ 
-~ dr.dr_init.issue_wr_ch0conf_wl /\ ~ dr.dr_init.issue_wr_ch0conf_speed /\ 
-~ dr.dr_init.issue_wr_ch0conf_mode /\ ~ spi.init.sysconfig_mode_done /\
-~ spi.init.ch0conf_wordlen_done /\ ~ spi.init.ch0conf_mode_done /\ 
-~ spi.init.ch0conf_speed_done /\ ~ spi.init.modulctrl_bus_done ==>
-n_tau_tr 4 local_tr (dr,spi) tau 
+~ spi.init.sysconfig_mode_done /\ ~ spi.init.modulctrl_bus_done /\
+spi.regs.CH0CONF.WL = 0w /\ spi.regs.CH0CONF.IS = 1w /\ 
+spi.regs.CH0CONF.FORCE = 0w ==>
+n_tau_tr 2 local_tr (dr,spi) tau 
 (dr with <| state := dr_ready; 
-dr_init := 
-<| issue_wr_sysconfig := T; issue_wr_modulctrl := T; 
-issue_wr_ch0conf_wl := T; issue_wr_ch0conf_mode := T; 
-issue_wr_ch0conf_speed := T |> |>, 
+dr_init := <| issue_wr_sysconfig := T; issue_wr_modulctrl := T |> |>, 
 spi with <|state := spi_ready;
 regs := spi.regs with 
 <| SYSCONFIG := spi.regs.SYSCONFIG with <|SIDLEMODE := 2w; AUTOIDLE := 1w|>;
@@ -184,10 +83,7 @@ MODULCTRL := <|SYSTEM_TEST := 0w; MS := 0w; SINGLE := 1w|>;
 CH0CONF := spi.regs.CH0CONF with
 <|PHA := 0w; POL := 0w; CLKD := 6w; EPOL := 1w; WL := 7w; 
 TRM := 0w; DPE0 := 1w; DPE1 := 0w; IS := 0w|> |>;
-init :=
-<|sysconfig_mode_done := T; modulctrl_bus_done := T; 
-ch0conf_wordlen_done :=  T; ch0conf_mode_done := T; 
-ch0conf_speed_done := T|> |>)``, 
+init := <|sysconfig_mode_done := T; modulctrl_bus_done := T |> |>)``, 
 rw [n_tau_tr_def, n_tau_tr_SUC, local_tr_cases, driver_tr_cases, spi_tr_cases, 
 DR_TAU_ENABLE_def, SPI_TAU_ENABLE_def, DR_WR_ENABLE_def, DR_RD_ENABLE_def] >>
 `(dr_write_state dr = dr with <| state := dr_init_setting;
@@ -195,16 +91,14 @@ dr_init := dr.dr_init with issue_wr_sysconfig := T |>) /\
 (dr_write_address dr = SOME SPI0_SYSCONFIG) /\
 (dr_write_value dr = SOME (0x00000011w:word32))` 
 by rw [dr_write_state_def, dr_write_address_def, dr_write_value_def,
-dr_write_def, dr_write_sysconfig_def] >>
-rw [] >>
+dr_write_def, dr_write_sysconfig_def] >> rw [] >>
 `write_SPI_regs SPI0_SYSCONFIG 17w spi = 
 (spi with <|state := init_setregs; 
 regs := spi.regs with 
 SYSCONFIG := spi.regs.SYSCONFIG with <|SIDLEMODE := 2w; AUTOIDLE := 1w|>; 
 init := spi.init with sysconfig_mode_done := T |>)`
 by rw [write_SPI_regs_def, SPI0_PA_RANGE_def, SPI0_START_def, SPI0_END_def, 
-SPI0_SYSCONFIG_def, write_SYSCONFIG_comb_def, write_SYSCONFIG_def] >>
-rw [] >>
+SPI0_SYSCONFIG_def, write_SYSCONFIG_comb_def, write_SYSCONFIG_def] >> rw [] >>
 `(dr_write_state (dr with <|state := dr_init_setting;
 dr_init := dr.dr_init with issue_wr_sysconfig := T |>) = 
 dr with <|state := dr_init_setting;
@@ -215,8 +109,8 @@ dr_init := dr.dr_init with issue_wr_sysconfig := T |>) = SOME SPI0_MODULCTRL) /\
 (dr_write_value (dr with <| state := dr_init_setting;
 dr_init := dr.dr_init with issue_wr_sysconfig := T |>) = SOME (0x00000001w))` 
 by fs [dr_write_state_def, dr_write_address_def, dr_write_value_def,
-dr_write_def, dr_write_modulctrl_def] >>
-rw [] >>
+dr_write_def, dr_write_modulctrl_def] >> rw [] >>
+`~(0w:word5 >+ 2w:word5)` by EVAL_TAC >>
 `write_SPI_regs SPI0_MODULCTRL 1w 
 (spi with <|state := init_setregs; regs := spi.regs with 
 SYSCONFIG := spi.regs.SYSCONFIG with <|SIDLEMODE := 2w; AUTOIDLE := 1w|>; 
@@ -226,65 +120,46 @@ init := spi.init with sysconfig_mode_done := T |>) =
 MODULCTRL := <|SYSTEM_TEST := 0w; MS := 0w; SINGLE := 1w|> |>;
 init := spi.init with <|sysconfig_mode_done := T; modulctrl_bus_done := T |> |>)`
 by rw [write_SPI_regs_def, SPI0_PA_RANGE_def, SPI0_START_def, SPI0_END_def, 
-SPI0_SYSCONFIG_def, SPI0_MODULCTRL_def, write_MODULCTRL_def] >>
-rw [] >>
+SPI0_SYSCONFIG_def, SPI0_MODULCTRL_def, write_MODULCTRL_def] >> fs [] >>
 `(dr_write_state (dr with <|state := dr_init_setting;
-dr_init := dr.dr_init with <|issue_wr_sysconfig := T; issue_wr_modulctrl := T|> |>) = 
-dr with <|state := dr_init_setting;
-dr_init := dr.dr_init with 
-<|issue_wr_sysconfig := T; issue_wr_modulctrl := T; issue_wr_ch0conf_wl := T |> |>) /\
+dr_init := <|issue_wr_sysconfig := T; issue_wr_modulctrl := T|> |>) = 
+dr with <|state := dr_ready;
+dr_init := <|issue_wr_sysconfig := T; issue_wr_modulctrl := T|> |>) /\
 (dr_write_address (dr with <|state := dr_init_setting;
-dr_init := dr.dr_init with <|issue_wr_sysconfig := T; issue_wr_modulctrl := T|> |>) = 
+dr_init := <|issue_wr_sysconfig := T; issue_wr_modulctrl := T|> |>) = 
 SOME SPI0_CH0CONF) /\
 (dr_write_value (dr with <|state := dr_init_setting;
-dr_init := dr.dr_init with <|issue_wr_sysconfig := T; issue_wr_modulctrl := T|> |>) = 
-SOME (0x00000380w:word32))` 
+dr_init := <|issue_wr_sysconfig := T; issue_wr_modulctrl := T|> |>) = 
+SOME (66520w:word32))` 
 by fs [dr_write_state_def, dr_write_address_def, dr_write_value_def,
-dr_write_def, dr_write_ch0conf_wl_def] >>
-rw [] >>
-`7w:word5 >+ 2w:word5` by EVAL_TAC >>
-`write_SPI_regs SPI0_CH0CONF 896w 
-(spi with <|state := init_setregs; 
-regs := spi.regs with 
-<| SYSCONFIG := spi.regs.SYSCONFIG with <|SIDLEMODE := 2w; AUTOIDLE := 1w|>;
+dr_write_def, dr_write_ch0conf_init_def] >> fs [] >>
+`(19 >< 19) (66520w:word32):word1 <> spi.regs.CH0CONF.IS` 
+by FULL_SIMP_TAC (std_ss++WORD_ss) [] >>
+`ch0conf_changed (66520w:word32) 
+(spi with <|state := init_setregs;
+regs:= spi.regs with <|SYSCONFIG := spi.regs.SYSCONFIG with 
+<|SIDLEMODE := 2w; AUTOIDLE := 1w|>;
 MODULCTRL := <|SYSTEM_TEST := 0w; MS := 0w; SINGLE := 1w|> |>;
-init := spi.init with 
-<|sysconfig_mode_done := T; modulctrl_bus_done := T|> |>) = 
-(spi with <|state := init_setregs; 
-regs := spi.regs with <|
-SYSCONFIG := spi.regs.SYSCONFIG with <|SIDLEMODE := 2w; AUTOIDLE := 1w|>;
-MODULCTRL := <|SYSTEM_TEST := 0w; MS := 0w; SINGLE := 1w|>;
-CH0CONF := spi.regs.CH0CONF with WL := 7w |>;
-init := spi.init with 
-<|ch0conf_wordlen_done := T; sysconfig_mode_done := T; modulctrl_bus_done := T |> |>)`
-by fs [write_SPI_regs_def, SPI0_CH0CONF_def, SPI0_PA_RANGE_def, 
-SPI0_START_def, SPI0_END_def, SPI0_SYSCONFIG_def, SPI0_MODULCTRL_def, 
-SPI0_TX0_def, write_CH0CONF_comb_def, write_CH0CONF_WL_def] >>
-rw [] >>
-rw [dr_write_state_def, dr_write_address_def, dr_write_value_def,
-dr_write_def, dr_write_ch0conf_speed_def, dr_write_ch0conf_mode_def] >>
-fs [write_SPI_regs_def, SPI0_CH0CONF_def, SPI0_PA_RANGE_def, 
-SPI0_START_def, SPI0_END_def, SPI0_SYSCONFIG_def, 
-SPI0_MODULCTRL_def, SPI0_TX0_def, write_CH0CONF_comb_def, 
-write_CH0CONF_def, write_CH0CONF_speed_def]);
+init := <|sysconfig_mode_done := T; modulctrl_bus_done := T|> |>)` by fs [ch0conf_changed_def] >>
+rw [write_SPI_regs_def, SPI0_CH0CONF_def, SPI0_PA_RANGE_def, SPI0_START_def, 
+SPI0_END_def, SPI0_SYSCONFIG_def, SPI0_MODULCTRL_def, SPI0_TX0_def, 
+write_CH0CONF_comb_def, write_CH0CONF_init_def] >>
+`7w:word5 >+ 2w:word5` by EVAL_TAC >>
+fs [ref_rel_def, IS_STATE_REL_def]);
 
 (* dr.state = dr_init_check_rep and spi.state = init_setregs, last_read_v = 1w *)
-val n_tau_tr_dr_init_check_rep_5 = store_thm("n_tau_tr_dr_init_check_rep_5",
+val n_tau_tr_dr_init_check_rep_3 = store_thm("n_tau_tr_dr_init_check_rep_3",
 ``!dr spi v. 
 dr.state = dr_init_check_rep /\ spi.state = init_setregs /\
 ~ dr.dr_init.issue_wr_sysconfig /\ ~ dr.dr_init.issue_wr_modulctrl /\ 
-~ dr.dr_init.issue_wr_ch0conf_wl /\ ~ dr.dr_init.issue_wr_ch0conf_speed /\ 
-~ dr.dr_init.issue_wr_ch0conf_mode /\ ~ spi.init.sysconfig_mode_done /\
-~ spi.init.ch0conf_wordlen_done /\ ~ spi.init.ch0conf_mode_done /\ 
-~ spi.init.ch0conf_speed_done /\ ~ spi.init.modulctrl_bus_done /\
+~ spi.init.sysconfig_mode_done /\ ~ spi.init.modulctrl_bus_done /\
 dr.dr_last_read_ad = SOME SPI0_SYSSTATUS /\ dr.dr_last_read_v = SOME v /\
-(0 >< 0) v:word1 = 1w ==>
-n_tau_tr 5 local_tr (dr,spi) tau 
+(0 >< 0) v:word1 = 1w /\ spi.regs.CH0CONF.WL = 0w /\ 
+spi.regs.CH0CONF.IS = 1w /\ spi.regs.CH0CONF.FORCE = 0w ==>
+n_tau_tr 3 local_tr (dr,spi) tau 
 (dr with <| state := dr_ready; 
 dr_init := 
-<| issue_wr_sysconfig := T; issue_wr_modulctrl := T; 
-issue_wr_ch0conf_wl := T; issue_wr_ch0conf_mode := T; 
-issue_wr_ch0conf_speed := T |> |>, 
+<|issue_wr_sysconfig := T; issue_wr_modulctrl := T|> |>, 
 spi with <|state := spi_ready;
 regs := spi.regs with 
 <| SYSCONFIG := spi.regs.SYSCONFIG with <|SIDLEMODE := 2w; AUTOIDLE := 1w|>;
@@ -292,30 +167,25 @@ MODULCTRL := <|SYSTEM_TEST := 0w; MS := 0w; SINGLE := 1w|>;
 CH0CONF := spi.regs.CH0CONF with
 <|PHA := 0w; POL := 0w; CLKD := 6w; EPOL := 1w; WL := 7w; 
 TRM := 0w; DPE0 := 1w; DPE1 := 0w; IS := 0w|> |>;
-init :=
-<|sysconfig_mode_done := T; modulctrl_bus_done := T; 
-ch0conf_wordlen_done :=  T; ch0conf_mode_done := T; 
-ch0conf_speed_done := T|> |>)``,
+init := <|sysconfig_mode_done := T; modulctrl_bus_done := T|> |>)``,
 rw [n_tau_tr_def, n_tau_tr_SUC, local_tr_cases, driver_tr_cases, spi_tr_cases, 
 DR_TAU_ENABLE_def, SPI_TAU_ENABLE_def, DR_WR_ENABLE_def, DR_RD_ENABLE_def] >>
-`dr_check dr SPI0_SYSSTATUS v = dr with state := dr_init_setting` by rw [dr_check_def, dr_check_sysstatus_def] >>
-rw [] >>
+`dr_check dr SPI0_SYSSTATUS v = dr with state := dr_init_setting` 
+by rw [dr_check_def, dr_check_sysstatus_def] >> rw [] >>
 `(dr_write_state (dr with state := dr_init_setting) = 
 dr with <| state := dr_init_setting;
 dr_init := dr.dr_init with issue_wr_sysconfig := T |>) /\
 (dr_write_address (dr with state := dr_init_setting) = SOME SPI0_SYSCONFIG) /\
 (dr_write_value (dr with state := dr_init_setting) = SOME (0x00000011w:word32))` 
 by rw [dr_write_state_def, dr_write_address_def, dr_write_value_def,
-dr_write_def, dr_write_sysconfig_def] >>
-rw [] >>
+dr_write_def, dr_write_sysconfig_def] >> rw [] >>
 `write_SPI_regs SPI0_SYSCONFIG 17w spi = 
 (spi with <|state := init_setregs; 
 regs := spi.regs with 
 SYSCONFIG := spi.regs.SYSCONFIG with <|SIDLEMODE := 2w; AUTOIDLE := 1w|>; 
 init := spi.init with sysconfig_mode_done := T |>)`
 by rw [write_SPI_regs_def, SPI0_PA_RANGE_def, SPI0_START_def, SPI0_END_def, 
-SPI0_SYSCONFIG_def, write_SYSCONFIG_comb_def, write_SYSCONFIG_def] >>
-rw [] >>
+SPI0_SYSCONFIG_def, write_SYSCONFIG_comb_def, write_SYSCONFIG_def] >> rw [] >>
 `(dr_write_state (dr with <|state := dr_init_setting;
 dr_init := dr.dr_init with issue_wr_sysconfig := T |>) = 
 dr with <|state := dr_init_setting;
@@ -326,8 +196,8 @@ dr_init := dr.dr_init with issue_wr_sysconfig := T |>) = SOME SPI0_MODULCTRL) /\
 (dr_write_value (dr with <| state := dr_init_setting;
 dr_init := dr.dr_init with issue_wr_sysconfig := T |>) = SOME (0x00000001w))` 
 by fs [dr_write_state_def, dr_write_address_def, dr_write_value_def,
-dr_write_def, dr_write_modulctrl_def] >>
-rw [] >>
+dr_write_def, dr_write_modulctrl_def] >> rw [] >>
+`~(0w:word5 >+ 2w:word5)` by EVAL_TAC >>
 `write_SPI_regs SPI0_MODULCTRL 1w 
 (spi with <|state := init_setregs; regs := spi.regs with 
 SYSCONFIG := spi.regs.SYSCONFIG with <|SIDLEMODE := 2w; AUTOIDLE := 1w|>; 
@@ -337,715 +207,490 @@ init := spi.init with sysconfig_mode_done := T |>) =
 MODULCTRL := <|SYSTEM_TEST := 0w; MS := 0w; SINGLE := 1w|> |>;
 init := spi.init with <|sysconfig_mode_done := T; modulctrl_bus_done := T |> |>)`
 by rw [write_SPI_regs_def, SPI0_PA_RANGE_def, SPI0_START_def, SPI0_END_def, 
-SPI0_SYSCONFIG_def, SPI0_MODULCTRL_def, write_MODULCTRL_def] >>
-rw [] >>
+SPI0_SYSCONFIG_def, SPI0_MODULCTRL_def, write_MODULCTRL_def] >> fs [] >>
 `(dr_write_state (dr with <|state := dr_init_setting;
 dr_init := dr.dr_init with <|issue_wr_sysconfig := T; issue_wr_modulctrl := T|> |>) = 
-dr with <|state := dr_init_setting;
+dr with <|state := dr_ready;
 dr_init := dr.dr_init with 
-<|issue_wr_sysconfig := T; issue_wr_modulctrl := T; issue_wr_ch0conf_wl := T |> |>) /\
+<|issue_wr_sysconfig := T; issue_wr_modulctrl := T|> |>) /\
 (dr_write_address (dr with <|state := dr_init_setting;
 dr_init := dr.dr_init with <|issue_wr_sysconfig := T; issue_wr_modulctrl := T|> |>) = 
 SOME SPI0_CH0CONF) /\
 (dr_write_value (dr with <|state := dr_init_setting;
 dr_init := dr.dr_init with <|issue_wr_sysconfig := T; issue_wr_modulctrl := T|> |>) = 
-SOME (0x00000380w:word32))` 
+SOME (66520w:word32))` 
 by fs [dr_write_state_def, dr_write_address_def, dr_write_value_def,
-dr_write_def, dr_write_ch0conf_wl_def] >>
-rw [] >>
-`7w:word5 >+ 2w:word5` by EVAL_TAC >>
-`write_SPI_regs SPI0_CH0CONF 896w 
-(spi with <|state := init_setregs; 
-regs := spi.regs with 
-<| SYSCONFIG := spi.regs.SYSCONFIG with <|SIDLEMODE := 2w; AUTOIDLE := 1w|>;
+dr_write_def, dr_write_ch0conf_init_def] >> fs [] >>
+`(19 >< 19) (66520w:word32):word1 <> spi.regs.CH0CONF.IS` 
+by FULL_SIMP_TAC (std_ss++WORD_ss) [] >>
+`ch0conf_changed (66520w:word32) 
+(spi with <|state := init_setregs;
+regs:= spi.regs with <|SYSCONFIG := spi.regs.SYSCONFIG with 
+<|SIDLEMODE := 2w; AUTOIDLE := 1w|>;
 MODULCTRL := <|SYSTEM_TEST := 0w; MS := 0w; SINGLE := 1w|> |>;
-init := spi.init with 
-<|sysconfig_mode_done := T; modulctrl_bus_done := T|> |>) = 
-(spi with <|state := init_setregs; 
-regs := spi.regs with <|
-SYSCONFIG := spi.regs.SYSCONFIG with <|SIDLEMODE := 2w; AUTOIDLE := 1w|>;
-MODULCTRL := <|SYSTEM_TEST := 0w; MS := 0w; SINGLE := 1w|>;
-CH0CONF := spi.regs.CH0CONF with WL := 7w |>;
-init := spi.init with 
-<|ch0conf_wordlen_done := T; sysconfig_mode_done := T; modulctrl_bus_done := T |> |>)`
-by fs [write_SPI_regs_def, SPI0_CH0CONF_def, SPI0_PA_RANGE_def, 
-SPI0_START_def, SPI0_END_def, SPI0_SYSCONFIG_def, SPI0_MODULCTRL_def, 
-SPI0_TX0_def, write_CH0CONF_comb_def, write_CH0CONF_WL_def] >>
-rw [] >>
-rw [dr_write_state_def, dr_write_address_def, dr_write_value_def,
-dr_write_def, dr_write_ch0conf_speed_def, dr_write_ch0conf_mode_def] >>
-fs [write_SPI_regs_def, SPI0_CH0CONF_def, SPI0_PA_RANGE_def, 
-SPI0_START_def, SPI0_END_def, SPI0_SYSCONFIG_def, 
-SPI0_MODULCTRL_def, SPI0_TX0_def, write_CH0CONF_comb_def, 
-write_CH0CONF_def, write_CH0CONF_speed_def]);
+init := <|sysconfig_mode_done := T; modulctrl_bus_done := T|> |>)` by fs [ch0conf_changed_def] >>
+rw [write_SPI_regs_def, SPI0_CH0CONF_def, SPI0_PA_RANGE_def, SPI0_START_def, 
+SPI0_END_def, SPI0_SYSCONFIG_def, SPI0_MODULCTRL_def, SPI0_TX0_def, 
+write_CH0CONF_comb_def, write_CH0CONF_init_def] >>
+`7w:word5 >+ 2w:word5` by EVAL_TAC >>
+fs [ref_rel_def, IS_STATE_REL_def]);
 
 (* dr.state = dr_init_read_req and spi.state = init_setregs *)
-val n_tau_tr_dr_init_read_req_6 = store_thm("n_tau_tr_dr_init_read_req_6",
+val n_tau_tr_dr_init_read_req_4 = store_thm("n_tau_tr_dr_init_read_req_4",
 ``!dr spi. 
 dr.state = dr_init_read_req /\ spi.state = init_setregs /\
 ~ dr.dr_init.issue_wr_sysconfig /\ ~ dr.dr_init.issue_wr_modulctrl /\ 
-~ dr.dr_init.issue_wr_ch0conf_wl /\ ~ dr.dr_init.issue_wr_ch0conf_speed /\ 
-~ dr.dr_init.issue_wr_ch0conf_mode /\ ~ spi.init.sysconfig_mode_done /\
-~ spi.init.ch0conf_wordlen_done /\ ~ spi.init.ch0conf_mode_done /\ 
-~ spi.init.ch0conf_speed_done /\ ~ spi.init.modulctrl_bus_done /\
-spi.regs.SYSSTATUS = 1w  ==>
+~ spi.init.sysconfig_mode_done /\ ~ spi.init.modulctrl_bus_done /\
+spi.regs.SYSSTATUS = 1w /\ spi.regs.CH0CONF.WL = 0w /\ 
+spi.regs.CH0CONF.IS = 1w /\ spi.regs.CH0CONF.FORCE = 0w  ==>
+n_tau_tr 4 local_tr (dr,spi) tau 
+(dr with <| state := dr_ready; 
+dr_last_read_ad := SOME SPI0_SYSSTATUS;
+dr_last_read_v := SOME 1w;
+dr_init := <| issue_wr_sysconfig := T; issue_wr_modulctrl := T|> |>, 
+spi with <|state := spi_ready;
+regs := spi.regs with 
+<| SYSCONFIG := spi.regs.SYSCONFIG with <|SIDLEMODE := 2w; AUTOIDLE := 1w|>;
+MODULCTRL := <|SYSTEM_TEST := 0w; MS := 0w; SINGLE := 1w|>;
+CH0CONF := spi.regs.CH0CONF with
+<|PHA := 0w; POL := 0w; CLKD := 6w; EPOL := 1w; WL := 7w; 
+TRM := 0w; DPE0 := 1w; DPE1 := 0w; IS := 0w|> |>;
+init := <|sysconfig_mode_done := T; modulctrl_bus_done := T|> |>)``, 
+rw [n_tau_tr_def, n_tau_tr_SUC, local_tr_cases, driver_tr_cases, spi_tr_cases, 
+DR_TAU_ENABLE_def, SPI_TAU_ENABLE_def, DR_WR_ENABLE_def, DR_RD_ENABLE_def] >>
+`dr_read dr = dr with <| state := dr_init_check_rep;
+dr_last_read_ad := SOME SPI0_SYSSTATUS |>` by rw [dr_read_def, dr_read_sysstatus_def] >> rw [] >>
+`read_SPI_regs_state SPI0_SYSSTATUS spi = spi /\
+read_SPI_regs_value SPI0_SYSSTATUS spi = w2w spi.regs.SYSSTATUS` by
+rw [read_SPI_regs_state_def, read_SPI_regs_value_def, read_SPI_regs_def, SPI0_SYSSTATUS_def,
+SPI0_PA_RANGE_def, SPI0_START_def, SPI0_END_def, SPI0_SYSCONFIG_def] >> rw [] >>
+`dr_check (dr with <|state := dr_init_check_rep; 
+dr_last_read_ad := SOME SPI0_SYSSTATUS;
+dr_last_read_v := SOME 1w|>) SPI0_SYSSTATUS 1w =
+dr with <|state := dr_init_setting; dr_last_read_ad := SOME SPI0_SYSSTATUS;
+dr_last_read_v := SOME 1w|>` by rw [dr_check_def, dr_check_sysstatus_def] >> rw [] >>
+`(dr_write_state (dr with <|state := dr_init_setting; 
+dr_last_read_ad := SOME SPI0_SYSSTATUS;
+dr_last_read_v := SOME 1w|>) = dr with <| state := dr_init_setting;
+dr_last_read_ad := SOME SPI0_SYSSTATUS;
+dr_last_read_v := SOME 1w;
+dr_init := dr.dr_init with issue_wr_sysconfig := T |>) /\
+(dr_write_address (dr with <|state := dr_init_setting; 
+dr_last_read_ad := SOME SPI0_SYSSTATUS;
+dr_last_read_v := SOME 1w|>) = SOME SPI0_SYSCONFIG) /\
+(dr_write_value (dr with <|state := dr_init_setting; 
+dr_last_read_ad := SOME SPI0_SYSSTATUS;
+dr_last_read_v := SOME 1w|>) = SOME (0x00000011w:word32))` 
+by rw [dr_write_state_def, dr_write_address_def, dr_write_value_def,
+dr_write_def, dr_write_sysconfig_def] >> rw [] >>
+`write_SPI_regs SPI0_SYSCONFIG 17w spi = 
+(spi with <|state := init_setregs; 
+regs := spi.regs with 
+SYSCONFIG := spi.regs.SYSCONFIG with <|SIDLEMODE := 2w; AUTOIDLE := 1w|>; 
+init := spi.init with sysconfig_mode_done := T |>)`
+by rw [write_SPI_regs_def, SPI0_PA_RANGE_def, SPI0_START_def, SPI0_END_def, 
+SPI0_SYSCONFIG_def, write_SYSCONFIG_comb_def, write_SYSCONFIG_def] >> rw [] >>
+`(dr_write_state (dr with <|state := dr_init_setting;
+dr_last_read_ad := SOME SPI0_SYSSTATUS;
+dr_last_read_v := SOME 1w;
+dr_init := dr.dr_init with issue_wr_sysconfig := T |>) = 
+dr with <|state := dr_init_setting;
+dr_last_read_ad := SOME SPI0_SYSSTATUS;
+dr_last_read_v := SOME 1w;
+dr_init := dr.dr_init with 
+<|issue_wr_sysconfig := T ; issue_wr_modulctrl := T |> |>) /\
+(dr_write_address (dr with <| state := dr_init_setting;
+dr_last_read_ad := SOME SPI0_SYSSTATUS;
+dr_last_read_v := SOME 1w;
+dr_init := dr.dr_init with issue_wr_sysconfig := T |>) = SOME SPI0_MODULCTRL) /\
+(dr_write_value (dr with <| state := dr_init_setting;
+dr_last_read_ad := SOME SPI0_SYSSTATUS;
+dr_last_read_v := SOME 1w;
+dr_init := dr.dr_init with issue_wr_sysconfig := T |>) = SOME (0x00000001w))` 
+by fs [dr_write_state_def, dr_write_address_def, dr_write_value_def,
+dr_write_def, dr_write_modulctrl_def] >> rw [] >>
+`~(0w:word5 >+ 2w:word5)` by EVAL_TAC >>
+`write_SPI_regs SPI0_MODULCTRL 1w 
+(spi with <|state := init_setregs; regs := spi.regs with 
+SYSCONFIG := spi.regs.SYSCONFIG with <|SIDLEMODE := 2w; AUTOIDLE := 1w|>; 
+init := spi.init with sysconfig_mode_done := T |>) =
+(spi with <|state := init_setregs; regs := spi.regs with
+<|SYSCONFIG := spi.regs.SYSCONFIG with <|SIDLEMODE := 2w; AUTOIDLE := 1w|>;
+MODULCTRL := <|SYSTEM_TEST := 0w; MS := 0w; SINGLE := 1w|> |>;
+init := spi.init with <|sysconfig_mode_done := T; modulctrl_bus_done := T |> |>)`
+by rw [write_SPI_regs_def, SPI0_PA_RANGE_def, SPI0_START_def, SPI0_END_def, 
+SPI0_SYSCONFIG_def, SPI0_MODULCTRL_def, write_MODULCTRL_def] >> fs [] >>
+`(dr_write_state (dr with <|state := dr_init_setting;
+dr_last_read_ad := SOME SPI0_SYSSTATUS;
+dr_last_read_v := SOME 1w;
+dr_init := dr.dr_init with <|issue_wr_sysconfig := T; issue_wr_modulctrl := T|> |>) = 
+dr with <|state := dr_ready;
+dr_last_read_ad := SOME SPI0_SYSSTATUS;
+dr_last_read_v := SOME 1w;
+dr_init := dr.dr_init with 
+<|issue_wr_sysconfig := T; issue_wr_modulctrl := T|> |>) /\
+(dr_write_address (dr with <|state := dr_init_setting;
+dr_last_read_ad := SOME SPI0_SYSSTATUS;
+dr_last_read_v := SOME 1w;
+dr_init := dr.dr_init with <|issue_wr_sysconfig := T; issue_wr_modulctrl := T|> |>) = 
+SOME SPI0_CH0CONF) /\
+(dr_write_value (dr with <|state := dr_init_setting;
+dr_last_read_ad := SOME SPI0_SYSSTATUS;
+dr_last_read_v := SOME 1w;
+dr_init := dr.dr_init with <|issue_wr_sysconfig := T; issue_wr_modulctrl := T|> |>) = 
+SOME (66520w:word32))` 
+by fs [dr_write_state_def, dr_write_address_def, dr_write_value_def,
+dr_write_def, dr_write_ch0conf_init_def] >> fs [] >>
+`(19 >< 19) (66520w:word32):word1 <> spi.regs.CH0CONF.IS` 
+by FULL_SIMP_TAC (std_ss++WORD_ss) [] >>
+`ch0conf_changed (66520w:word32) 
+(spi with <|state := init_setregs;
+regs:= spi.regs with <|SYSCONFIG := spi.regs.SYSCONFIG with 
+<|SIDLEMODE := 2w; AUTOIDLE := 1w|>;
+MODULCTRL := <|SYSTEM_TEST := 0w; MS := 0w; SINGLE := 1w|> |>;
+init := <|sysconfig_mode_done := T; modulctrl_bus_done := T|> |>)` by fs [ch0conf_changed_def] >>
+rw [write_SPI_regs_def, SPI0_CH0CONF_def, SPI0_PA_RANGE_def, SPI0_START_def, 
+SPI0_END_def, SPI0_SYSCONFIG_def, SPI0_MODULCTRL_def, SPI0_TX0_def, 
+write_CH0CONF_comb_def, write_CH0CONF_init_def] >>
+`7w:word5 >+ 2w:word5` by EVAL_TAC >>
+fs [ref_rel_def, IS_STATE_REL_def]);
+
+(* dr.state = dr_init_check_rep and spi.state = init_setregs, last_read_v = 0w *)
+val n_tau_tr_dr_init_check_rep_5 = store_thm("n_tau_tr_dr_init_check_rep_5",
+``!dr spi v. 
+dr.state = dr_init_check_rep /\ spi.state = init_setregs /\
+~ dr.dr_init.issue_wr_sysconfig /\ ~ dr.dr_init.issue_wr_modulctrl /\ 
+~ spi.init.sysconfig_mode_done /\ ~ spi.init.modulctrl_bus_done /\
+spi.regs.SYSSTATUS = 1w /\ spi.regs.CH0CONF.WL = 0w /\ 
+spi.regs.CH0CONF.IS = 1w /\ spi.regs.CH0CONF.FORCE = 0w /\
+dr.dr_last_read_ad = SOME SPI0_SYSSTATUS /\ dr.dr_last_read_v = SOME v /\ 
+(0 >< 0) v:word1 = 0w ==>
+n_tau_tr 5 local_tr (dr,spi) tau 
+(dr with <| state := dr_ready; 
+dr_last_read_ad := SOME SPI0_SYSSTATUS;
+dr_last_read_v := SOME 1w;
+dr_init := <|issue_wr_sysconfig := T; issue_wr_modulctrl := T|> |>, 
+spi with <|state := spi_ready;
+regs := spi.regs with 
+<| SYSCONFIG := spi.regs.SYSCONFIG with <|SIDLEMODE := 2w; AUTOIDLE := 1w|>;
+MODULCTRL := <|SYSTEM_TEST := 0w; MS := 0w; SINGLE := 1w|>;
+CH0CONF := spi.regs.CH0CONF with
+<|PHA := 0w; POL := 0w; CLKD := 6w; EPOL := 1w; WL := 7w; 
+TRM := 0w; DPE0 := 1w; DPE1 := 0w; IS := 0w|> |>;
+init := <|sysconfig_mode_done := T; modulctrl_bus_done := T|> |>)``,
+rw [n_tau_tr_def, n_tau_tr_SUC, local_tr_cases, driver_tr_cases, spi_tr_cases, 
+DR_TAU_ENABLE_def, SPI_TAU_ENABLE_def, DR_WR_ENABLE_def, DR_RD_ENABLE_def] >>
+`dr_check dr SPI0_SYSSTATUS v = dr with state := dr_init_read_req` 
+by rw [dr_check_def, dr_check_sysstatus_def] >> rw [] >>
+`dr_read (dr with state := dr_init_read_req) = dr with <| state := dr_init_check_rep;
+dr_last_read_ad := SOME SPI0_SYSSTATUS |>` by rw [dr_read_def, dr_read_sysstatus_def] >> rw [] >>
+`read_SPI_regs_state SPI0_SYSSTATUS spi = spi /\
+read_SPI_regs_value SPI0_SYSSTATUS spi = w2w spi.regs.SYSSTATUS` by
+rw [read_SPI_regs_state_def, read_SPI_regs_value_def, read_SPI_regs_def, SPI0_SYSSTATUS_def,
+SPI0_PA_RANGE_def, SPI0_START_def, SPI0_END_def, SPI0_SYSCONFIG_def] >> rw [] >>
+`dr_check (dr with <|state := dr_init_check_rep; 
+dr_last_read_ad := SOME SPI0_SYSSTATUS;
+dr_last_read_v := SOME 1w|>) SPI0_SYSSTATUS 1w =
+dr with <|state := dr_init_setting; dr_last_read_ad := SOME SPI0_SYSSTATUS;
+dr_last_read_v := SOME 1w|>` by rw [dr_check_def, dr_check_sysstatus_def] >> rw [] >>
+`(dr_write_state (dr with <|state := dr_init_setting; 
+dr_last_read_ad := SOME SPI0_SYSSTATUS;
+dr_last_read_v := SOME 1w|>) = dr with <| state := dr_init_setting;
+dr_last_read_ad := SOME SPI0_SYSSTATUS;
+dr_last_read_v := SOME 1w;
+dr_init := dr.dr_init with issue_wr_sysconfig := T |>) /\
+(dr_write_address (dr with <|state := dr_init_setting; 
+dr_last_read_ad := SOME SPI0_SYSSTATUS;
+dr_last_read_v := SOME 1w|>) = SOME SPI0_SYSCONFIG) /\
+(dr_write_value (dr with <|state := dr_init_setting; 
+dr_last_read_ad := SOME SPI0_SYSSTATUS;
+dr_last_read_v := SOME 1w|>) = SOME (0x00000011w:word32))` 
+by rw [dr_write_state_def, dr_write_address_def, dr_write_value_def,
+dr_write_def, dr_write_sysconfig_def] >> rw [] >>
+`write_SPI_regs SPI0_SYSCONFIG 17w spi = 
+(spi with <|state := init_setregs; 
+regs := spi.regs with 
+SYSCONFIG := spi.regs.SYSCONFIG with <|SIDLEMODE := 2w; AUTOIDLE := 1w|>; 
+init := spi.init with sysconfig_mode_done := T |>)`
+by rw [write_SPI_regs_def, SPI0_PA_RANGE_def, SPI0_START_def, SPI0_END_def, 
+SPI0_SYSCONFIG_def, write_SYSCONFIG_comb_def, write_SYSCONFIG_def] >> rw [] >>
+`(dr_write_state (dr with <|state := dr_init_setting;
+dr_last_read_ad := SOME SPI0_SYSSTATUS;
+dr_last_read_v := SOME 1w;
+dr_init := dr.dr_init with issue_wr_sysconfig := T |>) = 
+dr with <|state := dr_init_setting;
+dr_last_read_ad := SOME SPI0_SYSSTATUS;
+dr_last_read_v := SOME 1w;
+dr_init := dr.dr_init with 
+<|issue_wr_sysconfig := T ; issue_wr_modulctrl := T |> |>) /\
+(dr_write_address (dr with <| state := dr_init_setting;
+dr_last_read_ad := SOME SPI0_SYSSTATUS;
+dr_last_read_v := SOME 1w;
+dr_init := dr.dr_init with issue_wr_sysconfig := T |>) = SOME SPI0_MODULCTRL) /\
+(dr_write_value (dr with <| state := dr_init_setting;
+dr_last_read_ad := SOME SPI0_SYSSTATUS;
+dr_last_read_v := SOME 1w;
+dr_init := dr.dr_init with issue_wr_sysconfig := T |>) = SOME (0x00000001w))` 
+by fs [dr_write_state_def, dr_write_address_def, dr_write_value_def,
+dr_write_def, dr_write_modulctrl_def] >> rw [] >>
+`~(0w:word5 >+ 2w:word5)` by EVAL_TAC >>
+`write_SPI_regs SPI0_MODULCTRL 1w 
+(spi with <|state := init_setregs; regs := spi.regs with 
+SYSCONFIG := spi.regs.SYSCONFIG with <|SIDLEMODE := 2w; AUTOIDLE := 1w|>; 
+init := spi.init with sysconfig_mode_done := T |>) =
+(spi with <|state := init_setregs; regs := spi.regs with
+<|SYSCONFIG := spi.regs.SYSCONFIG with <|SIDLEMODE := 2w; AUTOIDLE := 1w|>;
+MODULCTRL := <|SYSTEM_TEST := 0w; MS := 0w; SINGLE := 1w|> |>;
+init := spi.init with <|sysconfig_mode_done := T; modulctrl_bus_done := T |> |>)`
+by rw [write_SPI_regs_def, SPI0_PA_RANGE_def, SPI0_START_def, SPI0_END_def, 
+SPI0_SYSCONFIG_def, SPI0_MODULCTRL_def, write_MODULCTRL_def] >> fs [] >>
+`(dr_write_state (dr with <|state := dr_init_setting;
+dr_last_read_ad := SOME SPI0_SYSSTATUS;
+dr_last_read_v := SOME 1w;
+dr_init := dr.dr_init with <|issue_wr_sysconfig := T; issue_wr_modulctrl := T|> |>) = 
+dr with <|state := dr_ready;
+dr_last_read_ad := SOME SPI0_SYSSTATUS;
+dr_last_read_v := SOME 1w;
+dr_init := dr.dr_init with 
+<|issue_wr_sysconfig := T; issue_wr_modulctrl := T|> |>) /\
+(dr_write_address (dr with <|state := dr_init_setting;
+dr_last_read_ad := SOME SPI0_SYSSTATUS;
+dr_last_read_v := SOME 1w;
+dr_init := dr.dr_init with <|issue_wr_sysconfig := T; issue_wr_modulctrl := T|> |>) = 
+SOME SPI0_CH0CONF) /\
+(dr_write_value (dr with <|state := dr_init_setting;
+dr_last_read_ad := SOME SPI0_SYSSTATUS;
+dr_last_read_v := SOME 1w;
+dr_init := dr.dr_init with <|issue_wr_sysconfig := T; issue_wr_modulctrl := T|> |>) = 
+SOME (66520w:word32))` 
+by fs [dr_write_state_def, dr_write_address_def, dr_write_value_def,
+dr_write_def, dr_write_ch0conf_init_def] >> fs [] >>
+`(19 >< 19) (66520w:word32):word1 <> spi.regs.CH0CONF.IS` 
+by FULL_SIMP_TAC (std_ss++WORD_ss) [] >>
+`ch0conf_changed (66520w:word32) 
+(spi with <|state := init_setregs;
+regs:= spi.regs with <|SYSCONFIG := spi.regs.SYSCONFIG with 
+<|SIDLEMODE := 2w; AUTOIDLE := 1w|>;
+MODULCTRL := <|SYSTEM_TEST := 0w; MS := 0w; SINGLE := 1w|> |>;
+init := <|sysconfig_mode_done := T; modulctrl_bus_done := T|> |>)` by fs [ch0conf_changed_def] >>
+rw [write_SPI_regs_def, SPI0_CH0CONF_def, SPI0_PA_RANGE_def, SPI0_START_def, 
+SPI0_END_def, SPI0_SYSCONFIG_def, SPI0_MODULCTRL_def, SPI0_TX0_def, 
+write_CH0CONF_comb_def, write_CH0CONF_init_def] >>
+`7w:word5 >+ 2w:word5` by EVAL_TAC >>
+fs [ref_rel_def, IS_STATE_REL_def]);
+
+(* dr.state = dr_init_read_req and spi.state = init_reset *)
+val n_tau_tr_dr_init_read_req_5 = store_thm("n_tau_tr_dr_init_read_req_5",
+``!dr spi. 
+dr.state = dr_init_read_req /\ spi.state = init_reset /\
+~ dr.dr_init.issue_wr_sysconfig /\ ~ dr.dr_init.issue_wr_modulctrl /\ 
+~ spi.init.sysconfig_mode_done /\ ~ spi.init.modulctrl_bus_done ==>
+n_tau_tr 5 local_tr (dr,spi) tau 
+(dr with <| state := dr_ready; 
+dr_last_read_ad := SOME SPI0_SYSSTATUS;
+dr_last_read_v := SOME 1w;
+dr_init := <|issue_wr_sysconfig := T; issue_wr_modulctrl := T|> |>, 
+spi with <|state := spi_ready;
+regs := spi.regs with 
+<| SYSCONFIG := spi.regs.SYSCONFIG with <|SIDLEMODE := 2w; AUTOIDLE := 1w|>;
+SYSSTATUS := 1w;
+MODULCTRL := <|SYSTEM_TEST := 0w; MS := 0w; SINGLE := 1w|>;
+CH0CONF := 
+<|PHA := 0w; POL := 0w; CLKD := 6w; EPOL := 1w; WL := 7w; 
+TRM := 0w; DPE0 := 1w; DPE1 := 0w; IS := 0w; FORCE := 0w|> |>;
+init := <|sysconfig_mode_done := T; modulctrl_bus_done := T|> |>)``, 
+rw [n_tau_tr_def, n_tau_tr_SUC, local_tr_cases, driver_tr_cases, spi_tr_cases, 
+DR_TAU_ENABLE_def, SPI_TAU_ENABLE_def, DR_WR_ENABLE_def, DR_RD_ENABLE_def, GSYM LEFT_EXISTS_AND_THM] >>
+Q.EXISTS_TAC `(dr,spi_tau_operations spi)` >> rw [] >>
+`spi_tau_operations spi = spi with <|regs := spi.regs with <|SYSSTATUS := 1w;
+CH0CONF := <|PHA := 0w; POL := 0w; CLKD := 0w; EPOL := 0w; WL := 0w;
+TRM := 0w; DPE0 := 0w; DPE1 := 1w; IS := 1w; FORCE := 0w|> |>;
+state := init_setregs |>` by rw [spi_tau_operations_def, init_reset_op_def] >> rw [] >>
+`dr_read dr = dr with <| state := dr_init_check_rep;
+dr_last_read_ad := SOME SPI0_SYSSTATUS |>` by rw [dr_read_def, dr_read_sysstatus_def] >> rw [] >>
+`(read_SPI_regs_state SPI0_SYSSTATUS (spi with <|state := init_setregs;
+regs := spi.regs with <|SYSSTATUS := 1w;
+CH0CONF := <|PHA := 0w; POL := 0w; CLKD := 0w; EPOL := 0w; WL := 0w;
+TRM := 0w; DPE0 := 0w; DPE1 := 1w; IS := 1w; FORCE := 0w|> |> |>) = 
+(spi with <|state := init_setregs;
+regs := spi.regs with <|SYSSTATUS := 1w;
+CH0CONF := <|PHA := 0w; POL := 0w; CLKD := 0w; EPOL := 0w; WL := 0w;
+TRM := 0w; DPE0 := 0w; DPE1 := 1w; IS := 1w; FORCE := 0w|> |> |>)) /\
+(read_SPI_regs_value SPI0_SYSSTATUS (spi with <|state := init_setregs;
+regs := spi.regs with <|SYSSTATUS := 1w;
+CH0CONF := <|PHA := 0w; POL := 0w; CLKD := 0w; EPOL := 0w; WL := 0w;
+TRM := 0w; DPE0 := 0w; DPE1 := 1w; IS := 1w; FORCE := 0w|> |> |>) = 1w:word32)` 
+by rw [read_SPI_regs_state_def, read_SPI_regs_value_def, read_SPI_regs_def, SPI0_SYSSTATUS_def,
+SPI0_PA_RANGE_def, SPI0_START_def, SPI0_END_def, SPI0_SYSCONFIG_def] >> rw [] >>
+`dr_check (dr with <|state := dr_init_check_rep; 
+dr_last_read_ad := SOME SPI0_SYSSTATUS;
+dr_last_read_v := SOME 1w|>) SPI0_SYSSTATUS 1w =
+dr with <|state := dr_init_setting; dr_last_read_ad := SOME SPI0_SYSSTATUS;
+dr_last_read_v := SOME 1w|>` by rw [dr_check_def, dr_check_sysstatus_def] >> rw [] >>
+`(dr_write_state (dr with <|state := dr_init_setting; 
+dr_last_read_ad := SOME SPI0_SYSSTATUS;
+dr_last_read_v := SOME 1w|>) = dr with <| state := dr_init_setting;
+dr_last_read_ad := SOME SPI0_SYSSTATUS;
+dr_last_read_v := SOME 1w;
+dr_init := dr.dr_init with issue_wr_sysconfig := T |>) /\
+(dr_write_address (dr with <|state := dr_init_setting; 
+dr_last_read_ad := SOME SPI0_SYSSTATUS;
+dr_last_read_v := SOME 1w|>) = SOME SPI0_SYSCONFIG) /\
+(dr_write_value (dr with <|state := dr_init_setting; 
+dr_last_read_ad := SOME SPI0_SYSSTATUS;
+dr_last_read_v := SOME 1w|>) = SOME (0x00000011w:word32))` 
+by rw [dr_write_state_def, dr_write_address_def, dr_write_value_def,
+dr_write_def, dr_write_sysconfig_def] >> rw [] >>
+`write_SPI_regs SPI0_SYSCONFIG 17w (spi with <|state := init_setregs;
+regs := spi.regs with <|SYSSTATUS := 1w;
+CH0CONF := <|PHA := 0w; POL := 0w; CLKD := 0w; EPOL := 0w; WL := 0w;
+TRM := 0w; DPE0 := 0w; DPE1 := 1w; IS := 1w; FORCE := 0w|> |> |>) = 
+(spi with <|state := init_setregs; 
+regs := spi.regs with  <|SYSSTATUS := 1w;
+CH0CONF := <|PHA := 0w; POL := 0w; CLKD := 0w; EPOL := 0w; WL := 0w;
+TRM := 0w; DPE0 := 0w; DPE1 := 1w; IS := 1w; FORCE := 0w|>;
+SYSCONFIG := spi.regs.SYSCONFIG with <|SIDLEMODE := 2w; AUTOIDLE := 1w|> |>; 
+init := spi.init with sysconfig_mode_done := T |>)`
+by rw [write_SPI_regs_def, SPI0_PA_RANGE_def, SPI0_START_def, SPI0_END_def, 
+SPI0_SYSCONFIG_def, write_SYSCONFIG_comb_def, write_SYSCONFIG_def] >> rw [] >>
+`(dr_write_state (dr with <|state := dr_init_setting;
+dr_last_read_ad := SOME SPI0_SYSSTATUS;
+dr_last_read_v := SOME 1w;
+dr_init := dr.dr_init with issue_wr_sysconfig := T |>) = 
+dr with <|state := dr_init_setting;
+dr_last_read_ad := SOME SPI0_SYSSTATUS;
+dr_last_read_v := SOME 1w;
+dr_init := dr.dr_init with 
+<|issue_wr_sysconfig := T ; issue_wr_modulctrl := T |> |>) /\
+(dr_write_address (dr with <| state := dr_init_setting;
+dr_last_read_ad := SOME SPI0_SYSSTATUS;
+dr_last_read_v := SOME 1w;
+dr_init := dr.dr_init with issue_wr_sysconfig := T |>) = SOME SPI0_MODULCTRL) /\
+(dr_write_value (dr with <| state := dr_init_setting;
+dr_last_read_ad := SOME SPI0_SYSSTATUS;
+dr_last_read_v := SOME 1w;
+dr_init := dr.dr_init with issue_wr_sysconfig := T |>) = SOME (0x00000001w))` 
+by fs [dr_write_state_def, dr_write_address_def, dr_write_value_def,
+dr_write_def, dr_write_modulctrl_def] >> rw [] >>
+`~(0w:word5 >+ 2w:word5)` by EVAL_TAC >>
+`write_SPI_regs SPI0_MODULCTRL 1w 
+(spi with <|state := init_setregs; 
+regs := spi.regs with 
+<|SYSCONFIG := spi.regs.SYSCONFIG with <|SIDLEMODE := 2w; AUTOIDLE := 1w|>;
+SYSSTATUS := 1w;
+CH0CONF := <|PHA := 0w; POL := 0w; CLKD := 0w; EPOL := 0w; WL := 0w; 
+TRM := 0w; DPE0 := 0w; DPE1 := 1w; IS := 1w; FORCE := 0w|> |>; 
+init := spi.init with sysconfig_mode_done := T |>) =
+(spi with <|state := init_setregs; regs := spi.regs with
+<|SYSCONFIG := spi.regs.SYSCONFIG with <|SIDLEMODE := 2w; AUTOIDLE := 1w|>;
+SYSSTATUS := 1w;
+MODULCTRL := <|SYSTEM_TEST := 0w; MS := 0w; SINGLE := 1w|>;
+CH0CONF := <|PHA := 0w; POL := 0w; CLKD := 0w; EPOL := 0w; WL := 0w; 
+TRM := 0w; DPE0 := 0w; DPE1 := 1w; IS := 1w; FORCE := 0w|> |>;
+init := <|sysconfig_mode_done := T; modulctrl_bus_done := T|> |>)`
+by rw [write_SPI_regs_def, SPI0_PA_RANGE_def, SPI0_START_def, SPI0_END_def, 
+SPI0_SYSCONFIG_def, SPI0_MODULCTRL_def, write_MODULCTRL_def] >> fs [] >>
+`(dr_write_state (dr with <|state := dr_init_setting;
+dr_last_read_ad := SOME SPI0_SYSSTATUS;
+dr_last_read_v := SOME 1w;
+dr_init := dr.dr_init with <|issue_wr_sysconfig := T; issue_wr_modulctrl := T|> |>) = 
+dr with <|state := dr_ready;
+dr_last_read_ad := SOME SPI0_SYSSTATUS;
+dr_last_read_v := SOME 1w;
+dr_init := <|issue_wr_sysconfig := T; issue_wr_modulctrl := T|> |>) /\
+(dr_write_address (dr with <|state := dr_init_setting;
+dr_last_read_ad := SOME SPI0_SYSSTATUS;
+dr_last_read_v := SOME 1w;
+dr_init := dr.dr_init with <|issue_wr_sysconfig := T; issue_wr_modulctrl := T|> |>) = 
+SOME SPI0_CH0CONF) /\
+(dr_write_value (dr with <|state := dr_init_setting;
+dr_last_read_ad := SOME SPI0_SYSSTATUS;
+dr_last_read_v := SOME 1w;
+dr_init := dr.dr_init with <|issue_wr_sysconfig := T; issue_wr_modulctrl := T|> |>) = 
+SOME (66520w:word32))` 
+by fs [dr_write_state_def, dr_write_address_def, dr_write_value_def,
+dr_write_def, dr_write_ch0conf_init_def] >> fs [] >>
+`(spi with <|state := init_setregs;
+regs := spi.regs with <|SYSCONFIG := spi.regs.SYSCONFIG with
+<|SIDLEMODE := 2w; AUTOIDLE := 1w|>; SYSSTATUS := 1w;
+MODULCTRL := <|SYSTEM_TEST := 0w; MS := 0w; SINGLE := 1w|>;
+CH0CONF := <|PHA := 0w; POL := 0w; CLKD := 0w; EPOL := 0w; WL := 0w;
+TRM := 0w; DPE0 := 0w; DPE1 := 1w; IS := 1w; FORCE := 0w|> |>;
+init := <|sysconfig_mode_done := T; modulctrl_bus_done := T|> |>).regs.CH0CONF.IS = 1w` by fs [] >>
+`(19 >< 19) (66520w:word32):word1 <> ((spi with <|state := init_setregs;
+regs := spi.regs with <|SYSCONFIG := spi.regs.SYSCONFIG with
+<|SIDLEMODE := 2w; AUTOIDLE := 1w|>; SYSSTATUS := 1w;
+MODULCTRL := <|SYSTEM_TEST := 0w; MS := 0w; SINGLE := 1w|>;
+CH0CONF := <|PHA := 0w; POL := 0w; CLKD := 0w; EPOL := 0w; WL := 0w;
+TRM := 0w; DPE0 := 0w; DPE1 := 1w; IS := 1w; FORCE := 0w|> |>;
+init := <|sysconfig_mode_done := T; modulctrl_bus_done := T|> |>).regs.CH0CONF.IS)` 
+by FULL_SIMP_TAC (std_ss++WORD_ss) [] >>
+`ch0conf_changed (66520w:word32) 
+(spi with <|state := init_setregs;
+regs := spi.regs with <|SYSCONFIG := spi.regs.SYSCONFIG with
+<|SIDLEMODE := 2w; AUTOIDLE := 1w|>; SYSSTATUS := 1w;
+MODULCTRL := <|SYSTEM_TEST := 0w; MS := 0w; SINGLE := 1w|>;
+CH0CONF := <|PHA := 0w; POL := 0w; CLKD := 0w; EPOL := 0w; WL := 0w;
+TRM := 0w; DPE0 := 0w; DPE1 := 1w; IS := 1w; FORCE := 0w|> |>;
+init := <|sysconfig_mode_done := T; modulctrl_bus_done := T|> |>)` by fs [ch0conf_changed_def] >>
+rw [write_SPI_regs_def, SPI0_CH0CONF_def, SPI0_PA_RANGE_def, SPI0_START_def, 
+SPI0_END_def, SPI0_SYSCONFIG_def, SPI0_MODULCTRL_def, SPI0_TX0_def, 
+write_CH0CONF_comb_def, write_CH0CONF_init_def] >>
+`7w:word5 >+ 2w:word5` by EVAL_TAC >>
+fs [ref_rel_def, IS_STATE_REL_def]);
+
+(* dr.state = dr_init_check_rep and spi.state = init_reset *)
+val n_tau_tr_dr_init_check_rep_6 = store_thm("n_tau_tr_dr_init_check_rep_6",
+``!dr spi v. 
+dr.state = dr_init_check_rep /\ spi.state = init_reset /\
+~ dr.dr_init.issue_wr_sysconfig /\ ~ dr.dr_init.issue_wr_modulctrl /\ 
+~ spi.init.sysconfig_mode_done /\ ~ spi.init.modulctrl_bus_done /\
+dr.dr_last_read_ad = SOME SPI0_SYSSTATUS /\ dr.dr_last_read_v = SOME v /\
+(0 >< 0) v:word1 = 0w ==>
 n_tau_tr 6 local_tr (dr,spi) tau 
 (dr with <| state := dr_ready; 
 dr_last_read_ad := SOME SPI0_SYSSTATUS;
 dr_last_read_v := SOME 1w;
-dr_init := 
-<| issue_wr_sysconfig := T; issue_wr_modulctrl := T; 
-issue_wr_ch0conf_wl := T; issue_wr_ch0conf_mode := T; 
-issue_wr_ch0conf_speed := T |> |>, 
-spi with <|state := spi_ready;
-regs := spi.regs with 
-<| SYSCONFIG := spi.regs.SYSCONFIG with <|SIDLEMODE := 2w; AUTOIDLE := 1w|>;
-MODULCTRL := <|SYSTEM_TEST := 0w; MS := 0w; SINGLE := 1w|>;
-CH0CONF := spi.regs.CH0CONF with
-<|PHA := 0w; POL := 0w; CLKD := 6w; EPOL := 1w; WL := 7w; 
-TRM := 0w; DPE0 := 1w; DPE1 := 0w; IS := 0w|> |>;
-init :=
-<|sysconfig_mode_done := T; modulctrl_bus_done := T; 
-ch0conf_wordlen_done :=  T; ch0conf_mode_done := T; 
-ch0conf_speed_done := T|> |>)``, 
-rw [n_tau_tr_def, n_tau_tr_SUC, local_tr_cases, driver_tr_cases, spi_tr_cases, 
-DR_TAU_ENABLE_def, SPI_TAU_ENABLE_def, DR_WR_ENABLE_def, DR_RD_ENABLE_def] >>
-`dr_read dr = dr with <| state := dr_init_check_rep;
-dr_last_read_ad := SOME SPI0_SYSSTATUS |>` by rw [dr_read_def, dr_read_sysstatus_def] >>
-rw [] >>
-`read_SPI_regs_state SPI0_SYSSTATUS spi = spi /\
-read_SPI_regs_value SPI0_SYSSTATUS spi = w2w spi.regs.SYSSTATUS` by
-rw [read_SPI_regs_state_def, read_SPI_regs_value_def, read_SPI_regs_def, SPI0_SYSSTATUS_def,
-SPI0_PA_RANGE_def, SPI0_START_def, SPI0_END_def, SPI0_SYSCONFIG_def] >>
-rw [] >>
-`dr_check (dr with <|state := dr_init_check_rep; 
-dr_last_read_ad := SOME SPI0_SYSSTATUS;
-dr_last_read_v := SOME 1w|>) SPI0_SYSSTATUS 1w =
-dr with <|state := dr_init_setting; dr_last_read_ad := SOME SPI0_SYSSTATUS;
-dr_last_read_v := SOME 1w|>` by rw [dr_check_def, dr_check_sysstatus_def] >>
-rw [] >>
-`(dr_write_state (dr with <|state := dr_init_setting; 
-dr_last_read_ad := SOME SPI0_SYSSTATUS;
-dr_last_read_v := SOME 1w|>) = dr with <| state := dr_init_setting;
-dr_last_read_ad := SOME SPI0_SYSSTATUS;
-dr_last_read_v := SOME 1w;
-dr_init := dr.dr_init with issue_wr_sysconfig := T |>) /\
-(dr_write_address (dr with <|state := dr_init_setting; 
-dr_last_read_ad := SOME SPI0_SYSSTATUS;
-dr_last_read_v := SOME 1w|>) = SOME SPI0_SYSCONFIG) /\
-(dr_write_value (dr with <|state := dr_init_setting; 
-dr_last_read_ad := SOME SPI0_SYSSTATUS;
-dr_last_read_v := SOME 1w|>) = SOME (0x00000011w:word32))` 
-by rw [dr_write_state_def, dr_write_address_def, dr_write_value_def,
-dr_write_def, dr_write_sysconfig_def] >>
-rw [] >>
-`write_SPI_regs SPI0_SYSCONFIG 17w spi = 
-(spi with <|state := init_setregs; 
-regs := spi.regs with 
-SYSCONFIG := spi.regs.SYSCONFIG with <|SIDLEMODE := 2w; AUTOIDLE := 1w|>; 
-init := spi.init with sysconfig_mode_done := T |>)`
-by rw [write_SPI_regs_def, SPI0_PA_RANGE_def, SPI0_START_def, SPI0_END_def, 
-SPI0_SYSCONFIG_def, write_SYSCONFIG_comb_def, write_SYSCONFIG_def] >>
-rw [] >>
-`(dr_write_state (dr with <|state := dr_init_setting;
-dr_last_read_ad := SOME SPI0_SYSSTATUS;
-dr_last_read_v := SOME 1w;
-dr_init := dr.dr_init with issue_wr_sysconfig := T |>) = 
-dr with <|state := dr_init_setting;
-dr_last_read_ad := SOME SPI0_SYSSTATUS;
-dr_last_read_v := SOME 1w;
-dr_init := dr.dr_init with 
-<|issue_wr_sysconfig := T ; issue_wr_modulctrl := T |> |>) /\
-(dr_write_address (dr with <| state := dr_init_setting;
-dr_last_read_ad := SOME SPI0_SYSSTATUS;
-dr_last_read_v := SOME 1w;
-dr_init := dr.dr_init with issue_wr_sysconfig := T |>) = SOME SPI0_MODULCTRL) /\
-(dr_write_value (dr with <| state := dr_init_setting;
-dr_last_read_ad := SOME SPI0_SYSSTATUS;
-dr_last_read_v := SOME 1w;
-dr_init := dr.dr_init with issue_wr_sysconfig := T |>) = SOME (0x00000001w))` 
-by fs [dr_write_state_def, dr_write_address_def, dr_write_value_def,
-dr_write_def, dr_write_modulctrl_def] >>
-rw [] >>
-`write_SPI_regs SPI0_MODULCTRL 1w 
-(spi with <|state := init_setregs; regs := spi.regs with 
-SYSCONFIG := spi.regs.SYSCONFIG with <|SIDLEMODE := 2w; AUTOIDLE := 1w|>; 
-init := spi.init with sysconfig_mode_done := T |>) =
-(spi with <|state := init_setregs; regs := spi.regs with
-<|SYSCONFIG := spi.regs.SYSCONFIG with <|SIDLEMODE := 2w; AUTOIDLE := 1w|>;
-MODULCTRL := <|SYSTEM_TEST := 0w; MS := 0w; SINGLE := 1w|> |>;
-init := spi.init with <|sysconfig_mode_done := T; modulctrl_bus_done := T |> |>)`
-by rw [write_SPI_regs_def, SPI0_PA_RANGE_def, SPI0_START_def, SPI0_END_def, 
-SPI0_SYSCONFIG_def, SPI0_MODULCTRL_def, write_MODULCTRL_def] >>
-rw [] >>
-`(dr_write_state (dr with <|state := dr_init_setting;
-dr_last_read_ad := SOME SPI0_SYSSTATUS;
-dr_last_read_v := SOME 1w;
-dr_init := dr.dr_init with <|issue_wr_sysconfig := T; issue_wr_modulctrl := T|> |>) = 
-dr with <|state := dr_init_setting;
-dr_last_read_ad := SOME SPI0_SYSSTATUS;
-dr_last_read_v := SOME 1w;
-dr_init := dr.dr_init with 
-<|issue_wr_sysconfig := T; issue_wr_modulctrl := T; issue_wr_ch0conf_wl := T |> |>) /\
-(dr_write_address (dr with <|state := dr_init_setting;
-dr_last_read_ad := SOME SPI0_SYSSTATUS;
-dr_last_read_v := SOME 1w;
-dr_init := dr.dr_init with <|issue_wr_sysconfig := T; issue_wr_modulctrl := T|> |>) = 
-SOME SPI0_CH0CONF) /\
-(dr_write_value (dr with <|state := dr_init_setting;
-dr_last_read_ad := SOME SPI0_SYSSTATUS;
-dr_last_read_v := SOME 1w;
-dr_init := dr.dr_init with <|issue_wr_sysconfig := T; issue_wr_modulctrl := T|> |>) = 
-SOME (0x00000380w:word32))` 
-by fs [dr_write_state_def, dr_write_address_def, dr_write_value_def,
-dr_write_def, dr_write_ch0conf_wl_def] >>
-rw [] >>
-`7w:word5 >+ 2w:word5` by EVAL_TAC >>
-`write_SPI_regs SPI0_CH0CONF 896w 
-(spi with <|state := init_setregs; 
-regs := spi.regs with 
-<| SYSCONFIG := spi.regs.SYSCONFIG with <|SIDLEMODE := 2w; AUTOIDLE := 1w|>;
-MODULCTRL := <|SYSTEM_TEST := 0w; MS := 0w; SINGLE := 1w|> |>;
-init := spi.init with 
-<|sysconfig_mode_done := T; modulctrl_bus_done := T|> |>) = 
-(spi with <|state := init_setregs; 
-regs := spi.regs with <|
-SYSCONFIG := spi.regs.SYSCONFIG with <|SIDLEMODE := 2w; AUTOIDLE := 1w|>;
-MODULCTRL := <|SYSTEM_TEST := 0w; MS := 0w; SINGLE := 1w|>;
-CH0CONF := spi.regs.CH0CONF with WL := 7w |>;
-init := spi.init with 
-<|ch0conf_wordlen_done := T; sysconfig_mode_done := T; modulctrl_bus_done := T |> |>)`
-by fs [write_SPI_regs_def, SPI0_CH0CONF_def, SPI0_PA_RANGE_def, 
-SPI0_START_def, SPI0_END_def, SPI0_SYSCONFIG_def, SPI0_MODULCTRL_def, 
-SPI0_TX0_def, write_CH0CONF_comb_def, write_CH0CONF_WL_def] >>
-rw [] >>
-rw [dr_write_state_def, dr_write_address_def, dr_write_value_def,
-dr_write_def, dr_write_ch0conf_speed_def, dr_write_ch0conf_mode_def] >>
-fs [write_SPI_regs_def, SPI0_CH0CONF_def, SPI0_PA_RANGE_def, 
-SPI0_START_def, SPI0_END_def, SPI0_SYSCONFIG_def, 
-SPI0_MODULCTRL_def, SPI0_TX0_def, write_CH0CONF_comb_def, 
-write_CH0CONF_def, write_CH0CONF_speed_def]);
-
-(* dr.state = dr_init_check_rep and spi.state = init_setregs, last_read_v = 0w *)
-val n_tau_tr_dr_init_check_rep_7 = store_thm("n_tau_tr_dr_init_check_rep_7",
-``!dr spi v. 
-dr.state = dr_init_check_rep /\ spi.state = init_setregs /\
-~ dr.dr_init.issue_wr_sysconfig /\ ~ dr.dr_init.issue_wr_modulctrl /\ 
-~ dr.dr_init.issue_wr_ch0conf_wl /\ ~ dr.dr_init.issue_wr_ch0conf_speed /\ 
-~ dr.dr_init.issue_wr_ch0conf_mode /\ ~ spi.init.sysconfig_mode_done /\
-~ spi.init.ch0conf_wordlen_done /\ ~ spi.init.ch0conf_mode_done /\ 
-~ spi.init.ch0conf_speed_done /\ ~ spi.init.modulctrl_bus_done /\
-spi.regs.SYSSTATUS = 1w /\ dr.dr_last_read_ad = SOME SPI0_SYSSTATUS /\
-dr.dr_last_read_v = SOME v /\ (0 >< 0) v:word1 = 0w ==>
-n_tau_tr 7 local_tr (dr,spi) tau 
-(dr with <| state := dr_ready; 
-dr_last_read_ad := SOME SPI0_SYSSTATUS;
-dr_last_read_v := SOME 1w;
-dr_init := 
-<| issue_wr_sysconfig := T; issue_wr_modulctrl := T; 
-issue_wr_ch0conf_wl := T; issue_wr_ch0conf_mode := T; 
-issue_wr_ch0conf_speed := T |> |>, 
-spi with <|state := spi_ready;
-regs := spi.regs with 
-<| SYSCONFIG := spi.regs.SYSCONFIG with <|SIDLEMODE := 2w; AUTOIDLE := 1w|>;
-MODULCTRL := <|SYSTEM_TEST := 0w; MS := 0w; SINGLE := 1w|>;
-CH0CONF := spi.regs.CH0CONF with
-<|PHA := 0w; POL := 0w; CLKD := 6w; EPOL := 1w; WL := 7w; 
-TRM := 0w; DPE0 := 1w; DPE1 := 0w; IS := 0w|> |>;
-init :=
-<|sysconfig_mode_done := T; modulctrl_bus_done := T; 
-ch0conf_wordlen_done :=  T; ch0conf_mode_done := T; 
-ch0conf_speed_done := T|> |>)``,
-rw [n_tau_tr_def, n_tau_tr_SUC, local_tr_cases, driver_tr_cases, spi_tr_cases, 
-DR_TAU_ENABLE_def, SPI_TAU_ENABLE_def, DR_WR_ENABLE_def, DR_RD_ENABLE_def] >>
-`dr_check dr SPI0_SYSSTATUS v = dr with state := dr_init_read_req` by rw [dr_check_def, dr_check_sysstatus_def] >>
-rw [] >>
-`dr_read (dr with state := dr_init_read_req) = dr with <| state := dr_init_check_rep;
-dr_last_read_ad := SOME SPI0_SYSSTATUS |>` by rw [dr_read_def, dr_read_sysstatus_def] >>
-rw [] >>
-`read_SPI_regs_state SPI0_SYSSTATUS spi = spi /\
-read_SPI_regs_value SPI0_SYSSTATUS spi = w2w spi.regs.SYSSTATUS` by
-rw [read_SPI_regs_state_def, read_SPI_regs_value_def, read_SPI_regs_def, SPI0_SYSSTATUS_def,
-SPI0_PA_RANGE_def, SPI0_START_def, SPI0_END_def, SPI0_SYSCONFIG_def] >>
-rw [] >>
-`dr_check (dr with <|state := dr_init_check_rep; 
-dr_last_read_ad := SOME SPI0_SYSSTATUS;
-dr_last_read_v := SOME 1w|>) SPI0_SYSSTATUS 1w =
-dr with <|state := dr_init_setting; dr_last_read_ad := SOME SPI0_SYSSTATUS;
-dr_last_read_v := SOME 1w|>` by rw [dr_check_def, dr_check_sysstatus_def] >>
-rw [] >>
-`(dr_write_state (dr with <|state := dr_init_setting; 
-dr_last_read_ad := SOME SPI0_SYSSTATUS;
-dr_last_read_v := SOME 1w|>) = dr with <| state := dr_init_setting;
-dr_last_read_ad := SOME SPI0_SYSSTATUS;
-dr_last_read_v := SOME 1w;
-dr_init := dr.dr_init with issue_wr_sysconfig := T |>) /\
-(dr_write_address (dr with <|state := dr_init_setting; 
-dr_last_read_ad := SOME SPI0_SYSSTATUS;
-dr_last_read_v := SOME 1w|>) = SOME SPI0_SYSCONFIG) /\
-(dr_write_value (dr with <|state := dr_init_setting; 
-dr_last_read_ad := SOME SPI0_SYSSTATUS;
-dr_last_read_v := SOME 1w|>) = SOME (0x00000011w:word32))` 
-by rw [dr_write_state_def, dr_write_address_def, dr_write_value_def,
-dr_write_def, dr_write_sysconfig_def] >>
-rw [] >>
-`write_SPI_regs SPI0_SYSCONFIG 17w spi = 
-(spi with <|state := init_setregs; 
-regs := spi.regs with 
-SYSCONFIG := spi.regs.SYSCONFIG with <|SIDLEMODE := 2w; AUTOIDLE := 1w|>; 
-init := spi.init with sysconfig_mode_done := T |>)`
-by rw [write_SPI_regs_def, SPI0_PA_RANGE_def, SPI0_START_def, SPI0_END_def, 
-SPI0_SYSCONFIG_def, write_SYSCONFIG_comb_def, write_SYSCONFIG_def] >>
-rw [] >>
-`(dr_write_state (dr with <|state := dr_init_setting;
-dr_last_read_ad := SOME SPI0_SYSSTATUS;
-dr_last_read_v := SOME 1w;
-dr_init := dr.dr_init with issue_wr_sysconfig := T |>) = 
-dr with <|state := dr_init_setting;
-dr_last_read_ad := SOME SPI0_SYSSTATUS;
-dr_last_read_v := SOME 1w;
-dr_init := dr.dr_init with 
-<|issue_wr_sysconfig := T ; issue_wr_modulctrl := T |> |>) /\
-(dr_write_address (dr with <| state := dr_init_setting;
-dr_last_read_ad := SOME SPI0_SYSSTATUS;
-dr_last_read_v := SOME 1w;
-dr_init := dr.dr_init with issue_wr_sysconfig := T |>) = SOME SPI0_MODULCTRL) /\
-(dr_write_value (dr with <| state := dr_init_setting;
-dr_last_read_ad := SOME SPI0_SYSSTATUS;
-dr_last_read_v := SOME 1w;
-dr_init := dr.dr_init with issue_wr_sysconfig := T |>) = SOME (0x00000001w))` 
-by fs [dr_write_state_def, dr_write_address_def, dr_write_value_def,
-dr_write_def, dr_write_modulctrl_def] >>
-rw [] >>
-`write_SPI_regs SPI0_MODULCTRL 1w 
-(spi with <|state := init_setregs; regs := spi.regs with 
-SYSCONFIG := spi.regs.SYSCONFIG with <|SIDLEMODE := 2w; AUTOIDLE := 1w|>; 
-init := spi.init with sysconfig_mode_done := T |>) =
-(spi with <|state := init_setregs; regs := spi.regs with
-<|SYSCONFIG := spi.regs.SYSCONFIG with <|SIDLEMODE := 2w; AUTOIDLE := 1w|>;
-MODULCTRL := <|SYSTEM_TEST := 0w; MS := 0w; SINGLE := 1w|> |>;
-init := spi.init with <|sysconfig_mode_done := T; modulctrl_bus_done := T |> |>)`
-by rw [write_SPI_regs_def, SPI0_PA_RANGE_def, SPI0_START_def, SPI0_END_def, 
-SPI0_SYSCONFIG_def, SPI0_MODULCTRL_def, write_MODULCTRL_def] >>
-rw [] >>
-`(dr_write_state (dr with <|state := dr_init_setting;
-dr_last_read_ad := SOME SPI0_SYSSTATUS;
-dr_last_read_v := SOME 1w;
-dr_init := dr.dr_init with <|issue_wr_sysconfig := T; issue_wr_modulctrl := T|> |>) = 
-dr with <|state := dr_init_setting;
-dr_last_read_ad := SOME SPI0_SYSSTATUS;
-dr_last_read_v := SOME 1w;
-dr_init := dr.dr_init with 
-<|issue_wr_sysconfig := T; issue_wr_modulctrl := T; issue_wr_ch0conf_wl := T |> |>) /\
-(dr_write_address (dr with <|state := dr_init_setting;
-dr_last_read_ad := SOME SPI0_SYSSTATUS;
-dr_last_read_v := SOME 1w;
-dr_init := dr.dr_init with <|issue_wr_sysconfig := T; issue_wr_modulctrl := T|> |>) = 
-SOME SPI0_CH0CONF) /\
-(dr_write_value (dr with <|state := dr_init_setting;
-dr_last_read_ad := SOME SPI0_SYSSTATUS;
-dr_last_read_v := SOME 1w;
-dr_init := dr.dr_init with <|issue_wr_sysconfig := T; issue_wr_modulctrl := T|> |>) = 
-SOME (0x00000380w:word32))` 
-by fs [dr_write_state_def, dr_write_address_def, dr_write_value_def,
-dr_write_def, dr_write_ch0conf_wl_def] >>
-rw [] >>
-`7w:word5 >+ 2w:word5` by EVAL_TAC >>
-`write_SPI_regs SPI0_CH0CONF 896w 
-(spi with <|state := init_setregs; 
-regs := spi.regs with 
-<| SYSCONFIG := spi.regs.SYSCONFIG with <|SIDLEMODE := 2w; AUTOIDLE := 1w|>;
-MODULCTRL := <|SYSTEM_TEST := 0w; MS := 0w; SINGLE := 1w|> |>;
-init := spi.init with 
-<|sysconfig_mode_done := T; modulctrl_bus_done := T|> |>) = 
-(spi with <|state := init_setregs; 
-regs := spi.regs with <|
-SYSCONFIG := spi.regs.SYSCONFIG with <|SIDLEMODE := 2w; AUTOIDLE := 1w|>;
-MODULCTRL := <|SYSTEM_TEST := 0w; MS := 0w; SINGLE := 1w|>;
-CH0CONF := spi.regs.CH0CONF with WL := 7w |>;
-init := spi.init with 
-<|ch0conf_wordlen_done := T; sysconfig_mode_done := T; modulctrl_bus_done := T |> |>)`
-by fs [write_SPI_regs_def, SPI0_CH0CONF_def, SPI0_PA_RANGE_def, 
-SPI0_START_def, SPI0_END_def, SPI0_SYSCONFIG_def, SPI0_MODULCTRL_def, 
-SPI0_TX0_def, write_CH0CONF_comb_def, write_CH0CONF_WL_def] >>
-rw [] >>
-rw [dr_write_state_def, dr_write_address_def, dr_write_value_def,
-dr_write_def, dr_write_ch0conf_speed_def, dr_write_ch0conf_mode_def] >>
-fs [write_SPI_regs_def, SPI0_CH0CONF_def, SPI0_PA_RANGE_def, 
-SPI0_START_def, SPI0_END_def, SPI0_SYSCONFIG_def, 
-SPI0_MODULCTRL_def, SPI0_TX0_def, write_CH0CONF_comb_def, 
-write_CH0CONF_def, write_CH0CONF_speed_def]);
-
-(* dr.state = dr_init_read_req and spi.state = init_reset *)
-val n_tau_tr_dr_init_read_req_7 = store_thm("n_tau_tr_dr_init_read_req_7",
-``!dr spi. 
-dr.state = dr_init_read_req /\ spi.state = init_reset /\
-~ dr.dr_init.issue_wr_sysconfig /\ ~ dr.dr_init.issue_wr_modulctrl /\ 
-~ dr.dr_init.issue_wr_ch0conf_wl /\ ~ dr.dr_init.issue_wr_ch0conf_speed /\ 
-~ dr.dr_init.issue_wr_ch0conf_mode /\ ~ spi.init.sysconfig_mode_done /\
-~ spi.init.ch0conf_wordlen_done /\ ~ spi.init.ch0conf_mode_done /\ 
-~ spi.init.ch0conf_speed_done /\ ~ spi.init.modulctrl_bus_done ==>
-n_tau_tr 7 local_tr (dr,spi) tau 
-(dr with <| state := dr_ready; 
-dr_last_read_ad := SOME SPI0_SYSSTATUS;
-dr_last_read_v := SOME 1w;
-dr_init := 
-<| issue_wr_sysconfig := T; issue_wr_modulctrl := T; 
-issue_wr_ch0conf_wl := T; issue_wr_ch0conf_mode := T; 
-issue_wr_ch0conf_speed := T |> |>, 
+dr_init := <| issue_wr_sysconfig := T; issue_wr_modulctrl := T |> |>, 
 spi with <|state := spi_ready;
 regs := spi.regs with 
 <| SYSCONFIG := spi.regs.SYSCONFIG with <|SIDLEMODE := 2w; AUTOIDLE := 1w|>;
 SYSSTATUS := 1w;
 MODULCTRL := <|SYSTEM_TEST := 0w; MS := 0w; SINGLE := 1w|>;
-CH0CONF := spi.regs.CH0CONF with
-<|PHA := 0w; POL := 0w; CLKD := 6w; EPOL := 1w; WL := 7w; 
-TRM := 0w; DPE0 := 1w; DPE1 := 0w; IS := 0w|> |>;
-init :=
-<|sysconfig_mode_done := T; modulctrl_bus_done := T; 
-ch0conf_wordlen_done :=  T; ch0conf_mode_done := T; 
-ch0conf_speed_done := T|> |>)``, 
+CH0CONF := <|PHA := 0w; POL := 0w; CLKD := 6w; EPOL := 1w; WL := 7w; 
+TRM := 0w; DPE0 := 1w; DPE1 := 0w; IS := 0w; FORCE := 0w|> |>;
+init := <|sysconfig_mode_done := T; modulctrl_bus_done := T|> |>)``, 
 rw [n_tau_tr_def, n_tau_tr_SUC, local_tr_cases, driver_tr_cases, spi_tr_cases, 
 DR_TAU_ENABLE_def, SPI_TAU_ENABLE_def, DR_WR_ENABLE_def, DR_RD_ENABLE_def, GSYM LEFT_EXISTS_AND_THM] >>
-Q.EXISTS_TAC `(dr,spi_tau_operations spi)` >>
-rw [] >>
-`spi_tau_operations spi = spi with <|regs := spi.regs with SYSSTATUS := 1w;
-state := init_setregs |>` by rw [spi_tau_operations_def, init_reset_op_def] >>
-rw [] >>
-`dr_read dr = dr with <| state := dr_init_check_rep;
-dr_last_read_ad := SOME SPI0_SYSSTATUS |>` by rw [dr_read_def, dr_read_sysstatus_def] >>
-rw [] >>
-`(read_SPI_regs_state SPI0_SYSSTATUS (spi with <|state := init_setregs;
-regs := spi.regs with SYSSTATUS := 1w|>) = (spi with <|state := init_setregs;
-regs := spi.regs with SYSSTATUS := 1w|>)) /\
-(read_SPI_regs_value SPI0_SYSSTATUS (spi with <|state := init_setregs;
-regs := spi.regs with SYSSTATUS := 1w|>) = 1w:word32)` 
-by rw [read_SPI_regs_state_def, read_SPI_regs_value_def, read_SPI_regs_def, SPI0_SYSSTATUS_def,
-SPI0_PA_RANGE_def, SPI0_START_def, SPI0_END_def, SPI0_SYSCONFIG_def] >>
-rw [] >>
-`dr_check (dr with <|state := dr_init_check_rep; 
-dr_last_read_ad := SOME SPI0_SYSSTATUS;
-dr_last_read_v := SOME 1w|>) SPI0_SYSSTATUS 1w =
-dr with <|state := dr_init_setting; dr_last_read_ad := SOME SPI0_SYSSTATUS;
-dr_last_read_v := SOME 1w|>` by rw [dr_check_def, dr_check_sysstatus_def] >>
-rw [] >>
-`(dr_write_state (dr with <|state := dr_init_setting; 
-dr_last_read_ad := SOME SPI0_SYSSTATUS;
-dr_last_read_v := SOME 1w|>) = dr with <| state := dr_init_setting;
-dr_last_read_ad := SOME SPI0_SYSSTATUS;
-dr_last_read_v := SOME 1w;
-dr_init := dr.dr_init with issue_wr_sysconfig := T |>) /\
-(dr_write_address (dr with <|state := dr_init_setting; 
-dr_last_read_ad := SOME SPI0_SYSSTATUS;
-dr_last_read_v := SOME 1w|>) = SOME SPI0_SYSCONFIG) /\
-(dr_write_value (dr with <|state := dr_init_setting; 
-dr_last_read_ad := SOME SPI0_SYSSTATUS;
-dr_last_read_v := SOME 1w|>) = SOME (0x00000011w:word32))` 
-by rw [dr_write_state_def, dr_write_address_def, dr_write_value_def,
-dr_write_def, dr_write_sysconfig_def] >>
-rw [] >>
-`write_SPI_regs SPI0_SYSCONFIG 17w (spi with <|state := init_setregs;
-regs := spi.regs with SYSSTATUS := 1w|>) = 
-(spi with <|state := init_setregs; 
-regs := spi.regs with 
-<|SYSSTATUS := 1w;
-SYSCONFIG := spi.regs.SYSCONFIG with <|SIDLEMODE := 2w; AUTOIDLE := 1w|> |>; 
-init := spi.init with sysconfig_mode_done := T |>)`
-by rw [write_SPI_regs_def, SPI0_PA_RANGE_def, SPI0_START_def, SPI0_END_def, 
-SPI0_SYSCONFIG_def, write_SYSCONFIG_comb_def, write_SYSCONFIG_def] >>
-rw [] >>
-`(dr_write_state (dr with <|state := dr_init_setting;
-dr_last_read_ad := SOME SPI0_SYSSTATUS;
-dr_last_read_v := SOME 1w;
-dr_init := dr.dr_init with issue_wr_sysconfig := T |>) = 
-dr with <|state := dr_init_setting;
-dr_last_read_ad := SOME SPI0_SYSSTATUS;
-dr_last_read_v := SOME 1w;
-dr_init := dr.dr_init with 
-<|issue_wr_sysconfig := T ; issue_wr_modulctrl := T |> |>) /\
-(dr_write_address (dr with <| state := dr_init_setting;
-dr_last_read_ad := SOME SPI0_SYSSTATUS;
-dr_last_read_v := SOME 1w;
-dr_init := dr.dr_init with issue_wr_sysconfig := T |>) = SOME SPI0_MODULCTRL) /\
-(dr_write_value (dr with <| state := dr_init_setting;
-dr_last_read_ad := SOME SPI0_SYSSTATUS;
-dr_last_read_v := SOME 1w;
-dr_init := dr.dr_init with issue_wr_sysconfig := T |>) = SOME (0x00000001w))` 
-by fs [dr_write_state_def, dr_write_address_def, dr_write_value_def,
-dr_write_def, dr_write_modulctrl_def] >>
-rw [] >>
-`write_SPI_regs SPI0_MODULCTRL 1w 
-(spi with <|state := init_setregs; regs := spi.regs with 
-<|SYSCONFIG := spi.regs.SYSCONFIG with <|SIDLEMODE := 2w; AUTOIDLE := 1w|>;
-SYSSTATUS := 1w|>; 
-init := spi.init with sysconfig_mode_done := T |>) =
-(spi with <|state := init_setregs; regs := spi.regs with
-<|SYSCONFIG := spi.regs.SYSCONFIG with <|SIDLEMODE := 2w; AUTOIDLE := 1w|>;
-SYSSTATUS := 1w;
-MODULCTRL := <|SYSTEM_TEST := 0w; MS := 0w; SINGLE := 1w|> |>;
-init := spi.init with <|sysconfig_mode_done := T; modulctrl_bus_done := T |> |>)`
-by rw [write_SPI_regs_def, SPI0_PA_RANGE_def, SPI0_START_def, SPI0_END_def, 
-SPI0_SYSCONFIG_def, SPI0_MODULCTRL_def, write_MODULCTRL_def] >>
-rw [] >>
-`(dr_write_state (dr with <|state := dr_init_setting;
-dr_last_read_ad := SOME SPI0_SYSSTATUS;
-dr_last_read_v := SOME 1w;
-dr_init := dr.dr_init with <|issue_wr_sysconfig := T; issue_wr_modulctrl := T|> |>) = 
-dr with <|state := dr_init_setting;
-dr_last_read_ad := SOME SPI0_SYSSTATUS;
-dr_last_read_v := SOME 1w;
-dr_init := dr.dr_init with 
-<|issue_wr_sysconfig := T; issue_wr_modulctrl := T; issue_wr_ch0conf_wl := T |> |>) /\
-(dr_write_address (dr with <|state := dr_init_setting;
-dr_last_read_ad := SOME SPI0_SYSSTATUS;
-dr_last_read_v := SOME 1w;
-dr_init := dr.dr_init with <|issue_wr_sysconfig := T; issue_wr_modulctrl := T|> |>) = 
-SOME SPI0_CH0CONF) /\
-(dr_write_value (dr with <|state := dr_init_setting;
-dr_last_read_ad := SOME SPI0_SYSSTATUS;
-dr_last_read_v := SOME 1w;
-dr_init := dr.dr_init with <|issue_wr_sysconfig := T; issue_wr_modulctrl := T|> |>) = 
-SOME (0x00000380w:word32))` 
-by fs [dr_write_state_def, dr_write_address_def, dr_write_value_def,
-dr_write_def, dr_write_ch0conf_wl_def] >>
-rw [] >>
-`7w:word5 >+ 2w:word5` by EVAL_TAC >>
-`write_SPI_regs SPI0_CH0CONF 896w 
-(spi with <|state := init_setregs; 
-regs := spi.regs with 
-<| SYSCONFIG := spi.regs.SYSCONFIG with <|SIDLEMODE := 2w; AUTOIDLE := 1w|>;
-SYSSTATUS := 1w;
-MODULCTRL := <|SYSTEM_TEST := 0w; MS := 0w; SINGLE := 1w|> |>;
-init := spi.init with 
-<|sysconfig_mode_done := T; modulctrl_bus_done := T|> |>) = 
-(spi with <|state := init_setregs; 
-regs := spi.regs with <|
-SYSCONFIG := spi.regs.SYSCONFIG with <|SIDLEMODE := 2w; AUTOIDLE := 1w|>;
-SYSSTATUS := 1w;
-MODULCTRL := <|SYSTEM_TEST := 0w; MS := 0w; SINGLE := 1w|>;
-CH0CONF := spi.regs.CH0CONF with WL := 7w |>;
-init := spi.init with 
-<|ch0conf_wordlen_done := T; sysconfig_mode_done := T; modulctrl_bus_done := T |> |>)`
-by fs [write_SPI_regs_def, SPI0_CH0CONF_def, SPI0_PA_RANGE_def, 
-SPI0_START_def, SPI0_END_def, SPI0_SYSCONFIG_def, SPI0_MODULCTRL_def, 
-SPI0_TX0_def, write_CH0CONF_comb_def, write_CH0CONF_WL_def] >>
-rw [] >>
-rw [dr_write_state_def, dr_write_address_def, dr_write_value_def,
-dr_write_def, dr_write_ch0conf_speed_def, dr_write_ch0conf_mode_def] >>
-fs [write_SPI_regs_def, SPI0_CH0CONF_def, SPI0_PA_RANGE_def, 
-SPI0_START_def, SPI0_END_def, SPI0_SYSCONFIG_def, 
-SPI0_MODULCTRL_def, SPI0_TX0_def, write_CH0CONF_comb_def, 
-write_CH0CONF_def, write_CH0CONF_speed_def]);
-
-(* dr.state = dr_init_check_rep and spi.state = init_setregs *)
-val n_tau_tr_dr_init_check_rep_7 = store_thm("n_tau_tr_dr_init_check_rep_7",
-``!dr spi v. 
-dr.state = dr_init_check_rep /\ spi.state = init_setregs /\
-~ dr.dr_init.issue_wr_sysconfig /\ ~ dr.dr_init.issue_wr_modulctrl /\ 
-~ dr.dr_init.issue_wr_ch0conf_wl /\ ~ dr.dr_init.issue_wr_ch0conf_speed /\ 
-~ dr.dr_init.issue_wr_ch0conf_mode /\ ~ spi.init.sysconfig_mode_done /\
-~ spi.init.ch0conf_wordlen_done /\ ~ spi.init.ch0conf_mode_done /\ 
-~ spi.init.ch0conf_speed_done /\ ~ spi.init.modulctrl_bus_done /\
-spi.regs.SYSSTATUS = 1w /\ dr.dr_last_read_ad = SOME SPI0_SYSSTATUS /\
-dr.dr_last_read_v = SOME v /\ (0 >< 0) v:word1 = 0w ==>
-n_tau_tr 7 local_tr (dr,spi) tau 
-(dr with <| state := dr_ready; 
-dr_last_read_ad := SOME SPI0_SYSSTATUS;
-dr_last_read_v := SOME 1w;
-dr_init := 
-<| issue_wr_sysconfig := T; issue_wr_modulctrl := T; 
-issue_wr_ch0conf_wl := T; issue_wr_ch0conf_mode := T; 
-issue_wr_ch0conf_speed := T |> |>, 
-spi with <|state := spi_ready;
-regs := spi.regs with 
-<| SYSCONFIG := spi.regs.SYSCONFIG with <|SIDLEMODE := 2w; AUTOIDLE := 1w|>;
-MODULCTRL := <|SYSTEM_TEST := 0w; MS := 0w; SINGLE := 1w|>;
-CH0CONF := spi.regs.CH0CONF with
-<|PHA := 0w; POL := 0w; CLKD := 6w; EPOL := 1w; WL := 7w; 
-TRM := 0w; DPE0 := 1w; DPE1 := 0w; IS := 0w|> |>;
-init :=
-<|sysconfig_mode_done := T; modulctrl_bus_done := T; 
-ch0conf_wordlen_done :=  T; ch0conf_mode_done := T; 
-ch0conf_speed_done := T|> |>)``,
-rw [n_tau_tr_def, n_tau_tr_SUC, local_tr_cases, driver_tr_cases, spi_tr_cases, 
-DR_TAU_ENABLE_def, SPI_TAU_ENABLE_def, DR_WR_ENABLE_def, DR_RD_ENABLE_def] >>
-`dr_check dr SPI0_SYSSTATUS v = dr with state := dr_init_read_req` by rw [dr_check_def, dr_check_sysstatus_def] >>
-rw [] >>
-`dr_read (dr with state := dr_init_read_req) = dr with <| state := dr_init_check_rep;
-dr_last_read_ad := SOME SPI0_SYSSTATUS |>` by rw [dr_read_def, dr_read_sysstatus_def] >>
-rw [] >>
-`read_SPI_regs_state SPI0_SYSSTATUS spi = spi /\
-read_SPI_regs_value SPI0_SYSSTATUS spi = w2w spi.regs.SYSSTATUS` by
-rw [read_SPI_regs_state_def, read_SPI_regs_value_def, read_SPI_regs_def, SPI0_SYSSTATUS_def,
-SPI0_PA_RANGE_def, SPI0_START_def, SPI0_END_def, SPI0_SYSCONFIG_def] >>
-rw [] >>
-`dr_check (dr with <|state := dr_init_check_rep; 
-dr_last_read_ad := SOME SPI0_SYSSTATUS;
-dr_last_read_v := SOME 1w|>) SPI0_SYSSTATUS 1w =
-dr with <|state := dr_init_setting; dr_last_read_ad := SOME SPI0_SYSSTATUS;
-dr_last_read_v := SOME 1w|>` by rw [dr_check_def, dr_check_sysstatus_def] >>
-rw [] >>
-`(dr_write_state (dr with <|state := dr_init_setting; 
-dr_last_read_ad := SOME SPI0_SYSSTATUS;
-dr_last_read_v := SOME 1w|>) = dr with <| state := dr_init_setting;
-dr_last_read_ad := SOME SPI0_SYSSTATUS;
-dr_last_read_v := SOME 1w;
-dr_init := dr.dr_init with issue_wr_sysconfig := T |>) /\
-(dr_write_address (dr with <|state := dr_init_setting; 
-dr_last_read_ad := SOME SPI0_SYSSTATUS;
-dr_last_read_v := SOME 1w|>) = SOME SPI0_SYSCONFIG) /\
-(dr_write_value (dr with <|state := dr_init_setting; 
-dr_last_read_ad := SOME SPI0_SYSSTATUS;
-dr_last_read_v := SOME 1w|>) = SOME (0x00000011w:word32))` 
-by rw [dr_write_state_def, dr_write_address_def, dr_write_value_def,
-dr_write_def, dr_write_sysconfig_def] >>
-rw [] >>
-`write_SPI_regs SPI0_SYSCONFIG 17w spi = 
-(spi with <|state := init_setregs; 
-regs := spi.regs with 
-SYSCONFIG := spi.regs.SYSCONFIG with <|SIDLEMODE := 2w; AUTOIDLE := 1w|>; 
-init := spi.init with sysconfig_mode_done := T |>)`
-by rw [write_SPI_regs_def, SPI0_PA_RANGE_def, SPI0_START_def, SPI0_END_def, 
-SPI0_SYSCONFIG_def, write_SYSCONFIG_comb_def, write_SYSCONFIG_def] >>
-rw [] >>
-`(dr_write_state (dr with <|state := dr_init_setting;
-dr_last_read_ad := SOME SPI0_SYSSTATUS;
-dr_last_read_v := SOME 1w;
-dr_init := dr.dr_init with issue_wr_sysconfig := T |>) = 
-dr with <|state := dr_init_setting;
-dr_last_read_ad := SOME SPI0_SYSSTATUS;
-dr_last_read_v := SOME 1w;
-dr_init := dr.dr_init with 
-<|issue_wr_sysconfig := T ; issue_wr_modulctrl := T |> |>) /\
-(dr_write_address (dr with <| state := dr_init_setting;
-dr_last_read_ad := SOME SPI0_SYSSTATUS;
-dr_last_read_v := SOME 1w;
-dr_init := dr.dr_init with issue_wr_sysconfig := T |>) = SOME SPI0_MODULCTRL) /\
-(dr_write_value (dr with <| state := dr_init_setting;
-dr_last_read_ad := SOME SPI0_SYSSTATUS;
-dr_last_read_v := SOME 1w;
-dr_init := dr.dr_init with issue_wr_sysconfig := T |>) = SOME (0x00000001w))` 
-by fs [dr_write_state_def, dr_write_address_def, dr_write_value_def,
-dr_write_def, dr_write_modulctrl_def] >>
-rw [] >>
-`write_SPI_regs SPI0_MODULCTRL 1w 
-(spi with <|state := init_setregs; regs := spi.regs with 
-SYSCONFIG := spi.regs.SYSCONFIG with <|SIDLEMODE := 2w; AUTOIDLE := 1w|>; 
-init := spi.init with sysconfig_mode_done := T |>) =
-(spi with <|state := init_setregs; regs := spi.regs with
-<|SYSCONFIG := spi.regs.SYSCONFIG with <|SIDLEMODE := 2w; AUTOIDLE := 1w|>;
-MODULCTRL := <|SYSTEM_TEST := 0w; MS := 0w; SINGLE := 1w|> |>;
-init := spi.init with <|sysconfig_mode_done := T; modulctrl_bus_done := T |> |>)`
-by rw [write_SPI_regs_def, SPI0_PA_RANGE_def, SPI0_START_def, SPI0_END_def, 
-SPI0_SYSCONFIG_def, SPI0_MODULCTRL_def, write_MODULCTRL_def] >>
-rw [] >>
-`(dr_write_state (dr with <|state := dr_init_setting;
-dr_last_read_ad := SOME SPI0_SYSSTATUS;
-dr_last_read_v := SOME 1w;
-dr_init := dr.dr_init with <|issue_wr_sysconfig := T; issue_wr_modulctrl := T|> |>) = 
-dr with <|state := dr_init_setting;
-dr_last_read_ad := SOME SPI0_SYSSTATUS;
-dr_last_read_v := SOME 1w;
-dr_init := dr.dr_init with 
-<|issue_wr_sysconfig := T; issue_wr_modulctrl := T; issue_wr_ch0conf_wl := T |> |>) /\
-(dr_write_address (dr with <|state := dr_init_setting;
-dr_last_read_ad := SOME SPI0_SYSSTATUS;
-dr_last_read_v := SOME 1w;
-dr_init := dr.dr_init with <|issue_wr_sysconfig := T; issue_wr_modulctrl := T|> |>) = 
-SOME SPI0_CH0CONF) /\
-(dr_write_value (dr with <|state := dr_init_setting;
-dr_last_read_ad := SOME SPI0_SYSSTATUS;
-dr_last_read_v := SOME 1w;
-dr_init := dr.dr_init with <|issue_wr_sysconfig := T; issue_wr_modulctrl := T|> |>) = 
-SOME (0x00000380w:word32))` 
-by fs [dr_write_state_def, dr_write_address_def, dr_write_value_def,
-dr_write_def, dr_write_ch0conf_wl_def] >>
-rw [] >>
-`7w:word5 >+ 2w:word5` by EVAL_TAC >>
-`write_SPI_regs SPI0_CH0CONF 896w 
-(spi with <|state := init_setregs; 
-regs := spi.regs with 
-<| SYSCONFIG := spi.regs.SYSCONFIG with <|SIDLEMODE := 2w; AUTOIDLE := 1w|>;
-MODULCTRL := <|SYSTEM_TEST := 0w; MS := 0w; SINGLE := 1w|> |>;
-init := spi.init with 
-<|sysconfig_mode_done := T; modulctrl_bus_done := T|> |>) = 
-(spi with <|state := init_setregs; 
-regs := spi.regs with <|
-SYSCONFIG := spi.regs.SYSCONFIG with <|SIDLEMODE := 2w; AUTOIDLE := 1w|>;
-MODULCTRL := <|SYSTEM_TEST := 0w; MS := 0w; SINGLE := 1w|>;
-CH0CONF := spi.regs.CH0CONF with WL := 7w |>;
-init := spi.init with 
-<|ch0conf_wordlen_done := T; sysconfig_mode_done := T; modulctrl_bus_done := T |> |>)`
-by fs [write_SPI_regs_def, SPI0_CH0CONF_def, SPI0_PA_RANGE_def, 
-SPI0_START_def, SPI0_END_def, SPI0_SYSCONFIG_def, SPI0_MODULCTRL_def, 
-SPI0_TX0_def, write_CH0CONF_comb_def, write_CH0CONF_WL_def] >>
-rw [] >>
-rw [dr_write_state_def, dr_write_address_def, dr_write_value_def,
-dr_write_def, dr_write_ch0conf_speed_def, dr_write_ch0conf_mode_def] >>
-fs [write_SPI_regs_def, SPI0_CH0CONF_def, SPI0_PA_RANGE_def, 
-SPI0_START_def, SPI0_END_def, SPI0_SYSCONFIG_def, 
-SPI0_MODULCTRL_def, SPI0_TX0_def, write_CH0CONF_comb_def, 
-write_CH0CONF_def, write_CH0CONF_speed_def]);
-
-(* dr.state = dr_init_check_rep and spi.state = init_reset *)
-val n_tau_tr_dr_init_check_rep_8 = store_thm("n_tau_tr_dr_init_check_rep_8",
-``!dr spi v. 
-dr.state = dr_init_check_rep /\ spi.state = init_reset /\
-~ dr.dr_init.issue_wr_sysconfig /\ ~ dr.dr_init.issue_wr_modulctrl /\ 
-~ dr.dr_init.issue_wr_ch0conf_wl /\ ~ dr.dr_init.issue_wr_ch0conf_speed /\ 
-~ dr.dr_init.issue_wr_ch0conf_mode /\ ~ spi.init.sysconfig_mode_done /\
-~ spi.init.ch0conf_wordlen_done /\ ~ spi.init.ch0conf_mode_done /\ 
-~ spi.init.ch0conf_speed_done /\ ~ spi.init.modulctrl_bus_done /\
-dr.dr_last_read_ad = SOME SPI0_SYSSTATUS /\ dr.dr_last_read_v = SOME v /\
-(0 >< 0) v:word1 = 0w ==>
-n_tau_tr 8 local_tr (dr,spi) tau 
-(dr with <| state := dr_ready; 
-dr_last_read_ad := SOME SPI0_SYSSTATUS;
-dr_last_read_v := SOME 1w;
-dr_init := 
-<| issue_wr_sysconfig := T; issue_wr_modulctrl := T; 
-issue_wr_ch0conf_wl := T; issue_wr_ch0conf_mode := T; 
-issue_wr_ch0conf_speed := T |> |>, 
-spi with <|state := spi_ready;
-regs := spi.regs with 
-<| SYSCONFIG := spi.regs.SYSCONFIG with <|SIDLEMODE := 2w; AUTOIDLE := 1w|>;
-SYSSTATUS := 1w;
-MODULCTRL := <|SYSTEM_TEST := 0w; MS := 0w; SINGLE := 1w|>;
-CH0CONF := spi.regs.CH0CONF with
-<|PHA := 0w; POL := 0w; CLKD := 6w; EPOL := 1w; WL := 7w; 
-TRM := 0w; DPE0 := 1w; DPE1 := 0w; IS := 0w|> |>;
-init :=
-<|sysconfig_mode_done := T; modulctrl_bus_done := T; 
-ch0conf_wordlen_done :=  T; ch0conf_mode_done := T; 
-ch0conf_speed_done := T|> |>)``, 
-rw [n_tau_tr_def, n_tau_tr_SUC, local_tr_cases, driver_tr_cases, spi_tr_cases, 
-DR_TAU_ENABLE_def, SPI_TAU_ENABLE_def, DR_WR_ENABLE_def, DR_RD_ENABLE_def, GSYM LEFT_EXISTS_AND_THM] >>
-Q.EXISTS_TAC `(dr_check dr SPI0_SYSSTATUS v,spi)` >>
-rw [] >>
+Q.EXISTS_TAC `(dr_check dr SPI0_SYSSTATUS v,spi)` >> rw [] >>
 `dr_check dr SPI0_SYSSTATUS v = dr with state := dr_init_read_req` by rw [dr_check_def, dr_check_sysstatus_def] >>
 rw [GSYM LEFT_EXISTS_AND_THM] >>
-Q.EXISTS_TAC `(dr with state := dr_init_read_req, spi_tau_operations spi)` >>
-rw [] >>
-`spi_tau_operations spi = spi with <|regs := spi.regs with SYSSTATUS := 1w;
-state := init_setregs |>` by rw [spi_tau_operations_def, init_reset_op_def] >>
-rw [] >>
+Q.EXISTS_TAC `(dr with state := dr_init_read_req, spi_tau_operations spi)` >> rw [] >>
+`spi_tau_operations spi = spi with <|regs := spi.regs with <|SYSSTATUS := 1w;
+CH0CONF := <|PHA := 0w; POL := 0w; CLKD := 0w; EPOL := 0w; WL := 0w;
+TRM := 0w; DPE0 := 0w; DPE1 := 1w; IS := 1w; FORCE := 0w|> |>;
+state := init_setregs |>` by rw [spi_tau_operations_def, init_reset_op_def] >> rw [] >>
 `dr_read (dr with state := dr_init_read_req) = dr with <| state := dr_init_check_rep;
-dr_last_read_ad := SOME SPI0_SYSSTATUS |>` by rw [dr_read_def, dr_read_sysstatus_def] >>
-rw [] >>
+dr_last_read_ad := SOME SPI0_SYSSTATUS |>` by rw [dr_read_def, dr_read_sysstatus_def] >> rw [] >>
 `(read_SPI_regs_state SPI0_SYSSTATUS (spi with <|state := init_setregs;
-regs := spi.regs with SYSSTATUS := 1w|>) = (spi with <|state := init_setregs;
-regs := spi.regs with SYSSTATUS := 1w|>)) /\
+regs := spi.regs with <|SYSSTATUS := 1w;
+CH0CONF := <|PHA := 0w; POL := 0w; CLKD := 0w; EPOL := 0w; WL := 0w;
+TRM := 0w; DPE0 := 0w; DPE1 := 1w; IS := 1w; FORCE := 0w|> |> |>) = 
+(spi with <|state := init_setregs;
+regs := spi.regs with <|SYSSTATUS := 1w;
+CH0CONF := <|PHA := 0w; POL := 0w; CLKD := 0w; EPOL := 0w; WL := 0w;
+TRM := 0w; DPE0 := 0w; DPE1 := 1w; IS := 1w; FORCE := 0w|> |> |>)) /\
 (read_SPI_regs_value SPI0_SYSSTATUS (spi with <|state := init_setregs;
-regs := spi.regs with SYSSTATUS := 1w|>) = 1w:word32)` 
+regs := spi.regs with <|SYSSTATUS := 1w;
+CH0CONF := <|PHA := 0w; POL := 0w; CLKD := 0w; EPOL := 0w; WL := 0w;
+TRM := 0w; DPE0 := 0w; DPE1 := 1w; IS := 1w; FORCE := 0w|> |> |>) = 1w:word32)` 
 by rw [read_SPI_regs_state_def, read_SPI_regs_value_def, read_SPI_regs_def, SPI0_SYSSTATUS_def,
-SPI0_PA_RANGE_def, SPI0_START_def, SPI0_END_def, SPI0_SYSCONFIG_def] >>
-rw [] >>
+SPI0_PA_RANGE_def, SPI0_START_def, SPI0_END_def, SPI0_SYSCONFIG_def] >> rw [] >>
 `dr_check (dr with <|state := dr_init_check_rep; 
 dr_last_read_ad := SOME SPI0_SYSSTATUS;
 dr_last_read_v := SOME 1w|>) SPI0_SYSSTATUS 1w =
 dr with <|state := dr_init_setting; dr_last_read_ad := SOME SPI0_SYSSTATUS;
-dr_last_read_v := SOME 1w|>` by rw [dr_check_def, dr_check_sysstatus_def] >>
-rw [] >>
+dr_last_read_v := SOME 1w|>` by rw [dr_check_def, dr_check_sysstatus_def] >> rw [] >>
 `(dr_write_state (dr with <|state := dr_init_setting; 
 dr_last_read_ad := SOME SPI0_SYSSTATUS;
 dr_last_read_v := SOME 1w|>) = dr with <| state := dr_init_setting;
@@ -1059,18 +704,19 @@ dr_last_read_v := SOME 1w|>) = SOME SPI0_SYSCONFIG) /\
 dr_last_read_ad := SOME SPI0_SYSSTATUS;
 dr_last_read_v := SOME 1w|>) = SOME (0x00000011w:word32))` 
 by rw [dr_write_state_def, dr_write_address_def, dr_write_value_def,
-dr_write_def, dr_write_sysconfig_def] >>
-rw [] >>
+dr_write_def, dr_write_sysconfig_def] >> rw [] >>
 `write_SPI_regs SPI0_SYSCONFIG 17w (spi with <|state := init_setregs;
-regs := spi.regs with SYSSTATUS := 1w|>) = 
+regs := spi.regs with <|SYSSTATUS := 1w;
+CH0CONF := <|PHA := 0w; POL := 0w; CLKD := 0w; EPOL := 0w; WL := 0w;
+TRM := 0w; DPE0 := 0w; DPE1 := 1w; IS := 1w; FORCE := 0w|> |> |>) = 
 (spi with <|state := init_setregs; 
-regs := spi.regs with 
-<|SYSSTATUS := 1w;
+regs := spi.regs with  <|SYSSTATUS := 1w;
+CH0CONF := <|PHA := 0w; POL := 0w; CLKD := 0w; EPOL := 0w; WL := 0w;
+TRM := 0w; DPE0 := 0w; DPE1 := 1w; IS := 1w; FORCE := 0w|>;
 SYSCONFIG := spi.regs.SYSCONFIG with <|SIDLEMODE := 2w; AUTOIDLE := 1w|> |>; 
 init := spi.init with sysconfig_mode_done := T |>)`
 by rw [write_SPI_regs_def, SPI0_PA_RANGE_def, SPI0_START_def, SPI0_END_def, 
-SPI0_SYSCONFIG_def, write_SYSCONFIG_comb_def, write_SYSCONFIG_def] >>
-rw [] >>
+SPI0_SYSCONFIG_def, write_SYSCONFIG_comb_def, write_SYSCONFIG_def] >> rw [] >>
 `(dr_write_state (dr with <|state := dr_init_setting;
 dr_last_read_ad := SOME SPI0_SYSSTATUS;
 dr_last_read_v := SOME 1w;
@@ -1089,30 +735,33 @@ dr_last_read_ad := SOME SPI0_SYSSTATUS;
 dr_last_read_v := SOME 1w;
 dr_init := dr.dr_init with issue_wr_sysconfig := T |>) = SOME (0x00000001w))` 
 by fs [dr_write_state_def, dr_write_address_def, dr_write_value_def,
-dr_write_def, dr_write_modulctrl_def] >>
-rw [] >>
+dr_write_def, dr_write_modulctrl_def] >> rw [] >>
+`~(0w:word5 >+ 2w:word5)` by EVAL_TAC >>
 `write_SPI_regs SPI0_MODULCTRL 1w 
-(spi with <|state := init_setregs; regs := spi.regs with 
+(spi with <|state := init_setregs; 
+regs := spi.regs with 
 <|SYSCONFIG := spi.regs.SYSCONFIG with <|SIDLEMODE := 2w; AUTOIDLE := 1w|>;
-SYSSTATUS := 1w|>; 
+SYSSTATUS := 1w;
+CH0CONF := <|PHA := 0w; POL := 0w; CLKD := 0w; EPOL := 0w; WL := 0w; 
+TRM := 0w; DPE0 := 0w; DPE1 := 1w; IS := 1w; FORCE := 0w|> |>; 
 init := spi.init with sysconfig_mode_done := T |>) =
 (spi with <|state := init_setregs; regs := spi.regs with
 <|SYSCONFIG := spi.regs.SYSCONFIG with <|SIDLEMODE := 2w; AUTOIDLE := 1w|>;
 SYSSTATUS := 1w;
-MODULCTRL := <|SYSTEM_TEST := 0w; MS := 0w; SINGLE := 1w|> |>;
-init := spi.init with <|sysconfig_mode_done := T; modulctrl_bus_done := T |> |>)`
+MODULCTRL := <|SYSTEM_TEST := 0w; MS := 0w; SINGLE := 1w|>;
+CH0CONF := <|PHA := 0w; POL := 0w; CLKD := 0w; EPOL := 0w; WL := 0w; 
+TRM := 0w; DPE0 := 0w; DPE1 := 1w; IS := 1w; FORCE := 0w|> |>;
+init := <|sysconfig_mode_done := T; modulctrl_bus_done := T|> |>)`
 by rw [write_SPI_regs_def, SPI0_PA_RANGE_def, SPI0_START_def, SPI0_END_def, 
-SPI0_SYSCONFIG_def, SPI0_MODULCTRL_def, write_MODULCTRL_def] >>
-rw [] >>
+SPI0_SYSCONFIG_def, SPI0_MODULCTRL_def, write_MODULCTRL_def] >> fs [] >>
 `(dr_write_state (dr with <|state := dr_init_setting;
 dr_last_read_ad := SOME SPI0_SYSSTATUS;
 dr_last_read_v := SOME 1w;
 dr_init := dr.dr_init with <|issue_wr_sysconfig := T; issue_wr_modulctrl := T|> |>) = 
-dr with <|state := dr_init_setting;
+dr with <|state := dr_ready;
 dr_last_read_ad := SOME SPI0_SYSSTATUS;
 dr_last_read_v := SOME 1w;
-dr_init := dr.dr_init with 
-<|issue_wr_sysconfig := T; issue_wr_modulctrl := T; issue_wr_ch0conf_wl := T |> |>) /\
+dr_init := <|issue_wr_sysconfig := T; issue_wr_modulctrl := T|> |>) /\
 (dr_write_address (dr with <|state := dr_init_setting;
 dr_last_read_ad := SOME SPI0_SYSSTATUS;
 dr_last_read_v := SOME 1w;
@@ -1122,277 +771,236 @@ SOME SPI0_CH0CONF) /\
 dr_last_read_ad := SOME SPI0_SYSSTATUS;
 dr_last_read_v := SOME 1w;
 dr_init := dr.dr_init with <|issue_wr_sysconfig := T; issue_wr_modulctrl := T|> |>) = 
-SOME (0x00000380w:word32))` 
+SOME (66520w:word32))` 
 by fs [dr_write_state_def, dr_write_address_def, dr_write_value_def,
-dr_write_def, dr_write_ch0conf_wl_def] >>
-rw [] >>
-`7w:word5 >+ 2w:word5` by EVAL_TAC >>
-`write_SPI_regs SPI0_CH0CONF 896w 
-(spi with <|state := init_setregs; 
-regs := spi.regs with 
-<| SYSCONFIG := spi.regs.SYSCONFIG with <|SIDLEMODE := 2w; AUTOIDLE := 1w|>;
-SYSSTATUS := 1w;
-MODULCTRL := <|SYSTEM_TEST := 0w; MS := 0w; SINGLE := 1w|> |>;
-init := spi.init with 
-<|sysconfig_mode_done := T; modulctrl_bus_done := T|> |>) = 
-(spi with <|state := init_setregs; 
-regs := spi.regs with <|
-SYSCONFIG := spi.regs.SYSCONFIG with <|SIDLEMODE := 2w; AUTOIDLE := 1w|>;
-SYSSTATUS := 1w;
+dr_write_def, dr_write_ch0conf_init_def] >> fs [] >>
+`(spi with <|state := init_setregs;
+regs := spi.regs with <|SYSCONFIG := spi.regs.SYSCONFIG with
+<|SIDLEMODE := 2w; AUTOIDLE := 1w|>; SYSSTATUS := 1w;
 MODULCTRL := <|SYSTEM_TEST := 0w; MS := 0w; SINGLE := 1w|>;
-CH0CONF := spi.regs.CH0CONF with WL := 7w |>;
-init := spi.init with 
-<|ch0conf_wordlen_done := T; sysconfig_mode_done := T; modulctrl_bus_done := T |> |>)`
-by fs [write_SPI_regs_def, SPI0_CH0CONF_def, SPI0_PA_RANGE_def, 
-SPI0_START_def, SPI0_END_def, SPI0_SYSCONFIG_def, SPI0_MODULCTRL_def, 
-SPI0_TX0_def, write_CH0CONF_comb_def, write_CH0CONF_WL_def] >>
-rw [] >>
-rw [dr_write_state_def, dr_write_address_def, dr_write_value_def,
-dr_write_def, dr_write_ch0conf_speed_def, dr_write_ch0conf_mode_def] >>
-fs [write_SPI_regs_def, SPI0_CH0CONF_def, SPI0_PA_RANGE_def, 
-SPI0_START_def, SPI0_END_def, SPI0_SYSCONFIG_def, 
-SPI0_MODULCTRL_def, SPI0_TX0_def, write_CH0CONF_comb_def, 
-write_CH0CONF_def, write_CH0CONF_speed_def]);
+CH0CONF := <|PHA := 0w; POL := 0w; CLKD := 0w; EPOL := 0w; WL := 0w;
+TRM := 0w; DPE0 := 0w; DPE1 := 1w; IS := 1w; FORCE := 0w|> |>;
+init := <|sysconfig_mode_done := T; modulctrl_bus_done := T|> |>).regs.CH0CONF.IS = 1w` by fs [] >>
+`(19 >< 19) (66520w:word32):word1 <> ((spi with <|state := init_setregs;
+regs := spi.regs with <|SYSCONFIG := spi.regs.SYSCONFIG with
+<|SIDLEMODE := 2w; AUTOIDLE := 1w|>; SYSSTATUS := 1w;
+MODULCTRL := <|SYSTEM_TEST := 0w; MS := 0w; SINGLE := 1w|>;
+CH0CONF := <|PHA := 0w; POL := 0w; CLKD := 0w; EPOL := 0w; WL := 0w;
+TRM := 0w; DPE0 := 0w; DPE1 := 1w; IS := 1w; FORCE := 0w|> |>;
+init := <|sysconfig_mode_done := T; modulctrl_bus_done := T|> |>).regs.CH0CONF.IS)` 
+by FULL_SIMP_TAC (std_ss++WORD_ss) [] >>
+`ch0conf_changed (66520w:word32) 
+(spi with <|state := init_setregs;
+regs := spi.regs with <|SYSCONFIG := spi.regs.SYSCONFIG with
+<|SIDLEMODE := 2w; AUTOIDLE := 1w|>; SYSSTATUS := 1w;
+MODULCTRL := <|SYSTEM_TEST := 0w; MS := 0w; SINGLE := 1w|>;
+CH0CONF := <|PHA := 0w; POL := 0w; CLKD := 0w; EPOL := 0w; WL := 0w;
+TRM := 0w; DPE0 := 0w; DPE1 := 1w; IS := 1w; FORCE := 0w|> |>;
+init := <|sysconfig_mode_done := T; modulctrl_bus_done := T|> |>)` by fs [ch0conf_changed_def] >>
+rw [write_SPI_regs_def, SPI0_CH0CONF_def, SPI0_PA_RANGE_def, SPI0_START_def, 
+SPI0_END_def, SPI0_SYSCONFIG_def, SPI0_MODULCTRL_def, SPI0_TX0_def, 
+write_CH0CONF_comb_def, write_CH0CONF_init_def] >>
+`7w:word5 >+ 2w:word5` by EVAL_TAC >>
+fs [ref_rel_def, IS_STATE_REL_def]);
 
 (* dr.state = dr_init_idle and spi.state = init_start or spi_ready *)
-val n_tau_tr_dr_init_idle_8 = store_thm("n_tau_tr_dr_init_check_rep_8",
+val n_tau_tr_dr_init_idle_6 = store_thm("n_tau_tr_dr_init_check_rep_6",
 ``!dr spi. 
 dr.state = dr_init_idle /\ (spi.state = init_start \/ spi.state = spi_ready) ==>
-n_tau_tr 8 local_tr (dr,spi) tau 
+n_tau_tr 6 local_tr (dr,spi) tau 
 (dr with <| state := dr_ready; 
 dr_last_read_ad := SOME SPI0_SYSSTATUS;
 dr_last_read_v := SOME 1w;
-dr_init := 
-<| issue_wr_sysconfig := T; issue_wr_modulctrl := T; 
-issue_wr_ch0conf_wl := T; issue_wr_ch0conf_mode := T; 
-issue_wr_ch0conf_speed := T |> |>, 
+dr_init := <|issue_wr_sysconfig := T; issue_wr_modulctrl := T|> |>, 
 spi with <|state := spi_ready;
 regs := spi.regs with 
 <| SYSCONFIG := <|SIDLEMODE := 2w; SOFTRESET := 0w; AUTOIDLE := 1w|>;
 SYSSTATUS := 1w;
 MODULCTRL := <|SYSTEM_TEST := 0w; MS := 0w; SINGLE := 1w|>;
-CH0CONF := spi.regs.CH0CONF with
-<|PHA := 0w; POL := 0w; CLKD := 6w; EPOL := 1w; WL := 7w; 
-TRM := 0w; DPE0 := 1w; DPE1 := 0w; IS := 0w|> |>;
-init :=
-<|sysconfig_mode_done := T; modulctrl_bus_done := T; 
-ch0conf_wordlen_done :=  T; ch0conf_mode_done := T; 
-ch0conf_speed_done := T|> |>)``,
+CH0CONF := <|PHA := 0w; POL := 0w; CLKD := 6w; EPOL := 1w; WL := 7w; 
+TRM := 0w; DPE0 := 1w; DPE1 := 0w; IS := 0w; FORCE := 0w|> |>;
+init := <|sysconfig_mode_done := T; modulctrl_bus_done := T|> |>)``,
 rw [n_tau_tr_def, n_tau_tr_SUC, local_tr_cases, driver_tr_cases, spi_tr_cases, 
 DR_TAU_ENABLE_def, SPI_TAU_ENABLE_def, DR_WR_ENABLE_def, DR_RD_ENABLE_def, GSYM LEFT_EXISTS_AND_THM] >>
 `(dr_write_state dr = dr with <| state := dr_init_read_req;
-dr_init := <|issue_wr_sysconfig := F; issue_wr_modulctrl := F; 
-issue_wr_ch0conf_wl := F; issue_wr_ch0conf_mode := F; issue_wr_ch0conf_speed := F |> |>) /\
+dr_init := <|issue_wr_sysconfig := F; issue_wr_modulctrl := F|> |>) /\
 (dr_write_address dr =  SOME SPI0_SYSCONFIG) /\
 (dr_write_value dr = SOME (0x00000002w:word32))` 
 by rw [dr_write_state_def, dr_write_value_def, dr_write_address_def,
-dr_write_def, dr_write_softreset_def] >>
-rw [] >>
+dr_write_def, dr_write_softreset_def] >> rw [] >>
 `write_SPI_regs SPI0_SYSCONFIG 2w spi =
 spi with <| regs := spi.regs with 
-<| SYSCONFIG := spi.regs.SYSCONFIG with SOFTRESET := 0w;
-SYSSTATUS := 0w |>;
+<| SYSCONFIG := spi.regs.SYSCONFIG with SOFTRESET := 0w; SYSSTATUS := 0w |>;
 state := init_reset;
-init := spi.init with 
-<| sysconfig_mode_done := F; modulctrl_bus_done := F; 
-ch0conf_wordlen_done := F; ch0conf_mode_done := F;
-ch0conf_speed_done := F |> |>` 
+init := <| sysconfig_mode_done := F; modulctrl_bus_done := F |> |>` 
 by rw [write_SPI_regs_def, SPI0_PA_RANGE_def, SPI0_START_def, SPI0_END_def, 
-SPI0_SYSCONFIG_def, write_SYSCONFIG_comb_def, write_SOFTRESET_def] >>
-rw [] >>
-Q.EXISTS_TAC `(dr with <| state := dr_init_read_req; dr_init := <|issue_wr_sysconfig := F; 
-issue_wr_modulctrl := F; issue_wr_ch0conf_wl := F; issue_wr_ch0conf_mode := F; 
-issue_wr_ch0conf_speed := F |> |>, 
+SPI0_SYSCONFIG_def, write_SYSCONFIG_comb_def, write_SOFTRESET_def] >> rw [] >>
+Q.EXISTS_TAC `(dr with <| state := dr_init_read_req; 
+dr_init := <|issue_wr_sysconfig := F; issue_wr_modulctrl := F|> |>, 
 spi_tau_operations (spi with <|state := init_reset; regs := spi.regs with
 <|SYSCONFIG := spi.regs.SYSCONFIG with SOFTRESET := 0w; SYSSTATUS := 0w|>;
-init := <|sysconfig_mode_done := F; modulctrl_bus_done := F;
-ch0conf_wordlen_done := F; ch0conf_mode_done := F; ch0conf_speed_done := F|> |>))` >>
-rw [] >>
+init := <|sysconfig_mode_done := F; modulctrl_bus_done := F|> |>))` >> rw [] >>
 `spi_tau_operations (spi with <|state := init_reset; regs := spi.regs with
 <|SYSCONFIG := spi.regs.SYSCONFIG with SOFTRESET := 0w; SYSSTATUS := 0w|>;
-init := <|sysconfig_mode_done := F; modulctrl_bus_done := F;
-ch0conf_wordlen_done := F; ch0conf_mode_done := F; ch0conf_speed_done := F|> |>) = 
+init := <|sysconfig_mode_done := F; modulctrl_bus_done := F|> |>) = 
 spi with <|regs := spi.regs with 
-<|SYSCONFIG := spi.regs.SYSCONFIG with SOFTRESET := 0w; SYSSTATUS := 1w|>;
-init := <|sysconfig_mode_done := F; modulctrl_bus_done := F;
-ch0conf_wordlen_done := F; ch0conf_mode_done := F; ch0conf_speed_done := F|>;
-state := init_setregs |>` by rw [spi_tau_operations_def, init_reset_op_def] >>
-rw [] >>
-`dr_read (dr with <|state := dr_init_read_req; dr_init := <|issue_wr_sysconfig := F; 
-issue_wr_modulctrl := F; issue_wr_ch0conf_wl := F; issue_wr_ch0conf_mode := F; 
-issue_wr_ch0conf_speed := F |> |>) = dr with <| state := dr_init_check_rep;
+<|SYSCONFIG := spi.regs.SYSCONFIG with SOFTRESET := 0w; SYSSTATUS := 1w;
+CH0CONF := <|PHA := 0w; POL := 0w; CLKD := 0w; EPOL := 0w; WL := 0w;
+TRM := 0w; DPE0 := 0w; DPE1 := 1w; IS := 1w; FORCE := 0w|> |>;
+init := <|sysconfig_mode_done := F; modulctrl_bus_done := F|>;
+state := init_setregs |>` by rw [spi_tau_operations_def, init_reset_op_def] >> rw [] >>
+`dr_read (dr with <|state := dr_init_read_req; 
+dr_init := <|issue_wr_sysconfig := F; issue_wr_modulctrl := F|> |>) = 
+dr with <| state := dr_init_check_rep;
 dr_last_read_ad := SOME SPI0_SYSSTATUS;
-dr_init := <|issue_wr_sysconfig := F; issue_wr_modulctrl := F; 
-issue_wr_ch0conf_wl := F; issue_wr_ch0conf_mode := F; 
-issue_wr_ch0conf_speed := F |> |>` by rw [dr_read_def, dr_read_sysstatus_def] >>
-rw [] >>
+dr_init := <|issue_wr_sysconfig := F; issue_wr_modulctrl := F|> |>` 
+by rw [dr_read_def, dr_read_sysstatus_def] >> rw [] >>
 `(read_SPI_regs_state SPI0_SYSSTATUS (spi with <|state := init_setregs;
 regs := spi.regs with <|SYSCONFIG := spi.regs.SYSCONFIG with SOFTRESET := 0w;
-SYSSTATUS := 1w|>;
-init := <|sysconfig_mode_done := F; modulctrl_bus_done := F;
-ch0conf_wordlen_done := F; ch0conf_mode_done := F; ch0conf_speed_done := F|> |>) = 
+SYSSTATUS := 1w;
+CH0CONF := <|PHA := 0w; POL := 0w; CLKD := 0w; EPOL := 0w; WL := 0w;
+TRM := 0w; DPE0 := 0w; DPE1 := 1w; IS := 1w; FORCE := 0w|> |>;
+init := <|sysconfig_mode_done := F; modulctrl_bus_done := F|> |>) = 
 (spi with <|state := init_setregs;
 regs := spi.regs with <|SYSCONFIG := spi.regs.SYSCONFIG with SOFTRESET := 0w;
-SYSSTATUS := 1w|>;
-init := <|sysconfig_mode_done := F; modulctrl_bus_done := F;
-ch0conf_wordlen_done := F; ch0conf_mode_done := F; ch0conf_speed_done := F|> |>)) /\
+SYSSTATUS := 1w;
+CH0CONF := <|PHA := 0w; POL := 0w; CLKD := 0w; EPOL := 0w; WL := 0w;
+TRM := 0w; DPE0 := 0w; DPE1 := 1w; IS := 1w; FORCE := 0w|> |>;
+init := <|sysconfig_mode_done := F; modulctrl_bus_done := F|> |>)) /\
 (read_SPI_regs_value SPI0_SYSSTATUS (spi with <|state := init_setregs;
 regs := spi.regs with <|SYSCONFIG := spi.regs.SYSCONFIG with SOFTRESET := 0w;
-SYSSTATUS := 1w|>;
-init := <|sysconfig_mode_done := F; modulctrl_bus_done := F;
-ch0conf_wordlen_done := F; ch0conf_mode_done := F; ch0conf_speed_done := F|> |>) = 1w:word32)` 
+SYSSTATUS := 1w;
+CH0CONF := <|PHA := 0w; POL := 0w; CLKD := 0w; EPOL := 0w; WL := 0w;
+TRM := 0w; DPE0 := 0w; DPE1 := 1w; IS := 1w; FORCE := 0w|> |>;
+init := <|sysconfig_mode_done := F; modulctrl_bus_done := F|> |>) = 1w:word32)` 
 by rw [read_SPI_regs_state_def, read_SPI_regs_value_def, read_SPI_regs_def, SPI0_SYSSTATUS_def,
-SPI0_PA_RANGE_def, SPI0_START_def, SPI0_END_def, SPI0_SYSCONFIG_def] >>
-rw [] >>
+SPI0_PA_RANGE_def, SPI0_START_def, SPI0_END_def, SPI0_SYSCONFIG_def] >> rw [] >>
 `dr_check (dr with <|state := dr_init_check_rep; 
 dr_last_read_ad := SOME SPI0_SYSSTATUS;
 dr_last_read_v := SOME 1w;
-dr_init := <|issue_wr_sysconfig := F; issue_wr_modulctrl := F; issue_wr_ch0conf_wl := F; 
-issue_wr_ch0conf_mode := F; issue_wr_ch0conf_speed := F |> |>) SPI0_SYSSTATUS 1w =
+dr_init := <|issue_wr_sysconfig := F; issue_wr_modulctrl := F|> |>) SPI0_SYSSTATUS 1w =
 dr with <|state := dr_init_setting; 
 dr_last_read_ad := SOME SPI0_SYSSTATUS;
 dr_last_read_v := SOME 1w;
-dr_init := <|issue_wr_sysconfig := F; issue_wr_modulctrl := F; issue_wr_ch0conf_wl := F; 
-issue_wr_ch0conf_mode := F; issue_wr_ch0conf_speed := F |> |>` 
-by rw [dr_check_def, dr_check_sysstatus_def] >>
-rw [] >>
+dr_init := <|issue_wr_sysconfig := F; issue_wr_modulctrl := F|> |>` 
+by rw [dr_check_def, dr_check_sysstatus_def] >> rw [] >>
 `(dr_write_state (dr with <|state := dr_init_setting; 
 dr_last_read_ad := SOME SPI0_SYSSTATUS;
 dr_last_read_v := SOME 1w;
-dr_init := <|issue_wr_sysconfig := F; issue_wr_modulctrl := F; issue_wr_ch0conf_wl := F; 
-issue_wr_ch0conf_mode := F; issue_wr_ch0conf_speed := F |> |>) = 
+dr_init := <|issue_wr_sysconfig := F; issue_wr_modulctrl := F|> |>) = 
 dr with <| state := dr_init_setting;
 dr_last_read_ad := SOME SPI0_SYSSTATUS;
 dr_last_read_v := SOME 1w;
-dr_init := <|issue_wr_sysconfig := T; issue_wr_modulctrl := F; 
-issue_wr_ch0conf_wl := F; issue_wr_ch0conf_mode := F; 
-issue_wr_ch0conf_speed := F |> |>) /\
+dr_init := <|issue_wr_sysconfig := T; issue_wr_modulctrl := F|> |>) /\
 (dr_write_address (dr with <|state := dr_init_setting; 
 dr_last_read_ad := SOME SPI0_SYSSTATUS;
 dr_last_read_v := SOME 1w;
-dr_init := <|issue_wr_sysconfig := F; issue_wr_modulctrl := F; issue_wr_ch0conf_wl := F; 
-issue_wr_ch0conf_mode := F; issue_wr_ch0conf_speed := F |> |>) = SOME SPI0_SYSCONFIG) /\
+dr_init := <|issue_wr_sysconfig := F; issue_wr_modulctrl := F|> |>) = SOME SPI0_SYSCONFIG) /\
 (dr_write_value (dr with <|state := dr_init_setting; 
 dr_last_read_ad := SOME SPI0_SYSSTATUS;
 dr_last_read_v := SOME 1w;
-dr_init := <|issue_wr_sysconfig := F; issue_wr_modulctrl := F; issue_wr_ch0conf_wl := F; 
-issue_wr_ch0conf_mode := F; issue_wr_ch0conf_speed := F |> |>) = SOME (0x00000011w:word32))` 
+dr_init := <|issue_wr_sysconfig := F; issue_wr_modulctrl := F|> |>) = SOME (0x00000011w:word32))` 
 by rw [dr_write_state_def, dr_write_address_def, dr_write_value_def,
-dr_write_def, dr_write_sysconfig_def] >>
-rw [] >>
+dr_write_def, dr_write_sysconfig_def] >> rw [] >>
 `write_SPI_regs SPI0_SYSCONFIG 17w (spi with <|state := init_setregs;
 regs := spi.regs with <|SYSCONFIG := spi.regs.SYSCONFIG with SOFTRESET := 0w;
-SYSSTATUS := 1w|>;
-init := <|sysconfig_mode_done := F; modulctrl_bus_done := F;
-ch0conf_wordlen_done := F; ch0conf_mode_done := F; ch0conf_speed_done := F|> |>) = 
+SYSSTATUS := 1w;
+CH0CONF := <|PHA := 0w; POL := 0w; CLKD := 0w; EPOL := 0w; WL := 0w;
+TRM := 0w; DPE0 := 0w; DPE1 := 1w; IS := 1w; FORCE := 0w|> |>;
+init := <|sysconfig_mode_done := F; modulctrl_bus_done := F|> |>) = 
 (spi with <|state := init_setregs; 
 regs := spi.regs with 
 <|SYSSTATUS := 1w;
+CH0CONF := <|PHA := 0w; POL := 0w; CLKD := 0w; EPOL := 0w; WL := 0w;
+TRM := 0w; DPE0 := 0w; DPE1 := 1w; IS := 1w; FORCE := 0w|>;
 SYSCONFIG := <|SIDLEMODE := 2w; SOFTRESET := 0w; AUTOIDLE := 1w|> |>; 
-init := <|sysconfig_mode_done := T; modulctrl_bus_done := F;
-ch0conf_wordlen_done := F; ch0conf_mode_done := F; ch0conf_speed_done := F|> |>)`
+init := <|sysconfig_mode_done := T; modulctrl_bus_done := F|> |>)`
 by rw [write_SPI_regs_def, SPI0_PA_RANGE_def, SPI0_START_def, SPI0_END_def, 
-SPI0_SYSCONFIG_def, write_SYSCONFIG_comb_def, write_SYSCONFIG_def] >>
-rw [] >>
+SPI0_SYSCONFIG_def, write_SYSCONFIG_comb_def, write_SYSCONFIG_def] >> rw [] >>
 `(dr_write_state (dr with <| state := dr_init_setting;
 dr_last_read_ad := SOME SPI0_SYSSTATUS;
 dr_last_read_v := SOME 1w;
-dr_init := <|issue_wr_sysconfig := T; issue_wr_modulctrl := F; 
-issue_wr_ch0conf_wl := F; issue_wr_ch0conf_mode := F; 
-issue_wr_ch0conf_speed := F |> |>) = 
+dr_init := <|issue_wr_sysconfig := T; issue_wr_modulctrl := F|> |>) = 
 dr with <|state := dr_init_setting;
 dr_last_read_ad := SOME SPI0_SYSSTATUS;
 dr_last_read_v := SOME 1w;
 dr_init := dr.dr_init with 
-<|issue_wr_sysconfig := T ; issue_wr_modulctrl := T;
-issue_wr_ch0conf_wl := F; issue_wr_ch0conf_mode := F; 
-issue_wr_ch0conf_speed := F |> |>) /\
+<|issue_wr_sysconfig := T ; issue_wr_modulctrl := T|> |>) /\
 (dr_write_address (dr with <| state := dr_init_setting;
 dr_last_read_ad := SOME SPI0_SYSSTATUS;
 dr_last_read_v := SOME 1w;
-dr_init := <|issue_wr_sysconfig := T; issue_wr_modulctrl := F; 
-issue_wr_ch0conf_wl := F; issue_wr_ch0conf_mode := F; 
-issue_wr_ch0conf_speed := F |> |>) = SOME SPI0_MODULCTRL) /\
+dr_init := <|issue_wr_sysconfig := T; issue_wr_modulctrl := F|> |>) = SOME SPI0_MODULCTRL) /\
 (dr_write_value (dr with <| state := dr_init_setting;
 dr_last_read_ad := SOME SPI0_SYSSTATUS;
 dr_last_read_v := SOME 1w;
-dr_init := <|issue_wr_sysconfig := T; issue_wr_modulctrl := F; 
-issue_wr_ch0conf_wl := F; issue_wr_ch0conf_mode := F; 
-issue_wr_ch0conf_speed := F |> |>) = SOME (0x00000001w))` 
+dr_init := <|issue_wr_sysconfig := T; issue_wr_modulctrl := F|> |>) = SOME (0x00000001w))` 
 by fs [dr_write_state_def, dr_write_address_def, dr_write_value_def,
-dr_write_def, dr_write_modulctrl_def] >>
-rw [] >>
+dr_write_def, dr_write_modulctrl_def] >> rw [] >>
+`~(0w:word5 >+ 2w:word5)` by EVAL_TAC >>
 `write_SPI_regs SPI0_MODULCTRL 1w 
 (spi with <|state := init_setregs; 
 regs := spi.regs with 
 <|SYSCONFIG := <|SIDLEMODE := 2w; SOFTRESET := 0w; AUTOIDLE := 1w|>;
-SYSSTATUS := 1w |>; 
-init := <|sysconfig_mode_done := T; modulctrl_bus_done := F;
-ch0conf_wordlen_done := F; ch0conf_mode_done := F; ch0conf_speed_done := F|> |>) =
+SYSSTATUS := 1w;
+CH0CONF := <|PHA := 0w; POL := 0w; CLKD := 0w; EPOL := 0w; WL := 0w; 
+TRM := 0w; DPE0 := 0w; DPE1 := 1w; IS := 1w; FORCE := 0w|> |>; 
+init := <|sysconfig_mode_done := T; modulctrl_bus_done := F |> |>) =
 (spi with <|state := init_setregs; regs := spi.regs with
 <|SYSCONFIG := <|SIDLEMODE := 2w; SOFTRESET := 0w; AUTOIDLE := 1w|>;
 SYSSTATUS := 1w;
-MODULCTRL := <|SYSTEM_TEST := 0w; MS := 0w; SINGLE := 1w|> |>;
-init := spi.init with <|sysconfig_mode_done := T; modulctrl_bus_done := T;
-ch0conf_wordlen_done := F; ch0conf_mode_done := F; ch0conf_speed_done := F|> |>)`
+MODULCTRL := <|SYSTEM_TEST := 0w; MS := 0w; SINGLE := 1w|>;
+CH0CONF := <|PHA := 0w; POL := 0w; CLKD := 0w; EPOL := 0w; WL := 0w; 
+TRM := 0w; DPE0 := 0w; DPE1 := 1w; IS := 1w; FORCE := 0w|> |>;
+init := <|sysconfig_mode_done := T; modulctrl_bus_done := T|> |>)`
 by rw [write_SPI_regs_def, SPI0_PA_RANGE_def, SPI0_START_def, SPI0_END_def, 
-SPI0_SYSCONFIG_def, SPI0_MODULCTRL_def, write_MODULCTRL_def] >>
-rw [] >>
+SPI0_SYSCONFIG_def, SPI0_MODULCTRL_def, write_MODULCTRL_def] >> fs [] >>
 `(dr_write_state (dr with <|state := dr_init_setting;
 dr_last_read_ad := SOME SPI0_SYSSTATUS; dr_last_read_v := SOME 1w;
-dr_init := 
-<|issue_wr_sysconfig := T ; issue_wr_modulctrl := T;
-issue_wr_ch0conf_wl := F; issue_wr_ch0conf_mode := F; 
-issue_wr_ch0conf_speed := F |> |>) = 
-dr with <|state := dr_init_setting;
+dr_init := <|issue_wr_sysconfig := T; issue_wr_modulctrl := T|> |>) = 
+dr with <|state := dr_ready;
 dr_last_read_ad := SOME SPI0_SYSSTATUS; dr_last_read_v := SOME 1w;
-dr_init :=
-<|issue_wr_sysconfig := T; issue_wr_modulctrl := T; issue_wr_ch0conf_wl := T;
-issue_wr_ch0conf_mode := F; issue_wr_ch0conf_speed := F |> |>) /\
+dr_init := <|issue_wr_sysconfig := T; issue_wr_modulctrl := T|> |>) /\
 (dr_write_address (dr with <|state := dr_init_setting;
 dr_last_read_ad := SOME SPI0_SYSSTATUS; dr_last_read_v := SOME 1w;
-dr_init := 
-<|issue_wr_sysconfig := T ; issue_wr_modulctrl := T;
-issue_wr_ch0conf_wl := F; issue_wr_ch0conf_mode := F; 
-issue_wr_ch0conf_speed := F |> |>) = 
+dr_init := <|issue_wr_sysconfig := T ; issue_wr_modulctrl := T|> |>) = 
 SOME SPI0_CH0CONF) /\
 (dr_write_value (dr with <|state := dr_init_setting;
 dr_last_read_ad := SOME SPI0_SYSSTATUS; dr_last_read_v := SOME 1w;
-dr_init := 
-<|issue_wr_sysconfig := T ; issue_wr_modulctrl := T;
-issue_wr_ch0conf_wl := F; issue_wr_ch0conf_mode := F; 
-issue_wr_ch0conf_speed := F |> |>) = 
-SOME (0x00000380w:word32))` 
+dr_init := <|issue_wr_sysconfig := T ; issue_wr_modulctrl := T|> |>) = 
+SOME (66520w:word32))` 
 by fs [dr_write_state_def, dr_write_address_def, dr_write_value_def,
-dr_write_def, dr_write_ch0conf_wl_def] >>
-rw [] >>
-`7w:word5 >+ 2w:word5` by EVAL_TAC >>
-`write_SPI_regs SPI0_CH0CONF 896w 
-(spi with <|state := init_setregs; regs := spi.regs with
-<|SYSCONFIG := <|SIDLEMODE := 2w; SOFTRESET := 0w; AUTOIDLE := 1w|>;
-SYSSTATUS := 1w;
-MODULCTRL := <|SYSTEM_TEST := 0w; MS := 0w; SINGLE := 1w|> |>;
-init := <|sysconfig_mode_done := T; modulctrl_bus_done := T;
-ch0conf_wordlen_done := F; ch0conf_mode_done := F; ch0conf_speed_done := F|> |>) = 
-(spi with <|state := init_setregs; 
+dr_write_def, dr_write_ch0conf_init_def] >> fs [] >>
+`(spi with <|state := init_setregs;
 regs := spi.regs with <|
-SYSCONFIG := <|SIDLEMODE := 2w; SOFTRESET := 0w; AUTOIDLE := 1w|>;
+SYSCONFIG := <|SIDLEMODE := 2w; SOFTRESET := 0w; AUTOIDLE := 1w|>; 
 SYSSTATUS := 1w;
 MODULCTRL := <|SYSTEM_TEST := 0w; MS := 0w; SINGLE := 1w|>;
-CH0CONF := spi.regs.CH0CONF with WL := 7w |>;
-init :=  
-<|ch0conf_wordlen_done := T; sysconfig_mode_done := T; modulctrl_bus_done := T;
-ch0conf_mode_done := F; ch0conf_speed_done := F |> |>)`
-by fs [write_SPI_regs_def, SPI0_CH0CONF_def, SPI0_PA_RANGE_def, 
-SPI0_START_def, SPI0_END_def, SPI0_SYSCONFIG_def, SPI0_MODULCTRL_def, 
-SPI0_TX0_def, write_CH0CONF_comb_def, write_CH0CONF_WL_def] >>
-rw [] >>
-rw [dr_write_state_def, dr_write_address_def, dr_write_value_def,
-dr_write_def, dr_write_ch0conf_speed_def, dr_write_ch0conf_mode_def] >>
-fs [write_SPI_regs_def, SPI0_CH0CONF_def, SPI0_PA_RANGE_def, 
-SPI0_START_def, SPI0_END_def, SPI0_SYSCONFIG_def, 
-SPI0_MODULCTRL_def, SPI0_TX0_def, write_CH0CONF_comb_def, 
-write_CH0CONF_def, write_CH0CONF_speed_def]);
+CH0CONF := <|PHA := 0w; POL := 0w; CLKD := 0w; EPOL := 0w; WL := 0w;
+TRM := 0w; DPE0 := 0w; DPE1 := 1w; IS := 1w; FORCE := 0w|> |>;
+init := <|sysconfig_mode_done := T; modulctrl_bus_done := T|> |>).regs.CH0CONF.IS = 1w` by fs [] >>
+`(19 >< 19) (66520w:word32):word1 <> ((spi with <|state := init_setregs;
+regs := spi.regs with <|
+SYSCONFIG := <|SIDLEMODE := 2w; SOFTRESET := 0w; AUTOIDLE := 1w|>; 
+SYSSTATUS := 1w;
+MODULCTRL := <|SYSTEM_TEST := 0w; MS := 0w; SINGLE := 1w|>;
+CH0CONF := <|PHA := 0w; POL := 0w; CLKD := 0w; EPOL := 0w; WL := 0w;
+TRM := 0w; DPE0 := 0w; DPE1 := 1w; IS := 1w; FORCE := 0w|> |>;
+init := <|sysconfig_mode_done := T; modulctrl_bus_done := T|> |>).regs.CH0CONF.IS)` 
+by FULL_SIMP_TAC (std_ss++WORD_ss) [] >>
+`ch0conf_changed (66520w:word32) 
+(spi with <|state := init_setregs;
+regs := spi.regs with <|
+SYSCONFIG := <|SIDLEMODE := 2w; SOFTRESET := 0w; AUTOIDLE := 1w|>; 
+SYSSTATUS := 1w;
+MODULCTRL := <|SYSTEM_TEST := 0w; MS := 0w; SINGLE := 1w|>;
+CH0CONF := <|PHA := 0w; POL := 0w; CLKD := 0w; EPOL := 0w; WL := 0w;
+TRM := 0w; DPE0 := 0w; DPE1 := 1w; IS := 1w; FORCE := 0w|> |>;
+init := <|sysconfig_mode_done := T; modulctrl_bus_done := T|> |>)` by fs [ch0conf_changed_def] >>
+rw [write_SPI_regs_def, SPI0_CH0CONF_def, SPI0_PA_RANGE_def, SPI0_START_def, 
+SPI0_END_def, SPI0_SYSCONFIG_def, SPI0_MODULCTRL_def, SPI0_TX0_def, 
+write_CH0CONF_comb_def, write_CH0CONF_init_def] >>
+`7w:word5 >+ 2w:word5` by EVAL_TAC >>
+fs [ref_rel_def, IS_STATE_REL_def]);
 
 (* (dr',spi') exists for init *)
 val abs1_comb_hold_ref_rel_tau_comb_init = store_thm("abs1_comb_hold_ref_rel_tau_comb_init",
@@ -1402,8 +1010,7 @@ val abs1_comb_hold_ref_rel_tau_comb_init = store_thm("abs1_comb_hold_ref_rel_tau
 (ref_rel (ds_abs1 with state := abs1_ready) (dr', spi'))) \/
 (?n dr' spi'. (n_tau_tr n local_tr (dr,spi) tau (dr',spi')) /\ 
 (ref_rel (ds_abs1 with state := abs1_ready) (dr',spi')))``,
-rw [] >>
-`IS_STATE_REL ds_abs1 dr spi` by fs [ref_rel_def] >>
+rw [] >> `IS_STATE_REL ds_abs1 dr spi` by fs [ref_rel_def] >>
 `(dr.state = dr_init_setting /\ spi.state = init_setregs) \/
 (dr.state = dr_init_read_req /\ spi.state = init_setregs) \/
 (dr.state = dr_init_check_rep /\ spi.state = init_setregs) \/
@@ -1413,80 +1020,48 @@ rw [] >>
 (dr.state = dr_init_idle /\ spi.state = spi_ready)` by fs [IS_STATE_REL_def] >|[
 (* dr_init_setting and init_setregs *)
 `(dr.dr_init.issue_wr_sysconfig = spi.init.sysconfig_mode_done) /\
-(dr.dr_init.issue_wr_modulctrl = spi.init.modulctrl_bus_done) /\
-(dr.dr_init.issue_wr_ch0conf_wl = spi.init.ch0conf_wordlen_done) /\
-(dr.dr_init.issue_wr_ch0conf_mode = spi.init.ch0conf_mode_done) /\
-(dr.dr_init.issue_wr_ch0conf_speed = spi.init.ch0conf_speed_done)`  
+(dr.dr_init.issue_wr_modulctrl = spi.init.modulctrl_bus_done)`  
 by fs [ref_rel_def] >>
 rw [local_tr_cases, driver_tr_cases, spi_tr_cases, DR_TAU_ENABLE_def, 
 SPI_TAU_ENABLE_def, DR_WR_ENABLE_def, DR_RD_ENABLE_def] >> 
 REVERSE (rw [dr_write_state_def, dr_write_address_def, dr_write_value_def, dr_write_def]) >|[
-(* ch0conf_speed *)
+(* ch0conf *)
 DISJ1_TAC >>
-rw [dr_write_ch0conf_speed_def, write_SPI_regs_def, SPI0_CH0CONF_def, 
-SPI0_PA_RANGE_def, SPI0_START_def, SPI0_END_def, SPI0_SYSCONFIG_def, 
-SPI0_MODULCTRL_def, SPI0_TX0_def, write_CH0CONF_comb_def] >>
-fs [write_CH0CONF_speed_def, ref_rel_def, IS_STATE_REL_def],
-(* ch0conf_mode *)
-`~ dr.dr_init.issue_wr_ch0conf_speed` by fs [ref_rel_def] >>
+rw [dr_write_ch0conf_init_def] >>
+`spi.regs.CH0CONF.IS = 1w /\ spi.regs.CH0CONF.FORCE = 0w` by fs [ref_rel_def] >>
+`(19 >< 19) (66520w:word32):word1 <> spi.regs.CH0CONF.IS` 
+by FULL_SIMP_TAC (std_ss++WORD_ss) [] >>
+`ch0conf_changed (66520w:word32) spi` by fs [ch0conf_changed_def] >>
+rw [write_SPI_regs_def, SPI0_CH0CONF_def, SPI0_PA_RANGE_def, SPI0_START_def, 
+SPI0_END_def, SPI0_SYSCONFIG_def, SPI0_MODULCTRL_def, SPI0_TX0_def, 
+write_CH0CONF_comb_def, write_CH0CONF_init_def] >>
+`7w:word5 >+ 2w:word5` by EVAL_TAC >>
+fs [ref_rel_def, IS_STATE_REL_def],
+(* modulctrl *)
 DISJ2_TAC >>
+`spi.regs.CH0CONF.IS = 1w /\ spi.regs.CH0CONF.FORCE = 0w /\ spi.regs.CH0CONF.WL = 0w` 
+by fs [ref_rel_def] >>
+`~dr.dr_init.issue_wr_modulctrl /\ dr.dr_init.issue_wr_sysconfig` by fs [ref_rel_def] >>
 Q.EXISTS_TAC `SUC 0` >>
 Q.EXISTS_TAC `dr with <| state := dr_ready; 
-dr_init := dr.dr_init with
-<| issue_wr_ch0conf_mode := T; issue_wr_ch0conf_speed := T |> |>` >>
-Q.EXISTS_TAC `spi with <|state := spi_ready;
-regs := spi.regs with CH0CONF := spi.regs.CH0CONF with
-<|PHA := 0w; POL := 0w; CLKD := 6w; EPOL := 1w; TRM := 0w;
-DPE0 := 1w; DPE1 := 0w; IS := 0w|>;
-init := spi.init with <|ch0conf_mode_done := T; ch0conf_speed_done := T|> |>` >>
-fs [n_tau_tr_dr_init_setting_1, ref_rel_def, IS_STATE_REL_def],
-(* ch0conf_wl *)
-`~ dr.dr_init.issue_wr_ch0conf_speed /\
- ~ dr.dr_init.issue_wr_ch0conf_mode` by fs [ref_rel_def] >>
-DISJ2_TAC >>
-Q.EXISTS_TAC `SUC 1` >>
-Q.EXISTS_TAC `dr with <| state := dr_ready; 
-dr_init := dr.dr_init with <| issue_wr_ch0conf_mode := T; 
-issue_wr_ch0conf_speed := T; issue_wr_ch0conf_wl := T |> |>` >> 
-Q.EXISTS_TAC `spi with <|state := spi_ready;
-regs := spi.regs with CH0CONF := spi.regs.CH0CONF with
-<|PHA := 0w; POL := 0w; CLKD := 6w; EPOL := 1w; WL := 7w; 
-TRM := 0w; DPE0 := 1w; DPE1 := 0w; IS := 0w|>;
-init := spi.init with <|ch0conf_mode_done := T; ch0conf_speed_done := T;
-ch0conf_wordlen_done :=  T |> |>` >>
-fs [n_tau_tr_dr_init_setting_2, ref_rel_def, IS_STATE_REL_def],
-(* modulctrl *)
-`~ dr.dr_init.issue_wr_ch0conf_wl /\
- ~ dr.dr_init.issue_wr_ch0conf_speed /\
- ~ dr.dr_init.issue_wr_ch0conf_mode` by fs [ref_rel_def] >>
-DISJ2_TAC >>
-Q.EXISTS_TAC `SUC 2` >>
-Q.EXISTS_TAC `dr with <| state := dr_ready; 
-dr_init := dr.dr_init with
-<| issue_wr_modulctrl := T; issue_wr_ch0conf_wl := T; 
-issue_wr_ch0conf_mode := T; issue_wr_ch0conf_speed := T |> |>` >> 
+dr_init := dr.dr_init with issue_wr_modulctrl := T |>` >> 
 Q.EXISTS_TAC `spi with <|state := spi_ready;
 regs := spi.regs with <| 
 MODULCTRL := <|SYSTEM_TEST := 0w; MS := 0w; SINGLE := 1w |>;
 CH0CONF := spi.regs.CH0CONF with
 <|PHA := 0w; POL := 0w; CLKD := 6w; EPOL := 1w; WL := 7w; 
 TRM := 0w; DPE0 := 1w; DPE1 := 0w; IS := 0w|> |>;
-init := spi.init with 
-<|modulctrl_bus_done := T; ch0conf_wordlen_done :=  T; 
-ch0conf_mode_done := T; ch0conf_speed_done := T|> |>` >>
-fs [n_tau_tr_dr_init_setting_3, ref_rel_def, IS_STATE_REL_def],
+init := spi.init with modulctrl_bus_done := T |>` >>
+fs [n_tau_tr_dr_init_setting_1, ref_rel_def, IS_STATE_REL_def],
 (* sysconfig_mode *)
-`~ dr.dr_init.issue_wr_modulctrl /\
- ~ dr.dr_init.issue_wr_ch0conf_wl /\
- ~ dr.dr_init.issue_wr_ch0conf_speed /\
- ~ dr.dr_init.issue_wr_ch0conf_mode` by fs [ref_rel_def] >>
 DISJ2_TAC >>
-Q.EXISTS_TAC `SUC 3` >>
+`spi.regs.CH0CONF.IS = 1w /\ spi.regs.CH0CONF.FORCE = 0w /\ spi.regs.CH0CONF.WL = 0w` 
+by fs [ref_rel_def] >>
+`~dr.dr_init.issue_wr_modulctrl /\ ~dr.dr_init.issue_wr_sysconfig /\
+~spi.init.modulctrl_bus_done` by fs [ref_rel_def] >>
+Q.EXISTS_TAC `SUC 1` >>
 Q.EXISTS_TAC `dr with <| state := dr_ready; 
-dr_init := 
-<| issue_wr_sysconfig := T;
-issue_wr_modulctrl := T; issue_wr_ch0conf_wl := T; 
-issue_wr_ch0conf_mode := T; issue_wr_ch0conf_speed := T |> |>` >> 
+dr_init := <| issue_wr_sysconfig := T; issue_wr_modulctrl := T |> |>` >> 
 Q.EXISTS_TAC `spi with <|state := spi_ready;
 regs := spi.regs with 
 <| SYSCONFIG := spi.regs.SYSCONFIG with <|SIDLEMODE := 2w; AUTOIDLE := 1w|>;
@@ -1494,188 +1069,132 @@ MODULCTRL := <|SYSTEM_TEST := 0w; MS := 0w; SINGLE := 1w|>;
 CH0CONF := spi.regs.CH0CONF with
 <|PHA := 0w; POL := 0w; CLKD := 6w; EPOL := 1w; WL := 7w; 
 TRM := 0w; DPE0 := 1w; DPE1 := 0w; IS := 0w|> |>;
-init :=  
-<|sysconfig_mode_done := T; modulctrl_bus_done := T; 
-ch0conf_wordlen_done :=  T; ch0conf_mode_done := T; 
-ch0conf_speed_done := T|> |>` >>
-fs [n_tau_tr_dr_init_setting_4, ref_rel_def, IS_STATE_REL_def]],
+init :=  <|sysconfig_mode_done := T; modulctrl_bus_done := T |> |>` >>
+fs [n_tau_tr_dr_init_setting_2, ref_rel_def, IS_STATE_REL_def]],
 (* dr_init_read_req and init_setregs *)
-`spi.regs.SYSSTATUS = 1w` by fs [ref_rel_def] >>
-`~ dr.dr_init.issue_wr_sysconfig /\ ~ dr.dr_init.issue_wr_modulctrl /\
-~ dr.dr_init.issue_wr_ch0conf_wl /\ ~ dr.dr_init.issue_wr_ch0conf_mode /\
-~ dr.dr_init.issue_wr_ch0conf_speed /\ ~ spi.init.sysconfig_mode_done /\ 
-~ spi.init.modulctrl_bus_done /\ ~ spi.init.ch0conf_wordlen_done /\ 
-~ spi.init.ch0conf_mode_done /\ ~ spi.init.ch0conf_speed_done` by fs [ref_rel_def] >>
+`spi.regs.SYSSTATUS = 1w /\ spi.regs.CH0CONF.WL = 0w /\
+spi.regs.CH0CONF.IS = 1w /\ spi.regs.CH0CONF.FORCE = 0w` by fs [ref_rel_def] >>
+`~ dr.dr_init.issue_wr_sysconfig /\ ~ dr.dr_init.issue_wr_modulctrl /\ 
+~ spi.init.sysconfig_mode_done /\ ~ spi.init.modulctrl_bus_done` by fs [ref_rel_def] >>
+DISJ2_TAC >>
+Q.EXISTS_TAC `SUC 3` >>
+Q.EXISTS_TAC `dr with <| state := dr_ready; 
+dr_last_read_ad := SOME SPI0_SYSSTATUS;
+dr_last_read_v := SOME 1w;
+dr_init := 
+<| issue_wr_sysconfig := T; issue_wr_modulctrl := T |> |>` >>
+Q.EXISTS_TAC `spi with <|state := spi_ready;
+regs := spi.regs with 
+<| SYSCONFIG := spi.regs.SYSCONFIG with <|SIDLEMODE := 2w; AUTOIDLE := 1w|>;
+MODULCTRL := <|SYSTEM_TEST := 0w; MS := 0w; SINGLE := 1w|>;
+CH0CONF := spi.regs.CH0CONF with
+<|PHA := 0w; POL := 0w; CLKD := 6w; EPOL := 1w; WL := 7w; 
+TRM := 0w; DPE0 := 1w; DPE1 := 0w; IS := 0w|> |>;
+init :=
+<|sysconfig_mode_done := T; modulctrl_bus_done := T |> |>` >>
+fs [n_tau_tr_dr_init_read_req_4, ref_rel_def, IS_STATE_REL_def],
+(* dr_init_check_rep and init_set_regs *)
+`~ dr.dr_init.issue_wr_sysconfig /\ ~ dr.dr_init.issue_wr_modulctrl /\ 
+~ spi.init.sysconfig_mode_done /\ ~ spi.init.modulctrl_bus_done` by fs [ref_rel_def] >>
+`dr.dr_last_read_ad = SOME SPI0_SYSSTATUS /\ ?v. dr.dr_last_read_v = SOME v` by fs [ref_rel_def] >>
+`spi.regs.SYSSTATUS = 1w /\ spi.regs.CH0CONF.WL = 0w /\
+spi.regs.CH0CONF.IS = 1w /\ spi.regs.CH0CONF.FORCE = 0w` by fs [ref_rel_def] >>
+DISJ2_TAC >>
+Cases_on `(0 >< 0) v:word1 = 1w` >-
+((* the store value of sysstatus  is 1w *)
+Q.EXISTS_TAC `SUC 2` >>
+Q.EXISTS_TAC `dr with <| state := dr_ready; 
+dr_init := <| issue_wr_sysconfig := T; issue_wr_modulctrl := T|> |>` >>
+Q.EXISTS_TAC `spi with <|state := spi_ready;
+regs := spi.regs with 
+<| SYSCONFIG := spi.regs.SYSCONFIG with <|SIDLEMODE := 2w; AUTOIDLE := 1w|>;
+MODULCTRL := <|SYSTEM_TEST := 0w; MS := 0w; SINGLE := 1w|>;
+CH0CONF := spi.regs.CH0CONF with
+<|PHA := 0w; POL := 0w; CLKD := 6w; EPOL := 1w; WL := 7w; 
+TRM := 0w; DPE0 := 1w; DPE1 := 0w; IS := 0w|> |>;
+init := <|sysconfig_mode_done := T; modulctrl_bus_done := T|> |>` >>
+fs [n_tau_tr_dr_init_check_rep_3, ref_rel_def, IS_STATE_REL_def]) >>
+(* the store value of sysstatus is 0w *)
+`(0 >< 0) v:word1 = 0w` by rw [word1_not_1w_eq_0w] >>
+Q.EXISTS_TAC `SUC 4` >>
+Q.EXISTS_TAC `dr with <| state := dr_ready; 
+dr_last_read_ad := SOME SPI0_SYSSTATUS;
+dr_last_read_v := SOME 1w;
+dr_init := <|issue_wr_sysconfig := T; issue_wr_modulctrl := T|> |>` >>
+Q.EXISTS_TAC `spi with <|state := spi_ready;
+regs := spi.regs with 
+<| SYSCONFIG := spi.regs.SYSCONFIG with <|SIDLEMODE := 2w; AUTOIDLE := 1w|>;
+MODULCTRL := <|SYSTEM_TEST := 0w; MS := 0w; SINGLE := 1w|>;
+CH0CONF := spi.regs.CH0CONF with
+<|PHA := 0w; POL := 0w; CLKD := 6w; EPOL := 1w; WL := 7w; 
+TRM := 0w; DPE0 := 1w; DPE1 := 0w; IS := 0w|> |>;
+init := <|sysconfig_mode_done := T; modulctrl_bus_done := T|> |>` >>
+fs [n_tau_tr_dr_init_check_rep_5, ref_rel_def, IS_STATE_REL_def],
+(* dr_init_read_req and init_reset *)
+`~ dr.dr_init.issue_wr_sysconfig /\ ~ dr.dr_init.issue_wr_modulctrl /\ 
+~ spi.init.sysconfig_mode_done /\ ~ spi.init.modulctrl_bus_done ` by fs [ref_rel_def] >>
+DISJ2_TAC >>
+Q.EXISTS_TAC `SUC 4` >>
+Q.EXISTS_TAC `dr with <| state := dr_ready; 
+dr_last_read_ad := SOME SPI0_SYSSTATUS;
+dr_last_read_v := SOME 1w;
+dr_init := <| issue_wr_sysconfig := T; issue_wr_modulctrl := T|> |>` >>
+Q.EXISTS_TAC `spi with <|state := spi_ready;
+regs := spi.regs with 
+<| SYSCONFIG := spi.regs.SYSCONFIG with <|SIDLEMODE := 2w; AUTOIDLE := 1w|>;
+SYSSTATUS := 1w;
+MODULCTRL := <|SYSTEM_TEST := 0w; MS := 0w; SINGLE := 1w|>;
+CH0CONF := 
+<|PHA := 0w; POL := 0w; CLKD := 6w; EPOL := 1w; WL := 7w; 
+TRM := 0w; DPE0 := 1w; DPE1 := 0w; IS := 0w; FORCE := 0w|> |>;
+init := <|sysconfig_mode_done := T; modulctrl_bus_done := T|> |>` >>
+fs [n_tau_tr_dr_init_read_req_5, ref_rel_def, IS_STATE_REL_def],
+(* dr_init_check_rep and init_reset *)
+`~ dr.dr_init.issue_wr_sysconfig /\ ~ dr.dr_init.issue_wr_modulctrl /\ 
+~ spi.init.sysconfig_mode_done /\ ~ spi.init.modulctrl_bus_done` by fs [ref_rel_def] >>
+`dr.dr_last_read_ad = SOME SPI0_SYSSTATUS /\ ?v. dr.dr_last_read_v = SOME v` by fs [ref_rel_def] >>
+`(0 >< 0) v:word1 = 0w` by fs [ref_rel_def] >>
 DISJ2_TAC >>
 Q.EXISTS_TAC `SUC 5` >>
 Q.EXISTS_TAC `dr with <| state := dr_ready; 
 dr_last_read_ad := SOME SPI0_SYSSTATUS;
 dr_last_read_v := SOME 1w;
-dr_init := 
-<| issue_wr_sysconfig := T; issue_wr_modulctrl := T; 
-issue_wr_ch0conf_wl := T; issue_wr_ch0conf_mode := T; 
-issue_wr_ch0conf_speed := T |> |>` >>
-Q.EXISTS_TAC `spi with <|state := spi_ready;
-regs := spi.regs with 
-<| SYSCONFIG := spi.regs.SYSCONFIG with <|SIDLEMODE := 2w; AUTOIDLE := 1w|>;
-MODULCTRL := <|SYSTEM_TEST := 0w; MS := 0w; SINGLE := 1w|>;
-CH0CONF := spi.regs.CH0CONF with
-<|PHA := 0w; POL := 0w; CLKD := 6w; EPOL := 1w; WL := 7w; 
-TRM := 0w; DPE0 := 1w; DPE1 := 0w; IS := 0w|> |>;
-init :=
-<|sysconfig_mode_done := T; modulctrl_bus_done := T; 
-ch0conf_wordlen_done :=  T; ch0conf_mode_done := T; 
-ch0conf_speed_done := T|> |>` >>
-fs [n_tau_tr_dr_init_read_req_6, ref_rel_def, IS_STATE_REL_def],
-(* dr_init_check_rep and init_set_regs *)
-`~ dr.dr_init.issue_wr_sysconfig /\ ~ dr.dr_init.issue_wr_modulctrl /\
-~ dr.dr_init.issue_wr_ch0conf_wl /\ ~ dr.dr_init.issue_wr_ch0conf_mode /\
-~ dr.dr_init.issue_wr_ch0conf_speed /\ ~ spi.init.sysconfig_mode_done /\ 
-~ spi.init.modulctrl_bus_done /\ ~ spi.init.ch0conf_wordlen_done /\ 
-~ spi.init.ch0conf_mode_done /\ ~ spi.init.ch0conf_speed_done` by fs [ref_rel_def] >>
-`dr.dr_last_read_ad = SOME SPI0_SYSSTATUS /\ ?v. dr.dr_last_read_v = SOME v` by fs [ref_rel_def] >>
-`spi.regs.SYSSTATUS = 1w` by fs [ref_rel_def] >>
-DISJ2_TAC >>
-Cases_on `(0 >< 0) v:word1 = 1w` >-
-((* the store value of sysstatus  is 1w *)
-Q.EXISTS_TAC `SUC 4` >>
-Q.EXISTS_TAC `dr with <| state := dr_ready; 
-dr_init := 
-<| issue_wr_sysconfig := T; issue_wr_modulctrl := T; 
-issue_wr_ch0conf_wl := T; issue_wr_ch0conf_mode := T; 
-issue_wr_ch0conf_speed := T |> |>` >>
-Q.EXISTS_TAC `spi with <|state := spi_ready;
-regs := spi.regs with 
-<| SYSCONFIG := spi.regs.SYSCONFIG with <|SIDLEMODE := 2w; AUTOIDLE := 1w|>;
-MODULCTRL := <|SYSTEM_TEST := 0w; MS := 0w; SINGLE := 1w|>;
-CH0CONF := spi.regs.CH0CONF with
-<|PHA := 0w; POL := 0w; CLKD := 6w; EPOL := 1w; WL := 7w; 
-TRM := 0w; DPE0 := 1w; DPE1 := 0w; IS := 0w|> |>;
-init :=
-<|sysconfig_mode_done := T; modulctrl_bus_done := T; 
-ch0conf_wordlen_done :=  T; ch0conf_mode_done := T; 
-ch0conf_speed_done := T|> |>` >>
-fs [n_tau_tr_dr_init_check_rep_5, ref_rel_def, IS_STATE_REL_def]) >>
-(* the store value of sysstatus is 0w *)
-`(0 >< 0) v:word1 = 0w` by rw [word1_not_1w_eq_0w] >>
-Q.EXISTS_TAC `SUC 6` >>
-Q.EXISTS_TAC `dr with <| state := dr_ready; 
-dr_last_read_ad := SOME SPI0_SYSSTATUS;
-dr_last_read_v := SOME 1w;
-dr_init := 
-<| issue_wr_sysconfig := T; issue_wr_modulctrl := T; 
-issue_wr_ch0conf_wl := T; issue_wr_ch0conf_mode := T; 
-issue_wr_ch0conf_speed := T |> |>` >>
-Q.EXISTS_TAC `spi with <|state := spi_ready;
-regs := spi.regs with 
-<| SYSCONFIG := spi.regs.SYSCONFIG with <|SIDLEMODE := 2w; AUTOIDLE := 1w|>;
-MODULCTRL := <|SYSTEM_TEST := 0w; MS := 0w; SINGLE := 1w|>;
-CH0CONF := spi.regs.CH0CONF with
-<|PHA := 0w; POL := 0w; CLKD := 6w; EPOL := 1w; WL := 7w; 
-TRM := 0w; DPE0 := 1w; DPE1 := 0w; IS := 0w|> |>;
-init :=
-<|sysconfig_mode_done := T; modulctrl_bus_done := T; 
-ch0conf_wordlen_done :=  T; ch0conf_mode_done := T; 
-ch0conf_speed_done := T|> |>` >>
-fs [n_tau_tr_dr_init_check_rep_7, ref_rel_def, IS_STATE_REL_def],
-(* dr_init_read_req and init_reset *)
-`~ dr.dr_init.issue_wr_sysconfig /\ ~ dr.dr_init.issue_wr_modulctrl /\
-~ dr.dr_init.issue_wr_ch0conf_wl /\ ~ dr.dr_init.issue_wr_ch0conf_mode /\
-~ dr.dr_init.issue_wr_ch0conf_speed /\ ~ spi.init.sysconfig_mode_done /\ 
-~ spi.init.modulctrl_bus_done /\ ~ spi.init.ch0conf_wordlen_done /\ 
-~ spi.init.ch0conf_mode_done /\ ~ spi.init.ch0conf_speed_done` by fs [ref_rel_def] >>
-DISJ2_TAC >>
-Q.EXISTS_TAC `SUC 6` >>
-Q.EXISTS_TAC `dr with <| state := dr_ready; 
-dr_last_read_ad := SOME SPI0_SYSSTATUS;
-dr_last_read_v := SOME 1w;
-dr_init := 
-<| issue_wr_sysconfig := T; issue_wr_modulctrl := T; 
-issue_wr_ch0conf_wl := T; issue_wr_ch0conf_mode := T; 
-issue_wr_ch0conf_speed := T |> |>` >>
+dr_init := <| issue_wr_sysconfig := T; issue_wr_modulctrl := T|> |>` >>
 Q.EXISTS_TAC `spi with <|state := spi_ready;
 regs := spi.regs with 
 <| SYSCONFIG := spi.regs.SYSCONFIG with <|SIDLEMODE := 2w; AUTOIDLE := 1w|>;
 SYSSTATUS := 1w;
 MODULCTRL := <|SYSTEM_TEST := 0w; MS := 0w; SINGLE := 1w|>;
-CH0CONF := spi.regs.CH0CONF with
-<|PHA := 0w; POL := 0w; CLKD := 6w; EPOL := 1w; WL := 7w; 
-TRM := 0w; DPE0 := 1w; DPE1 := 0w; IS := 0w|> |>;
-init :=
-<|sysconfig_mode_done := T; modulctrl_bus_done := T; 
-ch0conf_wordlen_done :=  T; ch0conf_mode_done := T; 
-ch0conf_speed_done := T|> |>` >>
-fs [n_tau_tr_dr_init_read_req_7, ref_rel_def, IS_STATE_REL_def],
-(* dr_init_check_rep and init_reset *)
-`~ dr.dr_init.issue_wr_sysconfig /\ ~ dr.dr_init.issue_wr_modulctrl /\
-~ dr.dr_init.issue_wr_ch0conf_wl /\ ~ dr.dr_init.issue_wr_ch0conf_mode /\
-~ dr.dr_init.issue_wr_ch0conf_speed /\ ~ spi.init.sysconfig_mode_done /\ 
-~ spi.init.modulctrl_bus_done /\ ~ spi.init.ch0conf_wordlen_done /\ 
-~ spi.init.ch0conf_mode_done /\ ~ spi.init.ch0conf_speed_done` by fs [ref_rel_def] >>
-`dr.dr_last_read_ad = SOME SPI0_SYSSTATUS /\ ?v. dr.dr_last_read_v = SOME v` by fs [ref_rel_def] >>
-`(0 >< 0) v:word1 = 0w` by fs [ref_rel_def] >>
-DISJ2_TAC >>
-Q.EXISTS_TAC `SUC 7` >>
-Q.EXISTS_TAC `dr with <| state := dr_ready; 
-dr_last_read_ad := SOME SPI0_SYSSTATUS;
-dr_last_read_v := SOME 1w;
-dr_init := 
-<| issue_wr_sysconfig := T; issue_wr_modulctrl := T; 
-issue_wr_ch0conf_wl := T; issue_wr_ch0conf_mode := T; 
-issue_wr_ch0conf_speed := T |> |>` >>
-Q.EXISTS_TAC `spi with <|state := spi_ready;
-regs := spi.regs with 
-<| SYSCONFIG := spi.regs.SYSCONFIG with <|SIDLEMODE := 2w; AUTOIDLE := 1w|>;
-SYSSTATUS := 1w;
-MODULCTRL := <|SYSTEM_TEST := 0w; MS := 0w; SINGLE := 1w|>;
-CH0CONF := spi.regs.CH0CONF with
-<|PHA := 0w; POL := 0w; CLKD := 6w; EPOL := 1w; WL := 7w; 
-TRM := 0w; DPE0 := 1w; DPE1 := 0w; IS := 0w|> |>;
-init :=
-<|sysconfig_mode_done := T; modulctrl_bus_done := T; 
-ch0conf_wordlen_done :=  T; ch0conf_mode_done := T; 
-ch0conf_speed_done := T|> |>` >>
-fs [n_tau_tr_dr_init_check_rep_8, ref_rel_def, IS_STATE_REL_def],
+CH0CONF := <|PHA := 0w; POL := 0w; CLKD := 6w; EPOL := 1w; WL := 7w; 
+TRM := 0w; DPE0 := 1w; DPE1 := 0w; IS := 0w; FORCE := 0w|> |>;
+init := <|sysconfig_mode_done := T; modulctrl_bus_done := T|> |>` >>
+fs [n_tau_tr_dr_init_check_rep_6, ref_rel_def, IS_STATE_REL_def],
 (* dr_init_idle and init_start *)
 DISJ2_TAC >>
-Q.EXISTS_TAC `SUC 7` >> 
+Q.EXISTS_TAC `SUC 5` >> 
 Q.EXISTS_TAC `dr with <| state := dr_ready; 
 dr_last_read_ad := SOME SPI0_SYSSTATUS; dr_last_read_v := SOME 1w;
-dr_init := 
-<| issue_wr_sysconfig := T; issue_wr_modulctrl := T; 
-issue_wr_ch0conf_wl := T; issue_wr_ch0conf_mode := T; 
-issue_wr_ch0conf_speed := T |> |>` >>
+dr_init := <| issue_wr_sysconfig := T; issue_wr_modulctrl := T|> |>` >>
 Q.EXISTS_TAC `spi with <|state := spi_ready;
 regs := spi.regs with <| SYSCONFIG := <|SIDLEMODE := 2w; SOFTRESET := 0w; AUTOIDLE := 1w|>;
 SYSSTATUS := 1w; MODULCTRL := <|SYSTEM_TEST := 0w; MS := 0w; SINGLE := 1w|>;
-CH0CONF := spi.regs.CH0CONF with
-<|PHA := 0w; POL := 0w; CLKD := 6w; EPOL := 1w; WL := 7w; 
-TRM := 0w; DPE0 := 1w; DPE1 := 0w; IS := 0w|> |>;
-init :=
-<|sysconfig_mode_done := T; modulctrl_bus_done := T; 
-ch0conf_wordlen_done :=  T; ch0conf_mode_done := T; 
-ch0conf_speed_done := T|> |>` >>
-fs [n_tau_tr_dr_init_idle_8, ref_rel_def, IS_STATE_REL_def],
+CH0CONF := <|PHA := 0w; POL := 0w; CLKD := 6w; EPOL := 1w; WL := 7w; 
+TRM := 0w; DPE0 := 1w; DPE1 := 0w; IS := 0w; FORCE := 0w|> |>;
+init := <|sysconfig_mode_done := T; modulctrl_bus_done := T|> |>` >>
+fs [n_tau_tr_dr_init_idle_6, ref_rel_def, IS_STATE_REL_def],
 (* dr_init_idle and spi_ready *)
 DISJ2_TAC >>
-Q.EXISTS_TAC `SUC 7` >> 
+Q.EXISTS_TAC `SUC 5` >> 
 Q.EXISTS_TAC `dr with <| state := dr_ready; 
 dr_last_read_ad := SOME SPI0_SYSSTATUS; dr_last_read_v := SOME 1w;
-dr_init := 
-<| issue_wr_sysconfig := T; issue_wr_modulctrl := T; 
-issue_wr_ch0conf_wl := T; issue_wr_ch0conf_mode := T; 
-issue_wr_ch0conf_speed := T |> |>` >>
+dr_init := <| issue_wr_sysconfig := T; issue_wr_modulctrl := T|> |>` >>
 Q.EXISTS_TAC `spi with <|state := spi_ready;
 regs := spi.regs with <| SYSCONFIG := <|SIDLEMODE := 2w; SOFTRESET := 0w; AUTOIDLE := 1w|>;
 SYSSTATUS := 1w; MODULCTRL := <|SYSTEM_TEST := 0w; MS := 0w; SINGLE := 1w|>;
-CH0CONF := spi.regs.CH0CONF with
-<|PHA := 0w; POL := 0w; CLKD := 6w; EPOL := 1w; WL := 7w; 
-TRM := 0w; DPE0 := 1w; DPE1 := 0w; IS := 0w|> |>;
-init :=
-<|sysconfig_mode_done := T; modulctrl_bus_done := T; 
-ch0conf_wordlen_done :=  T; ch0conf_mode_done := T; 
-ch0conf_speed_done := T|> |>` >>
-fs [n_tau_tr_dr_init_idle_8, ref_rel_def, IS_STATE_REL_def]]);
+CH0CONF := <|PHA := 0w; POL := 0w; CLKD := 6w; EPOL := 1w; WL := 7w; 
+TRM := 0w; DPE0 := 1w; DPE1 := 0w; IS := 0w; FORCE := 0w|> |>;
+init := <|sysconfig_mode_done := T; modulctrl_bus_done := T|> |>` >>
+fs [n_tau_tr_dr_init_idle_6, ref_rel_def, IS_STATE_REL_def]]);
 
 
 (* related to tx automaton *)
@@ -1866,114 +1385,292 @@ val ref_rel_holds_tau_comb_abs1_tx_reset = store_thm("ref_rel_holds_tau_comb_abs
 (ref_rel (comb_abs1_tx_operations ds_abs1) (dr',spi')))``,
 rw [comb_abs1_tx_operations_def, comb_abs1_tx_reset_op_def] >>
 `(dr.state = dr_tx_reset_conf /\ spi.state = tx_channel_disabled) \/
+(dr.state = dr_tx_read_conf /\ spi.state = tx_channel_disabled) \/
 (dr.state = dr_tx_issue_disable /\ spi.state = tx_ready_for_trans) \/
 (dr.state = dr_tx_read_eot /\ spi.state = tx_ready_for_trans) \/
 (dr.state = dr_tx_check_eot /\ spi.state = tx_ready_for_trans)` by fs [IS_STATE_REL_def] >|
 [(* dr_tx_reset_conf and tx_channel_disabled *)
 DISJ1_TAC >>
 rw [local_tr_cases, driver_tr_cases, spi_tr_cases, DR_TAU_ENABLE_def, 
-SPI_TAU_ENABLE_def, DR_WR_ENABLE_def, DR_RD_ENABLE_def] >>
-rw [dr_write_state_def, dr_write_address_def, dr_write_value_def, dr_write_def,
-dr_write_ch0conf_tx_def, write_SPI_regs_def, SPI0_CH0CONF_def, SPI0_PA_RANGE_def,
+SPI_TAU_ENABLE_def, DR_WR_ENABLE_def, DR_RD_ENABLE_def, dr_write_state_def, 
+dr_write_value_def,dr_write_address_def, dr_write_def, dr_write_ch0conf_tx_def] >>
+`dr.dr_last_read_v = SOME (build_CH0CONF spi.regs.CH0CONF)` by fs [ref_rel_def] >>
+`~ (ch0conf_changed ((4293918719w:word32) && (build_CH0CONF spi.regs.CH0CONF)) spi)` 
+by (fs [build_CH0CONF_def,ch0conf_changed_def] >>
+FULL_SIMP_TAC (std_ss++WORD_ss++WORD_BIT_EQ_ss) []) >>
+`spi.regs.CH0CONF.FORCE = 1w` by fs [ref_rel_def] >>
+`(20 >< 20) ((4293918719w:word32) && (build_CH0CONF spi.regs.CH0CONF)) :word1 <> spi.regs.CH0CONF.FORCE` by FULL_SIMP_TAC (std_ss++WORD_ss++WORD_BIT_EQ_ss) [] >>
+`(13 >< 12) ((4293918719w:word32) && (build_CH0CONF spi.regs.CH0CONF)): word2 = spi.regs.CH0CONF.TRM` by (fs [build_CH0CONF_def] >> FULL_SIMP_TAC (std_ss++WORD_ss++WORD_BIT_EQ_ss) []) >>
+rw [write_SPI_regs_def, SPI0_CH0CONF_def, SPI0_PA_RANGE_def,
 SPI0_START_def, SPI0_END_def, SPI0_SYSCONFIG_def, SPI0_MODULCTRL_def,
 write_CH0CONF_comb_def, write_CH0CONF_tx_def] >>
+FULL_SIMP_TAC (std_ss++WORD_ss++WORD_BIT_EQ_ss) [] >>
 fs [ref_rel_def, IS_STATE_REL_def],
-(* dr_tx_issue_disable and tx_ready_for_trans *)
+(* dr_tx_read_conf and tx_channel_disabled *)
 DISJ2_TAC >>
 Q.EXISTS_TAC `SUC 0:num` >>
 rw [n_tau_tr_def, local_tr_cases, driver_tr_cases, spi_tr_cases, DR_TAU_ENABLE_def, 
 SPI_TAU_ENABLE_def, DR_WR_ENABLE_def, DR_RD_ENABLE_def] >>
-`dr_write_state dr = dr with state := dr_tx_reset_conf` 
-by rw [dr_write_state_def, dr_write_def, dr_write_ch0ctrl_def] >>
-rw [] >>
-Q.EXISTS_TAC `dr_write_state (dr with state := dr_tx_reset_conf)` >>
-Q.EXISTS_TAC `write_SPI_regs (THE (dr_write_address (dr with state := dr_tx_reset_conf)))
-(THE (dr_write_value (dr with state := dr_tx_reset_conf)))
-(write_SPI_regs (THE (dr_write_address dr)) (THE (dr_write_value dr)) spi)` >>
-rw [dr_write_address_def, dr_write_state_def, dr_write_value_def, dr_write_def,
-dr_write_ch0conf_tx_def, dr_write_ch0ctrl_def] >>
-rw [write_SPI_regs_def, SPI0_CH0CONF_def, SPI0_PA_RANGE_def, SPI0_START_def, SPI0_END_def, 
-SPI0_SYSCONFIG_def, SPI0_MODULCTRL_def, SPI0_CH0CTRL_def, write_CH0CONF_comb_def, 
-write_CH0CTRL_def, write_CH0CONF_tx_def] >>
-fs [ref_rel_def, IS_STATE_REL_def],
+`dr_read dr = dr with <|state := dr_tx_reset_conf; 
+dr_last_read_ad := SOME SPI0_CH0CONF |>` by rw [dr_read_def,dr_read_ch0conf_def] >> fs [] >>
+`(read_SPI_regs_value SPI0_CH0CONF spi = build_CH0CONF spi.regs.CH0CONF) /\
+(read_SPI_regs_state SPI0_CH0CONF spi = spi)`
+by fs [read_SPI_regs_value_def,read_SPI_regs_state_def,read_SPI_regs_def,
+SPI0_CH0CTRL_def, SPI0_PA_RANGE_def, SPI0_END_def, SPI0_START_def,SPI0_SYSSTATUS_def,
+SPI0_SYSCONFIG_def, SPI0_MODULCTRL_def, SPI0_CH0CONF_def] >> 
+fs [dr_write_state_def,dr_write_address_def,dr_write_value_def,
+dr_write_def, dr_write_ch0conf_tx_def] >>
+`~ (ch0conf_changed ((4293918719w:word32) && (build_CH0CONF spi.regs.CH0CONF)) spi)` 
+by (fs [build_CH0CONF_def,ch0conf_changed_def] >>
+FULL_SIMP_TAC (std_ss++WORD_ss++WORD_BIT_EQ_ss) []) >>
+`spi.regs.CH0CONF.FORCE = 1w` by fs [ref_rel_def] >>
+`(20 >< 20) ((4293918719w:word32) && (build_CH0CONF spi.regs.CH0CONF)) : word1 <> 
+spi.regs.CH0CONF.FORCE` by FULL_SIMP_TAC (std_ss++WORD_ss++WORD_BIT_EQ_ss) [] >>
+`(13 >< 12) ((4293918719w:word32) && (build_CH0CONF spi.regs.CH0CONF)): word2 = 
+spi.regs.CH0CONF.TRM` by (fs [build_CH0CONF_def] >>
+FULL_SIMP_TAC (std_ss++WORD_ss++WORD_BIT_EQ_ss) []) >>
+rw [write_SPI_regs_def, write_CH0CONF_comb_def, write_CH0CONF_tx_def, 
+SPI0_CH0CTRL_def, SPI0_PA_RANGE_def, SPI0_END_def, SPI0_START_def,
+SPI0_SYSCONFIG_def, SPI0_MODULCTRL_def, SPI0_CH0CONF_def] >>
+FULL_SIMP_TAC (std_ss++WORD_ss++WORD_BIT_EQ_ss) [] >>
+fs [ref_rel_def,IS_STATE_REL_def],
+(* dr_tx_issue_disable and tx_ready_for_trans *)
+DISJ2_TAC >>
+Q.EXISTS_TAC `SUC 1:num` >>
+rw [n_tau_tr_def, n_tau_tr_SUC, local_tr_cases, driver_tr_cases, spi_tr_cases, DR_TAU_ENABLE_def, 
+SPI_TAU_ENABLE_def, DR_WR_ENABLE_def, DR_RD_ENABLE_def] >>
+`(dr_write_state dr = dr with state := dr_tx_read_conf) /\
+(dr_write_address dr = SOME SPI0_CH0CTRL) /\
+(dr_write_value dr = SOME (0w:word32))` 
+by rw [dr_write_state_def,dr_write_address_def,dr_write_value_def,dr_write_def, 
+dr_write_ch0ctrl_def] >> fs [] >>
+`write_SPI_regs SPI0_CH0CTRL 0w spi = 
+spi with <|regs := spi.regs with CH0CTRL := 0w;
+state := tx_channel_disabled|>` 
+by rw [write_SPI_regs_def, SPI0_CH0CONF_def, SPI0_PA_RANGE_def, SPI0_START_def, SPI0_END_def, 
+SPI0_SYSCONFIG_def, SPI0_MODULCTRL_def, SPI0_CH0CTRL_def, write_CH0CTRL_def] >> fs [] >>
+`dr_read (dr with state := dr_tx_read_conf) = dr with <|state := dr_tx_reset_conf; 
+dr_last_read_ad := SOME SPI0_CH0CONF |>` by rw [dr_read_def,dr_read_ch0conf_def] >> fs [] >>
+`(read_SPI_regs_value SPI0_CH0CONF (spi with <|state := tx_channel_disabled;
+regs := spi.regs with CH0CTRL := 0w |>) = build_CH0CONF spi.regs.CH0CONF) /\
+(read_SPI_regs_state SPI0_CH0CONF (spi with <|state := tx_channel_disabled;
+regs := spi.regs with CH0CTRL := 0w |>) = (spi with <|state := tx_channel_disabled;
+regs := spi.regs with CH0CTRL := 0w |>))`
+by fs [read_SPI_regs_value_def,read_SPI_regs_state_def,read_SPI_regs_def,
+SPI0_CH0CTRL_def, SPI0_PA_RANGE_def, SPI0_END_def, SPI0_START_def,SPI0_SYSSTATUS_def,
+SPI0_SYSCONFIG_def, SPI0_MODULCTRL_def, SPI0_CH0CONF_def] >> fs [] >>
+rw [dr_write_state_def,dr_write_address_def,dr_write_value_def,
+dr_write_def, dr_write_ch0conf_tx_def] >>
+`~ (ch0conf_changed ((4293918719w:word32) && (build_CH0CONF spi.regs.CH0CONF)) 
+(spi with <|state := tx_channel_disabled;
+regs := spi.regs with CH0CTRL := 0w|>))` 
+by (fs [build_CH0CONF_def,ch0conf_changed_def] >>
+FULL_SIMP_TAC (std_ss++WORD_ss++WORD_BIT_EQ_ss) []) >>
+`spi.regs.CH0CONF.FORCE = 1w` by fs [ref_rel_def] >>
+`(20 >< 20) ((4293918719w:word32) && (build_CH0CONF spi.regs.CH0CONF)) : word1 <> 
+spi.regs.CH0CONF.FORCE` by FULL_SIMP_TAC (std_ss++WORD_ss++WORD_BIT_EQ_ss) [] >>
+`(13 >< 12) ((4293918719w:word32) && (build_CH0CONF spi.regs.CH0CONF)): word2 = 
+spi.regs.CH0CONF.TRM` by (fs [build_CH0CONF_def] >>
+FULL_SIMP_TAC (std_ss++WORD_ss++WORD_BIT_EQ_ss) []) >>
+rw [write_SPI_regs_def, write_CH0CONF_comb_def, write_CH0CONF_tx_def, 
+SPI0_CH0CTRL_def, SPI0_PA_RANGE_def, SPI0_END_def, SPI0_START_def,
+SPI0_SYSCONFIG_def, SPI0_MODULCTRL_def, SPI0_CH0CONF_def] >>
+FULL_SIMP_TAC (std_ss++WORD_ss++WORD_BIT_EQ_ss) [] >>
+fs [ref_rel_def,IS_STATE_REL_def],
 (* dr_tx_read_eot and tx_ready_for_trans *)
 DISJ2_TAC >>
 `spi.regs.CH0STAT.EOT = 1w /\ spi.regs.CH0STAT.TXS = 1w` by fs [ref_rel_def] >>
-Q.EXISTS_TAC `SUC 2:num` >>
+Q.EXISTS_TAC `SUC 3:num` >>
 rw [n_tau_tr_def, n_tau_tr_SUC, local_tr_cases, driver_tr_cases, spi_tr_cases, 
 DR_TAU_ENABLE_def, SPI_TAU_ENABLE_def, DR_WR_ENABLE_def, DR_RD_ENABLE_def] >>
 `dr_read dr = dr with <| state := dr_tx_check_eot; 
-dr_last_read_ad := SOME SPI0_CH0STAT |>` by rw [dr_read_def, dr_read_ch0stat_def] >>
-rw [] >>
+dr_last_read_ad := SOME SPI0_CH0STAT |>` by rw [dr_read_def, dr_read_ch0stat_def] >> rw [] >>
 `read_SPI_regs_state SPI0_CH0STAT spi = spi /\
 read_SPI_regs_value SPI0_CH0STAT spi = build_CH0STAT spi.regs.CH0STAT` by
 rw [read_SPI_regs_state_def, read_SPI_regs_value_def, read_SPI_regs_def, SPI0_CH0STAT_def,
 SPI0_PA_RANGE_def, SPI0_START_def, SPI0_END_def, SPI0_SYSCONFIG_def, SPI0_SYSSTATUS_def,
-SPI0_MODULCTRL_def, SPI0_CH0CONF_def] >>
-rw [] >>
+SPI0_MODULCTRL_def, SPI0_CH0CONF_def] >> rw [] >>
 `dr_check (dr with <| state := dr_tx_check_eot; dr_last_read_ad := SOME SPI0_CH0STAT;
 dr_last_read_v := SOME (build_CH0STAT spi.regs.CH0STAT) |>) 
 SPI0_CH0STAT (build_CH0STAT spi.regs.CH0STAT) = 
 dr with <| state := dr_tx_issue_disable; dr_last_read_ad := SOME SPI0_CH0STAT;
 dr_last_read_v := SOME (build_CH0STAT spi.regs.CH0STAT) |> ` 
 by (rw [dr_check_def, dr_check_tx_ch0stat_def,build_CH0STAT_def] >>
-FULL_SIMP_TAC (std_ss++WORD_ss++WORD_EXTRACT_ss) []) >>
-rw [] >>
-rw [dr_write_address_def, dr_write_state_def, dr_write_value_def, dr_write_def,
-dr_write_ch0conf_tx_def, dr_write_ch0ctrl_def] >>
-rw [write_SPI_regs_def, SPI0_CH0CONF_def, SPI0_PA_RANGE_def, SPI0_START_def, SPI0_END_def, 
-SPI0_SYSCONFIG_def, SPI0_MODULCTRL_def, SPI0_CH0CTRL_def, write_CH0CONF_comb_def, 
-write_CH0CTRL_def, write_CH0CONF_tx_def] >>
-fs [ref_rel_def, IS_STATE_REL_def],
+FULL_SIMP_TAC (std_ss++WORD_ss++WORD_EXTRACT_ss) []) >> rw [] >>
+`(dr_write_state (dr with <|state := dr_tx_issue_disable;
+dr_last_read_ad := SOME SPI0_CH0STAT; 
+dr_last_read_v := SOME (build_CH0STAT spi.regs.CH0STAT)|>) = 
+dr with <|state := dr_tx_read_conf;
+dr_last_read_ad := SOME SPI0_CH0STAT; 
+dr_last_read_v := SOME (build_CH0STAT spi.regs.CH0STAT)|>) /\
+(dr_write_address (dr with <|state := dr_tx_issue_disable;
+dr_last_read_ad := SOME SPI0_CH0STAT; 
+dr_last_read_v := SOME (build_CH0STAT spi.regs.CH0STAT)|>) = SOME SPI0_CH0CTRL) /\
+(dr_write_value (dr with <|state := dr_tx_issue_disable;
+dr_last_read_ad := SOME SPI0_CH0STAT; 
+dr_last_read_v := SOME (build_CH0STAT spi.regs.CH0STAT)|>) = SOME (0w:word32))` 
+by rw [dr_write_state_def,dr_write_address_def,dr_write_value_def,dr_write_def, 
+dr_write_ch0ctrl_def] >> fs [] >>
+`write_SPI_regs SPI0_CH0CTRL 0w spi = 
+spi with <|regs := spi.regs with CH0CTRL := 0w;
+state := tx_channel_disabled|>` 
+by rw [write_SPI_regs_def, SPI0_CH0CONF_def, SPI0_PA_RANGE_def, SPI0_START_def, SPI0_END_def, 
+SPI0_SYSCONFIG_def, SPI0_MODULCTRL_def, SPI0_CH0CTRL_def, write_CH0CTRL_def] >> fs [] >>
+`dr_read (dr with <|state := dr_tx_read_conf;
+dr_last_read_ad := SOME SPI0_CH0STAT; 
+dr_last_read_v := SOME (build_CH0STAT spi.regs.CH0STAT)|>) = 
+dr with <|state := dr_tx_reset_conf; 
+dr_last_read_ad := SOME SPI0_CH0CONF;
+dr_last_read_v := SOME (build_CH0STAT spi.regs.CH0STAT)|>` 
+by rw [dr_read_def,dr_read_ch0conf_def] >> fs [] >>
+`(read_SPI_regs_value SPI0_CH0CONF (spi with <|state := tx_channel_disabled;
+regs := spi.regs with CH0CTRL := 0w |>) = build_CH0CONF spi.regs.CH0CONF) /\
+(read_SPI_regs_state SPI0_CH0CONF (spi with <|state := tx_channel_disabled;
+regs := spi.regs with CH0CTRL := 0w |>) = (spi with <|state := tx_channel_disabled;
+regs := spi.regs with CH0CTRL := 0w |>))`
+by fs [read_SPI_regs_value_def,read_SPI_regs_state_def,read_SPI_regs_def,
+SPI0_CH0CTRL_def, SPI0_PA_RANGE_def, SPI0_END_def, SPI0_START_def,SPI0_SYSSTATUS_def,
+SPI0_SYSCONFIG_def, SPI0_MODULCTRL_def, SPI0_CH0CONF_def] >> fs [] >>
+rw [dr_write_state_def,dr_write_address_def,dr_write_value_def,
+dr_write_def, dr_write_ch0conf_tx_def] >>
+`~ (ch0conf_changed ((4293918719w:word32) && (build_CH0CONF spi.regs.CH0CONF)) 
+(spi with <|state := tx_channel_disabled;
+regs := spi.regs with CH0CTRL := 0w|>))` 
+by (fs [build_CH0CONF_def,ch0conf_changed_def] >>
+FULL_SIMP_TAC (std_ss++WORD_ss++WORD_BIT_EQ_ss) []) >>
+`spi.regs.CH0CONF.FORCE = 1w` by fs [ref_rel_def] >>
+`(20 >< 20) ((4293918719w:word32) && (build_CH0CONF spi.regs.CH0CONF)) : word1 <> 
+spi.regs.CH0CONF.FORCE` by FULL_SIMP_TAC (std_ss++WORD_ss++WORD_BIT_EQ_ss) [] >>
+`(13 >< 12) ((4293918719w:word32) && (build_CH0CONF spi.regs.CH0CONF)): word2 = 
+spi.regs.CH0CONF.TRM` by (fs [build_CH0CONF_def] >>
+FULL_SIMP_TAC (std_ss++WORD_ss++WORD_BIT_EQ_ss) []) >>
+rw [write_SPI_regs_def, write_CH0CONF_comb_def, write_CH0CONF_tx_def, 
+SPI0_CH0CTRL_def, SPI0_PA_RANGE_def, SPI0_END_def, SPI0_START_def,
+SPI0_SYSCONFIG_def, SPI0_MODULCTRL_def, SPI0_CH0CONF_def] >>
+FULL_SIMP_TAC (std_ss++WORD_ss++WORD_BIT_EQ_ss) [] >>
+fs [ref_rel_def,IS_STATE_REL_def],
 (* dr_tx_check_eot and tx_ready_for_trans *)
 `dr.dr_last_read_ad = SOME SPI0_CH0STAT /\ ?v. dr.dr_last_read_v =  SOME v` by fs [ref_rel_def] >>
 DISJ2_TAC >>
 Cases_on `(2 >< 2) v:word1 = 1w /\ (1 >< 1) v:word1 = 1w` >|
 [(* the stored values of txs and eot are 1w *)
-Q.EXISTS_TAC `SUC 1` >>
+Q.EXISTS_TAC `SUC 2` >>
 rw [n_tau_tr_def, n_tau_tr_SUC, local_tr_cases, driver_tr_cases, spi_tr_cases, 
 DR_TAU_ENABLE_def, SPI_TAU_ENABLE_def, DR_WR_ENABLE_def, DR_RD_ENABLE_def] >>
 `dr_check dr SPI0_CH0STAT v = dr with state := dr_tx_issue_disable` 
-by rw [dr_check_def, dr_check_tx_ch0stat_def] >>
-rw [] >>
-rw [dr_write_address_def, dr_write_state_def, dr_write_value_def, dr_write_def,
-dr_write_ch0conf_tx_def, dr_write_ch0ctrl_def] >>
-rw [write_SPI_regs_def, SPI0_CH0CONF_def, SPI0_PA_RANGE_def, SPI0_START_def, SPI0_END_def, 
-SPI0_SYSCONFIG_def, SPI0_MODULCTRL_def, SPI0_CH0CTRL_def, write_CH0CONF_comb_def, 
-write_CH0CTRL_def, write_CH0CONF_tx_def] >>
-fs [ref_rel_def, IS_STATE_REL_def],
+by rw [dr_check_def, dr_check_tx_ch0stat_def] >> rw [] >>
+`(dr_write_state (dr with state := dr_tx_issue_disable) = dr with state := dr_tx_read_conf) /\
+(dr_write_address (dr with state := dr_tx_issue_disable) = SOME SPI0_CH0CTRL) /\
+(dr_write_value (dr with state := dr_tx_issue_disable) = SOME (0w:word32))` 
+by rw [dr_write_state_def,dr_write_address_def,dr_write_value_def,dr_write_def, 
+dr_write_ch0ctrl_def] >> fs [] >>
+`write_SPI_regs SPI0_CH0CTRL 0w spi = 
+spi with <|regs := spi.regs with CH0CTRL := 0w;
+state := tx_channel_disabled|>` 
+by rw [write_SPI_regs_def, SPI0_CH0CONF_def, SPI0_PA_RANGE_def, SPI0_START_def, SPI0_END_def, 
+SPI0_SYSCONFIG_def, SPI0_MODULCTRL_def, SPI0_CH0CTRL_def, write_CH0CTRL_def] >> fs [] >>
+`dr_read (dr with state := dr_tx_read_conf) = dr with <|state := dr_tx_reset_conf; 
+dr_last_read_ad := SOME SPI0_CH0CONF |>` by rw [dr_read_def,dr_read_ch0conf_def] >> fs [] >>
+`(read_SPI_regs_value SPI0_CH0CONF (spi with <|state := tx_channel_disabled;
+regs := spi.regs with CH0CTRL := 0w |>) = build_CH0CONF spi.regs.CH0CONF) /\
+(read_SPI_regs_state SPI0_CH0CONF (spi with <|state := tx_channel_disabled;
+regs := spi.regs with CH0CTRL := 0w |>) = (spi with <|state := tx_channel_disabled;
+regs := spi.regs with CH0CTRL := 0w |>))`
+by fs [read_SPI_regs_value_def,read_SPI_regs_state_def,read_SPI_regs_def,
+SPI0_CH0CTRL_def, SPI0_PA_RANGE_def, SPI0_END_def, SPI0_START_def,SPI0_SYSSTATUS_def,
+SPI0_SYSCONFIG_def, SPI0_MODULCTRL_def, SPI0_CH0CONF_def] >> fs [] >>
+rw [dr_write_state_def,dr_write_address_def,dr_write_value_def,
+dr_write_def, dr_write_ch0conf_tx_def] >>
+`~ (ch0conf_changed ((4293918719w:word32) && (build_CH0CONF spi.regs.CH0CONF)) 
+(spi with <|state := tx_channel_disabled;
+regs := spi.regs with CH0CTRL := 0w|>))` 
+by (fs [build_CH0CONF_def,ch0conf_changed_def] >>
+FULL_SIMP_TAC (std_ss++WORD_ss++WORD_BIT_EQ_ss) []) >>
+`spi.regs.CH0CONF.FORCE = 1w` by fs [ref_rel_def] >>
+`(20 >< 20) ((4293918719w:word32) && (build_CH0CONF spi.regs.CH0CONF)) : word1 <> 
+spi.regs.CH0CONF.FORCE` by FULL_SIMP_TAC (std_ss++WORD_ss++WORD_BIT_EQ_ss) [] >>
+`(13 >< 12) ((4293918719w:word32) && (build_CH0CONF spi.regs.CH0CONF)): word2 = 
+spi.regs.CH0CONF.TRM` by (fs [build_CH0CONF_def] >>
+FULL_SIMP_TAC (std_ss++WORD_ss++WORD_BIT_EQ_ss) []) >>
+rw [write_SPI_regs_def, write_CH0CONF_comb_def, write_CH0CONF_tx_def, 
+SPI0_CH0CTRL_def, SPI0_PA_RANGE_def, SPI0_END_def, SPI0_START_def,
+SPI0_SYSCONFIG_def, SPI0_MODULCTRL_def, SPI0_CH0CONF_def] >>
+FULL_SIMP_TAC (std_ss++WORD_ss++WORD_BIT_EQ_ss) [] >>
+fs [ref_rel_def,IS_STATE_REL_def],
 (* the stored values are not 1w *)
-Q.EXISTS_TAC `SUC 3` >>
+Q.EXISTS_TAC `SUC 4` >>
 rw [n_tau_tr_def, n_tau_tr_SUC, local_tr_cases, driver_tr_cases, spi_tr_cases, 
 DR_TAU_ENABLE_def, SPI_TAU_ENABLE_def, DR_WR_ENABLE_def, DR_RD_ENABLE_def] >>
 `dr_check dr SPI0_CH0STAT v = dr with state := dr_tx_read_eot` 
-by rw [dr_check_def, dr_check_tx_ch0stat_def] >>
-rw [] >>
+by rw [dr_check_def, dr_check_tx_ch0stat_def] >> rw [] >>
 `spi.regs.CH0STAT.EOT = 1w /\ spi.regs.CH0STAT.TXS = 1w` by fs [ref_rel_def] >>
 `dr_read (dr with state := dr_tx_read_eot) = 
 dr with <| state := dr_tx_check_eot; 
-dr_last_read_ad := SOME SPI0_CH0STAT |>` by rw [dr_read_def, dr_read_ch0stat_def] >>
-rw [] >>
+dr_last_read_ad := SOME SPI0_CH0STAT |>` by rw [dr_read_def, dr_read_ch0stat_def] >> rw [] >>
 `read_SPI_regs_state SPI0_CH0STAT spi = spi /\
 read_SPI_regs_value SPI0_CH0STAT spi = build_CH0STAT spi.regs.CH0STAT` by
 rw [read_SPI_regs_state_def, read_SPI_regs_value_def, read_SPI_regs_def, SPI0_CH0STAT_def,
 SPI0_PA_RANGE_def, SPI0_START_def, SPI0_END_def, SPI0_SYSCONFIG_def, SPI0_SYSSTATUS_def,
-SPI0_MODULCTRL_def, SPI0_CH0CONF_def] >>
-rw [] >>
+SPI0_MODULCTRL_def, SPI0_CH0CONF_def] >> rw [] >>
 `dr_check (dr with <| state := dr_tx_check_eot; dr_last_read_ad := SOME SPI0_CH0STAT;
 dr_last_read_v := SOME (build_CH0STAT spi.regs.CH0STAT) |>) 
 SPI0_CH0STAT (build_CH0STAT spi.regs.CH0STAT) = 
 dr with <| state := dr_tx_issue_disable; dr_last_read_ad := SOME SPI0_CH0STAT;
 dr_last_read_v := SOME (build_CH0STAT spi.regs.CH0STAT) |> ` 
 by (rw [dr_check_def, dr_check_tx_ch0stat_def,build_CH0STAT_def] >>
-FULL_SIMP_TAC (std_ss++WORD_ss++WORD_EXTRACT_ss) []) >>
-rw [] >>
-rw [dr_write_address_def, dr_write_state_def, dr_write_value_def, dr_write_def,
-dr_write_ch0conf_tx_def, dr_write_ch0ctrl_def] >>
-rw [write_SPI_regs_def, SPI0_CH0CONF_def, SPI0_PA_RANGE_def, SPI0_START_def, SPI0_END_def, 
-SPI0_SYSCONFIG_def, SPI0_MODULCTRL_def, SPI0_CH0CTRL_def, write_CH0CONF_comb_def, 
-write_CH0CTRL_def, write_CH0CONF_tx_def] >>
-fs [ref_rel_def, IS_STATE_REL_def]]]);
+FULL_SIMP_TAC (std_ss++WORD_ss++WORD_EXTRACT_ss) []) >> rw [] >>
+`(dr_write_state (dr with <|state := dr_tx_issue_disable;
+dr_last_read_ad := SOME SPI0_CH0STAT; 
+dr_last_read_v := SOME (build_CH0STAT spi.regs.CH0STAT)|>) = 
+dr with <|state := dr_tx_read_conf;
+dr_last_read_ad := SOME SPI0_CH0STAT; 
+dr_last_read_v := SOME (build_CH0STAT spi.regs.CH0STAT)|>) /\
+(dr_write_address (dr with <|state := dr_tx_issue_disable;
+dr_last_read_ad := SOME SPI0_CH0STAT; 
+dr_last_read_v := SOME (build_CH0STAT spi.regs.CH0STAT)|>) = SOME SPI0_CH0CTRL) /\
+(dr_write_value (dr with <|state := dr_tx_issue_disable;
+dr_last_read_ad := SOME SPI0_CH0STAT; 
+dr_last_read_v := SOME (build_CH0STAT spi.regs.CH0STAT)|>) = SOME (0w:word32))` 
+by rw [dr_write_state_def,dr_write_address_def,dr_write_value_def,dr_write_def, 
+dr_write_ch0ctrl_def] >> fs [] >>
+`write_SPI_regs SPI0_CH0CTRL 0w spi = 
+spi with <|regs := spi.regs with CH0CTRL := 0w;
+state := tx_channel_disabled|>` 
+by rw [write_SPI_regs_def, SPI0_CH0CONF_def, SPI0_PA_RANGE_def, SPI0_START_def, SPI0_END_def, 
+SPI0_SYSCONFIG_def, SPI0_MODULCTRL_def, SPI0_CH0CTRL_def, write_CH0CTRL_def] >> fs [] >>
+`dr_read (dr with <|state := dr_tx_read_conf;
+dr_last_read_ad := SOME SPI0_CH0STAT; 
+dr_last_read_v := SOME (build_CH0STAT spi.regs.CH0STAT)|>) = 
+dr with <|state := dr_tx_reset_conf; 
+dr_last_read_ad := SOME SPI0_CH0CONF;
+dr_last_read_v := SOME (build_CH0STAT spi.regs.CH0STAT)|>` 
+by rw [dr_read_def,dr_read_ch0conf_def] >> fs [] >>
+`(read_SPI_regs_value SPI0_CH0CONF (spi with <|state := tx_channel_disabled;
+regs := spi.regs with CH0CTRL := 0w |>) = build_CH0CONF spi.regs.CH0CONF) /\
+(read_SPI_regs_state SPI0_CH0CONF (spi with <|state := tx_channel_disabled;
+regs := spi.regs with CH0CTRL := 0w |>) = (spi with <|state := tx_channel_disabled;
+regs := spi.regs with CH0CTRL := 0w |>))`
+by fs [read_SPI_regs_value_def,read_SPI_regs_state_def,read_SPI_regs_def,
+SPI0_CH0CTRL_def, SPI0_PA_RANGE_def, SPI0_END_def, SPI0_START_def,SPI0_SYSSTATUS_def,
+SPI0_SYSCONFIG_def, SPI0_MODULCTRL_def, SPI0_CH0CONF_def] >> fs [] >>
+rw [dr_write_state_def,dr_write_address_def,dr_write_value_def,
+dr_write_def, dr_write_ch0conf_tx_def] >>
+`~ (ch0conf_changed ((4293918719w:word32) && (build_CH0CONF spi.regs.CH0CONF)) 
+(spi with <|state := tx_channel_disabled;
+regs := spi.regs with CH0CTRL := 0w|>))` 
+by (fs [build_CH0CONF_def,ch0conf_changed_def] >>
+FULL_SIMP_TAC (std_ss++WORD_ss++WORD_BIT_EQ_ss) []) >>
+`spi.regs.CH0CONF.FORCE = 1w` by fs [ref_rel_def] >>
+`(20 >< 20) ((4293918719w:word32) && (build_CH0CONF spi.regs.CH0CONF)) : word1 <> 
+spi.regs.CH0CONF.FORCE` by FULL_SIMP_TAC (std_ss++WORD_ss++WORD_BIT_EQ_ss) [] >>
+`(13 >< 12) ((4293918719w:word32) && (build_CH0CONF spi.regs.CH0CONF)): word2 = 
+spi.regs.CH0CONF.TRM` by (fs [build_CH0CONF_def] >>
+FULL_SIMP_TAC (std_ss++WORD_ss++WORD_BIT_EQ_ss) []) >>
+rw [write_SPI_regs_def, write_CH0CONF_comb_def, write_CH0CONF_tx_def, 
+SPI0_CH0CTRL_def, SPI0_PA_RANGE_def, SPI0_END_def, SPI0_START_def,
+SPI0_SYSCONFIG_def, SPI0_MODULCTRL_def, SPI0_CH0CONF_def] >>
+FULL_SIMP_TAC (std_ss++WORD_ss++WORD_BIT_EQ_ss) [] >>
+fs [ref_rel_def,IS_STATE_REL_def]]]);
 
 (* (dr', spi') exists for tx *)
 val abs1_comb_hold_ref_rel_tau_comb_tx = store_thm("abs1_comb_hold_ref_rel_tau_comb_tx",
@@ -2020,34 +1717,96 @@ val ref_rel_holds_tau_comb_abs1_rx_reset = store_thm("ref_rel_holds_tau_comb_abs
 (ref_rel (comb_abs1_rx_operations ds_abs1) (dr',spi')))``,
 rw [comb_abs1_rx_operations_def, comb_abs1_rx_reset_op_def] >>
 `(dr.state = dr_rx_reset_conf /\ spi.state = rx_channel_disabled) \/
-(dr.state = dr_rx_issue_disable /\ spi.state = rx_data_ready)` by fs [IS_STATE_REL_def] >-
-((* dr_rx_reset_conf and rx_rx_channel_disabled *)
+(dr.state = dr_rx_read_conf /\ spi.state = rx_channel_disabled) \/
+(dr.state = dr_rx_issue_disable /\ spi.state = rx_data_ready)` by fs [IS_STATE_REL_def] >| 
+[(* dr_rx_reset_conf and rx_rx_channel_disabled *)
 DISJ1_TAC >>
 rw [local_tr_cases, driver_tr_cases, spi_tr_cases, DR_TAU_ENABLE_def, 
-SPI_TAU_ENABLE_def, DR_WR_ENABLE_def, DR_RD_ENABLE_def] >>
-rw [dr_write_state_def, dr_write_address_def, dr_write_value_def, dr_write_def,
-dr_write_ch0conf_rx_def, write_SPI_regs_def, SPI0_CH0CONF_def, SPI0_PA_RANGE_def,
+SPI_TAU_ENABLE_def, DR_WR_ENABLE_def, DR_RD_ENABLE_def, dr_write_state_def, 
+dr_write_value_def,dr_write_address_def, dr_write_def, dr_write_ch0conf_rx_def] >>
+`dr.dr_last_read_v = SOME (build_CH0CONF spi.regs.CH0CONF)` by fs [ref_rel_def] >>
+`~ (ch0conf_changed ((4293918719w:word32) && (build_CH0CONF spi.regs.CH0CONF)) spi)` 
+by (fs [build_CH0CONF_def,ch0conf_changed_def] >>
+FULL_SIMP_TAC (std_ss++WORD_ss++WORD_BIT_EQ_ss) []) >>
+`spi.regs.CH0CONF.FORCE = 1w` by fs [ref_rel_def] >>
+`(20 >< 20) ((4293918719w:word32) && (build_CH0CONF spi.regs.CH0CONF)) :word1 <> spi.regs.CH0CONF.FORCE` by FULL_SIMP_TAC (std_ss++WORD_ss++WORD_BIT_EQ_ss) [] >>
+`(13 >< 12) ((4293918719w:word32) && (build_CH0CONF spi.regs.CH0CONF)): word2 = spi.regs.CH0CONF.TRM` by (fs [build_CH0CONF_def] >> FULL_SIMP_TAC (std_ss++WORD_ss++WORD_BIT_EQ_ss) []) >>
+rw [write_SPI_regs_def, SPI0_CH0CONF_def, SPI0_PA_RANGE_def,
 SPI0_START_def, SPI0_END_def, SPI0_SYSCONFIG_def, SPI0_MODULCTRL_def,
 write_CH0CONF_comb_def, write_CH0CONF_rx_def] >>
-fs [ref_rel_def, IS_STATE_REL_def]) >>
-(* dr_rx_issue_disable and rx_data_ready *)
+FULL_SIMP_TAC (std_ss++WORD_ss++WORD_BIT_EQ_ss) [] >>
+fs [ref_rel_def, IS_STATE_REL_def],
+(* dr_rx_read_conf and rx_channel_disabled *)
 DISJ2_TAC >>
 Q.EXISTS_TAC `SUC 0:num` >>
 rw [n_tau_tr_def, local_tr_cases, driver_tr_cases, spi_tr_cases, DR_TAU_ENABLE_def, 
 SPI_TAU_ENABLE_def, DR_WR_ENABLE_def, DR_RD_ENABLE_def] >>
-`dr_write_state dr = dr with state := dr_rx_reset_conf` 
-by rw [dr_write_state_def, dr_write_def, dr_write_ch0ctrl_def] >>
-rw [] >>
-Q.EXISTS_TAC `dr_write_state (dr with state := dr_rx_reset_conf)` >>
-Q.EXISTS_TAC `write_SPI_regs (THE (dr_write_address (dr with state := dr_rx_reset_conf)))
-(THE (dr_write_value (dr with state := dr_rx_reset_conf)))
-(write_SPI_regs (THE (dr_write_address dr)) (THE (dr_write_value dr)) spi)` >>
-rw [dr_write_address_def, dr_write_state_def, dr_write_value_def, dr_write_def,
-dr_write_ch0conf_rx_def, dr_write_ch0ctrl_def] >>
-rw [write_SPI_regs_def, SPI0_CH0CONF_def, SPI0_PA_RANGE_def, SPI0_START_def, SPI0_END_def, 
-SPI0_SYSCONFIG_def, SPI0_MODULCTRL_def, SPI0_CH0CTRL_def, write_CH0CONF_comb_def, 
-write_CH0CTRL_def, write_CH0CONF_rx_def] >>
-fs [ref_rel_def, IS_STATE_REL_def]);
+`dr_read dr = dr with <|state := dr_rx_reset_conf; 
+dr_last_read_ad := SOME SPI0_CH0CONF |>` by rw [dr_read_def,dr_read_ch0conf_def] >> fs [] >>
+`(read_SPI_regs_value SPI0_CH0CONF spi = build_CH0CONF spi.regs.CH0CONF) /\
+(read_SPI_regs_state SPI0_CH0CONF spi = spi)`
+by fs [read_SPI_regs_value_def,read_SPI_regs_state_def,read_SPI_regs_def,
+SPI0_CH0CTRL_def, SPI0_PA_RANGE_def, SPI0_END_def, SPI0_START_def,SPI0_SYSSTATUS_def,
+SPI0_SYSCONFIG_def, SPI0_MODULCTRL_def, SPI0_CH0CONF_def] >> 
+fs [dr_write_state_def,dr_write_address_def,dr_write_value_def,
+dr_write_def, dr_write_ch0conf_rx_def] >>
+`~ (ch0conf_changed ((4293918719w:word32) && (build_CH0CONF spi.regs.CH0CONF)) spi)` 
+by (fs [build_CH0CONF_def,ch0conf_changed_def] >>
+FULL_SIMP_TAC (std_ss++WORD_ss++WORD_BIT_EQ_ss) []) >>
+`spi.regs.CH0CONF.FORCE = 1w` by fs [ref_rel_def] >>
+`(20 >< 20) ((4293918719w:word32) && (build_CH0CONF spi.regs.CH0CONF)) : word1 <> 
+spi.regs.CH0CONF.FORCE` by FULL_SIMP_TAC (std_ss++WORD_ss++WORD_BIT_EQ_ss) [] >>
+`(13 >< 12) ((4293918719w:word32) && (build_CH0CONF spi.regs.CH0CONF)): word2 = 
+spi.regs.CH0CONF.TRM` by (fs [build_CH0CONF_def] >>
+FULL_SIMP_TAC (std_ss++WORD_ss++WORD_BIT_EQ_ss) []) >>
+rw [write_SPI_regs_def, write_CH0CONF_comb_def, write_CH0CONF_rx_def, 
+SPI0_CH0CTRL_def, SPI0_PA_RANGE_def, SPI0_END_def, SPI0_START_def,
+SPI0_SYSCONFIG_def, SPI0_MODULCTRL_def, SPI0_CH0CONF_def] >>
+FULL_SIMP_TAC (std_ss++WORD_ss++WORD_BIT_EQ_ss) [] >>
+fs [ref_rel_def,IS_STATE_REL_def],
+(* dr_rx_issue_disable and rx_data_ready *)
+DISJ2_TAC >>
+Q.EXISTS_TAC `SUC 1:num` >>
+rw [n_tau_tr_def, n_tau_tr_SUC, local_tr_cases, driver_tr_cases, spi_tr_cases, DR_TAU_ENABLE_def, 
+SPI_TAU_ENABLE_def, DR_WR_ENABLE_def, DR_RD_ENABLE_def] >>
+`(dr_write_state dr = dr with state := dr_rx_read_conf) /\
+(dr_write_address dr = SOME SPI0_CH0CTRL) /\
+(dr_write_value dr = SOME (0w:word32))` 
+by rw [dr_write_state_def,dr_write_address_def,dr_write_value_def,dr_write_def, 
+dr_write_ch0ctrl_def] >> fs [] >>
+`write_SPI_regs SPI0_CH0CTRL 0w spi = 
+spi with <|regs := spi.regs with CH0CTRL := 0w;
+state := rx_channel_disabled|>` 
+by rw [write_SPI_regs_def, SPI0_CH0CONF_def, SPI0_PA_RANGE_def, SPI0_START_def, SPI0_END_def, 
+SPI0_SYSCONFIG_def, SPI0_MODULCTRL_def, SPI0_CH0CTRL_def, write_CH0CTRL_def] >> fs [] >>
+`dr_read (dr with state := dr_rx_read_conf) = dr with <|state := dr_rx_reset_conf; 
+dr_last_read_ad := SOME SPI0_CH0CONF |>` by rw [dr_read_def,dr_read_ch0conf_def] >> fs [] >>
+`(read_SPI_regs_value SPI0_CH0CONF (spi with <|state := rx_channel_disabled;
+regs := spi.regs with CH0CTRL := 0w |>) = build_CH0CONF spi.regs.CH0CONF) /\
+(read_SPI_regs_state SPI0_CH0CONF (spi with <|state := rx_channel_disabled;
+regs := spi.regs with CH0CTRL := 0w |>) = (spi with <|state := rx_channel_disabled;
+regs := spi.regs with CH0CTRL := 0w |>))`
+by fs [read_SPI_regs_value_def,read_SPI_regs_state_def,read_SPI_regs_def,
+SPI0_CH0CTRL_def, SPI0_PA_RANGE_def, SPI0_END_def, SPI0_START_def,SPI0_SYSSTATUS_def,
+SPI0_SYSCONFIG_def, SPI0_MODULCTRL_def, SPI0_CH0CONF_def] >> fs [] >>
+rw [dr_write_state_def,dr_write_address_def,dr_write_value_def,
+dr_write_def, dr_write_ch0conf_rx_def] >>
+`~ (ch0conf_changed ((4293918719w:word32) && (build_CH0CONF spi.regs.CH0CONF)) 
+(spi with <|state := rx_channel_disabled;
+regs := spi.regs with CH0CTRL := 0w|>))` 
+by (fs [build_CH0CONF_def,ch0conf_changed_def] >>
+FULL_SIMP_TAC (std_ss++WORD_ss++WORD_BIT_EQ_ss) []) >>
+`spi.regs.CH0CONF.FORCE = 1w` by fs [ref_rel_def] >>
+`(20 >< 20) ((4293918719w:word32) && (build_CH0CONF spi.regs.CH0CONF)) : word1 <> 
+spi.regs.CH0CONF.FORCE` by FULL_SIMP_TAC (std_ss++WORD_ss++WORD_BIT_EQ_ss) [] >>
+`(13 >< 12) ((4293918719w:word32) && (build_CH0CONF spi.regs.CH0CONF)): word2 = 
+spi.regs.CH0CONF.TRM` by (fs [build_CH0CONF_def] >>
+FULL_SIMP_TAC (std_ss++WORD_ss++WORD_BIT_EQ_ss) []) >>
+rw [write_SPI_regs_def, write_CH0CONF_comb_def, write_CH0CONF_rx_def, 
+SPI0_CH0CTRL_def, SPI0_PA_RANGE_def, SPI0_END_def, SPI0_START_def,
+SPI0_SYSCONFIG_def, SPI0_MODULCTRL_def, SPI0_CH0CONF_def] >>
+FULL_SIMP_TAC (std_ss++WORD_ss++WORD_BIT_EQ_ss) [] >>
+fs [ref_rel_def,IS_STATE_REL_def]]);
 
 (* (ds',spi') exists for rx *)
 val abs1_comb_hold_ref_rel_tau_comb_rx = store_thm("abs1_comb_hold_ref_rel_tau_comb_rx",
@@ -2242,33 +2001,96 @@ val ref_rel_holds_tau_comb_abs1_xfer_reset = store_thm("ref_rel_holds_tau_comb_a
 (ref_rel (comb_abs1_xfer_operations ds_abs1) (dr',spi')))``,
 rw [comb_abs1_xfer_operations_def, comb_abs1_xfer_reset_op_def] >>
 `(dr.state = dr_xfer_reset_conf /\ spi.state = xfer_channel_disabled) \/
-(dr.state = dr_xfer_issue_disable /\ spi.state = xfer_ready_for_trans)` by fs [IS_STATE_REL_def] >-
-((* dr_xfer_reset_conf and xfer_channel_disabled *)
+(dr.state = dr_xfer_read_conf /\ spi.state = xfer_channel_disabled) \/
+(dr.state = dr_xfer_issue_disable /\ spi.state = xfer_ready_for_trans)` by fs [IS_STATE_REL_def] >|
+[(* dr_xfer_reset_conf and xfer_channel_disabled *)
 DISJ1_TAC >>
 rw [local_tr_cases, driver_tr_cases, spi_tr_cases, DR_TAU_ENABLE_def, 
-SPI_TAU_ENABLE_def, DR_WR_ENABLE_def, DR_RD_ENABLE_def] >>
-rw [dr_write_state_def, dr_write_value_def, dr_write_address_def, dr_write_def, 
-dr_write_ch0conf_xfer_def, write_SPI_regs_def, SPI0_CH0CONF_def, SPI0_PA_RANGE_def,
-SPI0_START_def, SPI0_END_def, SPI0_SYSCONFIG_def, SPI0_MODULCTRL_def, write_CH0CONF_comb_def,
-write_CH0CONF_xfer_def] >>
-fs [ref_rel_def, IS_STATE_REL_def]) >>
+SPI_TAU_ENABLE_def, DR_WR_ENABLE_def, DR_RD_ENABLE_def, dr_write_state_def, 
+dr_write_value_def,dr_write_address_def, dr_write_def, dr_write_ch0conf_xfer_def] >>
+`dr.dr_last_read_v = SOME (build_CH0CONF spi.regs.CH0CONF)` by fs [ref_rel_def] >>
+`~ (ch0conf_changed ((4293918719w:word32) && (build_CH0CONF spi.regs.CH0CONF)) spi)` 
+by (fs [build_CH0CONF_def,ch0conf_changed_def] >>
+FULL_SIMP_TAC (std_ss++WORD_ss++WORD_BIT_EQ_ss) []) >>
+`spi.regs.CH0CONF.FORCE = 1w` by fs [ref_rel_def] >>
+`(20 >< 20) ((4293918719w:word32) && (build_CH0CONF spi.regs.CH0CONF)) :word1 <> spi.regs.CH0CONF.FORCE` by FULL_SIMP_TAC (std_ss++WORD_ss++WORD_BIT_EQ_ss) [] >>
+`(13 >< 12) ((4293918719w:word32) && (build_CH0CONF spi.regs.CH0CONF)): word2 = spi.regs.CH0CONF.TRM` by (fs [build_CH0CONF_def] >> FULL_SIMP_TAC (std_ss++WORD_ss++WORD_BIT_EQ_ss) []) >>
+rw [write_SPI_regs_def, SPI0_CH0CONF_def, SPI0_PA_RANGE_def,
+SPI0_START_def, SPI0_END_def, SPI0_SYSCONFIG_def, SPI0_MODULCTRL_def,
+write_CH0CONF_comb_def, write_CH0CONF_xfer_def] >>
+FULL_SIMP_TAC (std_ss++WORD_ss++WORD_BIT_EQ_ss) [] >>
+fs [ref_rel_def, IS_STATE_REL_def],
+(* dr_xfer_read_conf and xfer_channel_disabled *)
 DISJ2_TAC >>
 Q.EXISTS_TAC `SUC 0:num` >>
 rw [n_tau_tr_def, local_tr_cases, driver_tr_cases, spi_tr_cases, DR_TAU_ENABLE_def, 
 SPI_TAU_ENABLE_def, DR_WR_ENABLE_def, DR_RD_ENABLE_def] >>
-`dr_write_state dr = dr with state := dr_xfer_reset_conf` 
-by rw [dr_write_state_def, dr_write_def, dr_write_ch0ctrl_def] >>
-rw [] >>
-Q.EXISTS_TAC `dr_write_state (dr with state := dr_xfer_reset_conf)` >>
-Q.EXISTS_TAC `write_SPI_regs (THE (dr_write_address (dr with state := dr_xfer_reset_conf)))
-(THE (dr_write_value (dr with state := dr_xfer_reset_conf)))
-(write_SPI_regs (THE (dr_write_address dr)) (THE (dr_write_value dr)) spi)` >>
-rw [dr_write_address_def, dr_write_state_def, dr_write_value_def, dr_write_def,
-dr_write_ch0conf_xfer_def, dr_write_ch0ctrl_def] >>
-rw [write_SPI_regs_def, SPI0_CH0CONF_def, SPI0_PA_RANGE_def, SPI0_START_def, SPI0_END_def, 
-SPI0_SYSCONFIG_def, SPI0_MODULCTRL_def, SPI0_CH0CTRL_def, write_CH0CONF_comb_def, 
-write_CH0CTRL_def, write_CH0CONF_xfer_def] >>
-fs [ref_rel_def, IS_STATE_REL_def]);
+`dr_read dr = dr with <|state := dr_xfer_reset_conf; 
+dr_last_read_ad := SOME SPI0_CH0CONF |>` by rw [dr_read_def,dr_read_ch0conf_def] >> fs [] >>
+`(read_SPI_regs_value SPI0_CH0CONF spi = build_CH0CONF spi.regs.CH0CONF) /\
+(read_SPI_regs_state SPI0_CH0CONF spi = spi)`
+by fs [read_SPI_regs_value_def,read_SPI_regs_state_def,read_SPI_regs_def,
+SPI0_CH0CTRL_def, SPI0_PA_RANGE_def, SPI0_END_def, SPI0_START_def,SPI0_SYSSTATUS_def,
+SPI0_SYSCONFIG_def, SPI0_MODULCTRL_def, SPI0_CH0CONF_def] >> 
+fs [dr_write_state_def,dr_write_address_def,dr_write_value_def,
+dr_write_def, dr_write_ch0conf_xfer_def] >>
+`~ (ch0conf_changed ((4293918719w:word32) && (build_CH0CONF spi.regs.CH0CONF)) spi)` 
+by (fs [build_CH0CONF_def,ch0conf_changed_def] >>
+FULL_SIMP_TAC (std_ss++WORD_ss++WORD_BIT_EQ_ss) []) >>
+`spi.regs.CH0CONF.FORCE = 1w` by fs [ref_rel_def] >>
+`(20 >< 20) ((4293918719w:word32) && (build_CH0CONF spi.regs.CH0CONF)) : word1 <> 
+spi.regs.CH0CONF.FORCE` by FULL_SIMP_TAC (std_ss++WORD_ss++WORD_BIT_EQ_ss) [] >>
+`(13 >< 12) ((4293918719w:word32) && (build_CH0CONF spi.regs.CH0CONF)): word2 = 
+spi.regs.CH0CONF.TRM` by (fs [build_CH0CONF_def] >>
+FULL_SIMP_TAC (std_ss++WORD_ss++WORD_BIT_EQ_ss) []) >>
+rw [write_SPI_regs_def, write_CH0CONF_comb_def, write_CH0CONF_xfer_def, 
+SPI0_CH0CTRL_def, SPI0_PA_RANGE_def, SPI0_END_def, SPI0_START_def,
+SPI0_SYSCONFIG_def, SPI0_MODULCTRL_def, SPI0_CH0CONF_def] >>
+FULL_SIMP_TAC (std_ss++WORD_ss++WORD_BIT_EQ_ss) [] >>
+fs [ref_rel_def,IS_STATE_REL_def],
+(* dr_xfer_issue_disable and xfer_ready_for_trans_*)
+DISJ2_TAC >>
+Q.EXISTS_TAC `SUC 1:num` >>
+rw [n_tau_tr_def, n_tau_tr_SUC, local_tr_cases, driver_tr_cases, spi_tr_cases, DR_TAU_ENABLE_def, 
+SPI_TAU_ENABLE_def, DR_WR_ENABLE_def, DR_RD_ENABLE_def] >>
+`(dr_write_state dr = dr with state := dr_xfer_read_conf) /\
+(dr_write_address dr = SOME SPI0_CH0CTRL) /\
+(dr_write_value dr = SOME (0w:word32))` 
+by rw [dr_write_state_def,dr_write_address_def,dr_write_value_def,dr_write_def, 
+dr_write_ch0ctrl_def] >> fs [] >>
+`write_SPI_regs SPI0_CH0CTRL 0w spi = 
+spi with <|regs := spi.regs with CH0CTRL := 0w;
+state := xfer_channel_disabled|>` 
+by rw [write_SPI_regs_def, SPI0_CH0CONF_def, SPI0_PA_RANGE_def, SPI0_START_def, SPI0_END_def, 
+SPI0_SYSCONFIG_def, SPI0_MODULCTRL_def, SPI0_CH0CTRL_def, write_CH0CTRL_def] >> fs [] >>
+`dr_read (dr with state := dr_xfer_read_conf) = dr with <|state := dr_xfer_reset_conf; 
+dr_last_read_ad := SOME SPI0_CH0CONF |>` by rw [dr_read_def,dr_read_ch0conf_def] >> fs [] >>
+`(read_SPI_regs_value SPI0_CH0CONF (spi with <|state := xfer_channel_disabled;
+regs := spi.regs with CH0CTRL := 0w |>) = build_CH0CONF spi.regs.CH0CONF) /\
+(read_SPI_regs_state SPI0_CH0CONF (spi with <|state := xfer_channel_disabled;
+regs := spi.regs with CH0CTRL := 0w |>) = (spi with <|state := xfer_channel_disabled;
+regs := spi.regs with CH0CTRL := 0w |>))`
+by fs [read_SPI_regs_value_def,read_SPI_regs_state_def,read_SPI_regs_def,
+SPI0_CH0CTRL_def, SPI0_PA_RANGE_def, SPI0_END_def, SPI0_START_def,SPI0_SYSSTATUS_def,
+SPI0_SYSCONFIG_def, SPI0_MODULCTRL_def, SPI0_CH0CONF_def] >> fs [] >>
+rw [dr_write_state_def,dr_write_address_def,dr_write_value_def,
+dr_write_def, dr_write_ch0conf_xfer_def] >>
+`~ (ch0conf_changed ((4293918719w:word32) && (build_CH0CONF spi.regs.CH0CONF)) 
+(spi with <|state := xfer_channel_disabled;
+regs := spi.regs with CH0CTRL := 0w|>))` 
+by (fs [build_CH0CONF_def,ch0conf_changed_def] >>
+FULL_SIMP_TAC (std_ss++WORD_ss++WORD_BIT_EQ_ss) []) >>
+`spi.regs.CH0CONF.FORCE = 1w` by fs [ref_rel_def] >>
+`(20 >< 20) ((4293918719w:word32) && (build_CH0CONF spi.regs.CH0CONF)) : word1 <> 
+spi.regs.CH0CONF.FORCE` by FULL_SIMP_TAC (std_ss++WORD_ss++WORD_BIT_EQ_ss) [] >>
+`(13 >< 12) ((4293918719w:word32) && (build_CH0CONF spi.regs.CH0CONF)): word2 = 
+spi.regs.CH0CONF.TRM` by (fs [build_CH0CONF_def] >>
+FULL_SIMP_TAC (std_ss++WORD_ss++WORD_BIT_EQ_ss) []) >>
+rw [write_SPI_regs_def, write_CH0CONF_comb_def, write_CH0CONF_xfer_def, 
+SPI0_CH0CTRL_def, SPI0_PA_RANGE_def, SPI0_END_def, SPI0_START_def,
+SPI0_SYSCONFIG_def, SPI0_MODULCTRL_def, SPI0_CH0CONF_def] >>
+FULL_SIMP_TAC (std_ss++WORD_ss++WORD_BIT_EQ_ss) [] >>
+fs [ref_rel_def,IS_STATE_REL_def]]);
 
 (* (dr',spi') exists for xfer *)
 val abs1_comb_hold_ref_rel_tau_comb_xfer = store_thm("abs1_comb_hold_ref_rel_tau_comb_xfer",
